# baseURI: https://w3id.org/con-tax/zones/aat-buildingSites
# prefix: aat-bsites

@prefix : <https://w3id.org/con-tax/zones/aat-buildingSites#> .
@prefix aat: <http://vocab.getty.edu/aat/> .
@prefix aat-bsites: <https://w3id.org/con-tax/zones/aat-buildingSites#> .
@prefix bot: <https://w3id.org/bot#> .
@prefix cc: <http://creativecommons.org/ns#> .
@prefix contax: <https://w3id.org/con-tax#> .
@prefix dbr: <http://dbpedia.org/resource/> .
@prefix dct: <http://purl.org/dc/terms/> .
@prefix dcterms: <http://purl.org/dc/terms/> .
@prefix gvp: <http://vocab.getty.edu/ontology#> .
@prefix iso-thes: <http://purl.org/iso25964/skos-thes#> .
@prefix owl: <http://www.w3.org/2002/07/owl#> .
@prefix rdf: <http://www.w3.org/1999/02/22-rdf-syntax-ns#> .
@prefix rdfs: <http://www.w3.org/2000/01/rdf-schema#> .
@prefix schema: <http://schema.org/> .
@prefix skos: <http://www.w3.org/2004/02/skos/core#> .
@prefix vann: <http://purl.org/vocab/vann/> .
@prefix vcard: <http://www.w3.org/2006/vcard/ns#> .
@prefix voaf: <http://purl.org/vocommons/voaf#> .
@prefix wd: <http://www.wikidata.org/entity/> .
@prefix xl: <http://www.w3.org/2008/05/skos-xl#> .
@prefix xsd: <http://www.w3.org/2001/XMLSchema#> .

bot:Site
  rdf:type owl:Class ;
.
<https://w3id.org/con-tax/zones/aat-buildingSites>
  rdf:type voaf:Vocabulary ;
  rdf:type owl:Ontology ;
  cc:license <https://opendatacommons.org/licenses/by/1-0/> ;
  dcterms:creator [
      rdf:type vcard:Individual ;
      vcard:family-name "Bonduel" ;
      vcard:fn "Mathias Bonduel" ;
      vcard:given-name "Mathias" ;
      vcard:hasOrganizationName [
          rdf:type vcard:Organization ;
          owl:sameAs dbr:Katholieke_Universiteit_Leuven ;
          vcard:hasURL <https://www.kuleuven.be> ;
          vcard:organization-name "KU Leuven" ;
        ] ;
      vcard:hasURL <https://orcid.org/0000-0002-3313-924X> ;
      vcard:hasURL <https://www.kuleuven.be/wieiswie/nl/person/00110827> ;
      vcard:hasURL <https://www.researchgate.net/profile/Mathias_Bonduel> ;
    ] ;
  dcterms:description """A taxonomy of building materials derived from the Getty Art & Architecture Thesaurus (Getty AAT: https://www.getty.edu/research/tools/vocabularies/aat/about.html), v2020-07-29.

Note: Contains information from the J. Paul Getty Trust, Getty Research Institute, the Art & Architecture Thesaurus, which is made available under the ODC Attribution License."""@en ;
  dcterms:issued "2020-11-29"^^xsd:date ;
  dcterms:title "AAT-buildingSITES taxonomy"@en ;
  vann:preferredNamespacePrefix "aat-bsites" ;
  vann:preferredNamespaceUri "https://w3id.org/con-tax/zones/aat-buildingSites#" ;
  rdfs:comment "- Version 0.0.1: initial version"@en ;
  owl:versionInfo "0.0.1" ;
.
<https://w3id.org/con-tax/zones/aat-buildingSites#300000202>
  rdf:type owl:Class ;
  rdfs:comment "Aggregations of buildings, other structures, and/or open spaces, often multifunctional, and more extensive than single built works, usually shaped over a longer period of time by more participants."@en ;
  rdfs:comment "Samenstellingen van gebouwen, andere bouwconstructies en open ruimten, vaak met meerdere functies; zijn uitgebreider en veelzijdiger dan afzonderlijk gebouwen."@nl ;
  rdfs:isDefinedBy <https://w3id.org/con-tax/zones/aat-buildingSites> ;
  rdfs:label "complex (gebouw)"@nl ;
  rdfs:label "complex"@nl ;
  rdfs:label "complexen (gebouwen)"@nl ;
  rdfs:label "complexen"@nl ;
  rdfs:label "complexes (buildings and sites)"@en ;
  rdfs:seeAlso <http://vocab.getty.edu/aat/300000202> ;
  rdfs:seeAlso wd:Q1497364 ;
  rdfs:subClassOf bot:Site ;
  contax:containsGuideTerm <https://w3id.org/con-tax/zones/aat-buildingSites#300000203> ;
  contax:containsGuideTerm <https://w3id.org/con-tax/zones/aat-buildingSites#300128200> ;
.
<https://w3id.org/con-tax/zones/aat-buildingSites#300000203>
  rdf:type gvp:GuideTerm ;
  rdfs:isDefinedBy <https://w3id.org/con-tax/zones/aat-buildingSites> ;
  rdfs:label "<complexen naar functie>"@nl ;
  rdfs:label "<complexes by function>"@en ;
  rdfs:label "complexen naar functie"@nl ;
  rdfs:seeAlso <http://vocab.getty.edu/aat/300000203> ;
  contax:containsConcept <https://w3id.org/con-tax/zones/aat-buildingSites#300000271> ;
  contax:containsConcept <https://w3id.org/con-tax/zones/aat-buildingSites#300000330> ;
  contax:containsConcept <https://w3id.org/con-tax/zones/aat-buildingSites#300000347> ;
  contax:containsConcept <https://w3id.org/con-tax/zones/aat-buildingSites#300000348> ;
  contax:containsConcept <https://w3id.org/con-tax/zones/aat-buildingSites#300000385> ;
  contax:containsConcept <https://w3id.org/con-tax/zones/aat-buildingSites#300000490> ;
  contax:containsConcept <https://w3id.org/con-tax/zones/aat-buildingSites#300000510> ;
  contax:containsConcept <https://w3id.org/con-tax/zones/aat-buildingSites#300000617> ;
  contax:containsConcept <https://w3id.org/con-tax/zones/aat-buildingSites#300000672> ;
  contax:containsConcept <https://w3id.org/con-tax/zones/aat-buildingSites#300000677> ;
  contax:containsConcept <https://w3id.org/con-tax/zones/aat-buildingSites#300000701> ;
  contax:containsConcept <https://w3id.org/con-tax/zones/aat-buildingSites#300000809> ;
  contax:containsConcept <https://w3id.org/con-tax/zones/aat-buildingSites#300008505> ;
  contax:containsConcept <https://w3id.org/con-tax/zones/aat-buildingSites#300122216> ;
  contax:containsConcept <https://w3id.org/con-tax/zones/aat-buildingSites#300125766> ;
  contax:containsConcept <https://w3id.org/con-tax/zones/aat-buildingSites#300132652> ;
  contax:containsConcept <https://w3id.org/con-tax/zones/aat-buildingSites#300164060> ;
  contax:containsConcept <https://w3id.org/con-tax/zones/aat-buildingSites#300259362> ;
  contax:containsConcept <https://w3id.org/con-tax/zones/aat-buildingSites#300262710> ;
  contax:containsConcept <https://w3id.org/con-tax/zones/aat-buildingSites#300263741> ;
  contax:containsConcept <https://w3id.org/con-tax/zones/aat-buildingSites#300386996> ;
  contax:containsConcept <https://w3id.org/con-tax/zones/aat-buildingSites#300387027> ;
  contax:containsConcept <https://w3id.org/con-tax/zones/aat-buildingSites#300387201> ;
  contax:containsConcept <https://w3id.org/con-tax/zones/aat-buildingSites#300410262> ;
  contax:containsConcept <https://w3id.org/con-tax/zones/aat-buildingSites#300417317> ;
.
<https://w3id.org/con-tax/zones/aat-buildingSites#300000206>
  rdf:type owl:Class ;
  rdfs:comment "Complexen waar planten worden verbouwd of dieren gefokt voor levensonderhoud of handel."@nl ;
  rdfs:comment "Complexes where plants or animals are raised for livelihood or commerce."@en ;
  rdfs:isDefinedBy <https://w3id.org/con-tax/zones/aat-buildingSites> ;
  rdfs:label "boerderij (complex)"@nl ;
  rdfs:label "boerderij"@nl ;
  rdfs:label "boerderijen (complexen)"@nl ;
  rdfs:label "boerderijen"@nl ;
  rdfs:label "farms"@en ;
  rdfs:label "hoeven (complexen)"@nl ;
  rdfs:label "hoeven"@nl ;
  rdfs:seeAlso <http://vocab.getty.edu/aat/300000206> ;
  rdfs:seeAlso wd:Q131596 ;
  rdfs:subClassOf <https://w3id.org/con-tax/zones/aat-buildingSites#300125766> ;
  contax:containsGuideTerm <https://w3id.org/con-tax/zones/aat-buildingSites#300000208> ;
  contax:containsGuideTerm <https://w3id.org/con-tax/zones/aat-buildingSites#300000213> ;
.
<https://w3id.org/con-tax/zones/aat-buildingSites#300000208>
  rdf:type gvp:GuideTerm ;
  rdfs:isDefinedBy <https://w3id.org/con-tax/zones/aat-buildingSites> ;
  rdfs:label "<boerderijen naar eigenaar>"@nl ;
  rdfs:label "<farms by ownership>"@en ;
  rdfs:label "boerderijen naar eigenaar"@nl ;
  rdfs:seeAlso <http://vocab.getty.edu/aat/300000208> ;
  contax:containsConcept <https://w3id.org/con-tax/zones/aat-buildingSites#300000210> ;
  contax:containsConcept <https://w3id.org/con-tax/zones/aat-buildingSites#300045490> ;
.
<https://w3id.org/con-tax/zones/aat-buildingSites#300000210>
  rdf:type owl:Class ;
  rdfs:comment "Boerenbedrijven die bestaan uit vele kleine boerderijtjes die zijn samengevoegd tot een eenheid waar gezamenlijk wordt gewerkt en die onder toezicht staan van de overheid of de provincie."@nl ;
  rdfs:comment "Farms consisting of many small holdings collected into a single unit for joint operation by a community under public or state supervision."@en ;
  rdfs:isDefinedBy <https://w3id.org/con-tax/zones/aat-buildingSites> ;
  rdfs:label "collectief landbouwbedrijf"@nl ;
  rdfs:label "collectieve landbouwbedrijven"@nl ;
  rdfs:label "collective farms"@en ;
  rdfs:seeAlso <http://vocab.getty.edu/aat/300000210> ;
  rdfs:seeAlso wd:Q4314084 ;
  rdfs:subClassOf <https://w3id.org/con-tax/zones/aat-buildingSites#300000206> ;
.
<https://w3id.org/con-tax/zones/aat-buildingSites#300000213>
  rdf:type gvp:GuideTerm ;
  rdfs:isDefinedBy <https://w3id.org/con-tax/zones/aat-buildingSites> ;
  rdfs:label "<boerderijen naar functie>"@nl ;
  rdfs:label "<farms by function>"@en ;
  rdfs:label "boerderijen naar functie"@nl ;
  rdfs:seeAlso <http://vocab.getty.edu/aat/300000213> ;
  contax:containsConcept <https://w3id.org/con-tax/zones/aat-buildingSites#300000214> ;
  contax:containsConcept <https://w3id.org/con-tax/zones/aat-buildingSites#300000218> ;
  contax:containsConcept <https://w3id.org/con-tax/zones/aat-buildingSites#300000228> ;
  contax:containsConcept <https://w3id.org/con-tax/zones/aat-buildingSites#300000246> ;
  contax:containsConcept <https://w3id.org/con-tax/zones/aat-buildingSites#300000248> ;
  contax:containsConcept <https://w3id.org/con-tax/zones/aat-buildingSites#300000340> ;
  contax:containsConcept <https://w3id.org/con-tax/zones/aat-buildingSites#300008890> ;
  contax:containsConcept <https://w3id.org/con-tax/zones/aat-buildingSites#300199033> ;
  contax:containsConcept <https://w3id.org/con-tax/zones/aat-buildingSites#300265732> ;
  contax:containsConcept <https://w3id.org/con-tax/zones/aat-buildingSites#300411503> ;
  contax:containsConcept <https://w3id.org/con-tax/zones/aat-buildingSites#300411558> ;
.
<https://w3id.org/con-tax/zones/aat-buildingSites#300000214>
  rdf:type owl:Class ;
  rdfs:comment "Farms chiefly devoted to the raising of dairy cattle and the production of milk, butter, and cheese."@en ;
  rdfs:isDefinedBy <https://w3id.org/con-tax/zones/aat-buildingSites> ;
  rdfs:label "dairy farms"@en ;
  rdfs:label "melkveebedrijf"@nl ;
  rdfs:label "melkveebedrijven"@nl ;
  rdfs:seeAlso <http://vocab.getty.edu/aat/300000214> ;
  rdfs:seeAlso wd:Q14096331 ;
  rdfs:subClassOf <https://w3id.org/con-tax/zones/aat-buildingSites#300000206> ;
.
<https://w3id.org/con-tax/zones/aat-buildingSites#300000218>
  rdf:type owl:Class ;
  rdfs:comment "Farms or areas of forest used to raise trees, typically managed in a way that ensures the regular production of trees to replace those extracted for timber or other purposes."@en ;
  rdfs:isDefinedBy <https://w3id.org/con-tax/zones/aat-buildingSites> ;
  rdfs:label "boomkwekerij (landbouwcomplex)"@nl ;
  rdfs:label "boomkwekerij"@nl ;
  rdfs:label "boomkwekerijen (landbouwcomplexen)"@nl ;
  rdfs:label "boomkwekerijen"@nl ;
  rdfs:label "tree farms"@en ;
  rdfs:seeAlso <http://vocab.getty.edu/aat/300000218> ;
  rdfs:seeAlso wd:Q2843044 ;
  rdfs:subClassOf <https://w3id.org/con-tax/zones/aat-buildingSites#300000206> ;
.
<https://w3id.org/con-tax/zones/aat-buildingSites#300000222>
  rdf:type owl:Class ;
  rdfs:comment "Farms that are considered historical because they preserve methods of rural life and farming from past centuries, whether for tourists, historical preservation, or to produce crops or livestock. For former farms that have been abandoned, use \"abandoned farms.\""@en ;
  rdfs:isDefinedBy <https://w3id.org/con-tax/zones/aat-buildingSites> ;
  rdfs:label "historic farms"@en ;
  rdfs:label "historische boerderij"@nl ;
  rdfs:label "historische boerderijen"@nl ;
  rdfs:label "historische hoven"@nl ;
  rdfs:seeAlso <http://vocab.getty.edu/aat/300000222> ;
  rdfs:subClassOf <https://w3id.org/con-tax/zones/aat-buildingSites#300000206> ;
.
<https://w3id.org/con-tax/zones/aat-buildingSites#300000228>
  rdf:type owl:Class ;
  rdfs:comment "Facilities where fish eggs are hatched and the fry raised, especially to stock lakes, streams, and ponds. Facilities where fish eggs are hatched and the fry raised, especially to stock lakes, streams, and ponds."@en ;
  rdfs:comment "Inrichting waar visseneitjes worden uitgebroed en de jonge vissen, die later in meren, stromen en vijvers worden uitgezet, worden grootgebracht."@nl ;
  rdfs:isDefinedBy <https://w3id.org/con-tax/zones/aat-buildingSites> ;
  rdfs:label "fish hatcheries"@en ;
  rdfs:label "viskwekerij"@nl ;
  rdfs:label "viskwekerijen"@nl ;
  rdfs:seeAlso <http://vocab.getty.edu/aat/300000228> ;
  rdfs:seeAlso wd:Q15615109 ;
  rdfs:subClassOf <https://w3id.org/con-tax/zones/aat-buildingSites#300000206> ;
.
<https://w3id.org/con-tax/zones/aat-buildingSites#300000231>
  rdf:type owl:Class ;
  rdfs:comment "Grote Spaans-Amerikaanse landgoederen, boerderijen of ranches; kan ook worden gebruikt voor het hoofdgebouw van een dergelijk complex."@nl ;
  rdfs:comment "Large Spanish landed estates common to 17th century Seville used as farms, or ranches. Also applies to Spanish-American estates and the main building of such a complex."@en ;
  rdfs:isDefinedBy <https://w3id.org/con-tax/zones/aat-buildingSites> ;
  rdfs:label "haciendas"@en ;
  rdfs:label "haciënda"@nl ;
  rdfs:label "haciënda's"@nl ;
  rdfs:seeAlso <http://vocab.getty.edu/aat/300000231> ;
  rdfs:seeAlso wd:Q917730 ;
  rdfs:subClassOf <https://w3id.org/con-tax/zones/aat-buildingSites#300125766> ;
.
<https://w3id.org/con-tax/zones/aat-buildingSites#300000235>
  rdf:type owl:Class ;
  rdfs:comment "Grote, antieke Romeinse agrarische landgoederen."@nl ;
  rdfs:comment "Large, ancient Roman agricultural estates; for modern Spanish Latin American contexts, prefer \"haciendas.\""@en ;
  rdfs:isDefinedBy <https://w3id.org/con-tax/zones/aat-buildingSites> ;
  rdfs:label "latifundia"@en ;
  rdfs:label "latifundia"@nl ;
  rdfs:label "latifundium"@nl ;
  rdfs:seeAlso <http://vocab.getty.edu/aat/300000235> ;
  rdfs:seeAlso wd:Q428382 ;
  rdfs:subClassOf <https://w3id.org/con-tax/zones/aat-buildingSites#300125766> ;
.
<https://w3id.org/con-tax/zones/aat-buildingSites#300000238>
  rdf:type owl:Class ;
  rdfs:comment "Landed estates administered as units and consisting of the main residence (manor house), demesnes, and the land over which the lord has privileges."@en ;
  rdfs:comment "Wordt gebruikt voor landgoederen die worden beheerd als een geheel en die bestaan uit een hoofdwoning (herenhuis), domeinen en het land waar de landheer privileges heeft."@nl ;
  rdfs:isDefinedBy <https://w3id.org/con-tax/zones/aat-buildingSites> ;
  rdfs:label "landgoed (landbouwcomplex)"@nl ;
  rdfs:label "landgoed"@nl ;
  rdfs:label "landgoederen (landbouwcomplexen)"@nl ;
  rdfs:label "landgoederen"@nl ;
  rdfs:label "manors (agricultural complexes)"@en ;
  rdfs:seeAlso <http://vocab.getty.edu/aat/300000238> ;
  rdfs:subClassOf <https://w3id.org/con-tax/zones/aat-buildingSites#300125766> ;
.
<https://w3id.org/con-tax/zones/aat-buildingSites#300000240>
  rdf:type owl:Class ;
  rdfs:comment "Generally, agricultural complexes usually worked by resident labor. More specifically, large estates in tropical or subtropical regions that are usually cultivated by resident unskilled or semi-skilled labor under central direction. Meaning and usage overlap with \"estates(commercial agricultural holding),\" although such estates are typically smaller enterprises than plantations."@en ;
  rdfs:comment "In algemene zin, landbouwcomplexen die doorgaans worden bewerkt door ter plaatse gehuisveste arbeidskrachten. In meer specifieke zin verwijst de term naar grote landgoederen in tropische of subtropische gebieden die meestal worden bewerkt door ongeschoolde of laaggeschoolde arbeidskrachten, onder centraal toezicht."@nl ;
  rdfs:isDefinedBy <https://w3id.org/con-tax/zones/aat-buildingSites> ;
  rdfs:label "plantage"@nl ;
  rdfs:label "plantages"@nl ;
  rdfs:label "plantations"@en ;
  rdfs:seeAlso <http://vocab.getty.edu/aat/300000240> ;
  rdfs:seeAlso wd:Q188913 ;
  rdfs:subClassOf <https://w3id.org/con-tax/zones/aat-buildingSites#300125766> ;
.
<https://w3id.org/con-tax/zones/aat-buildingSites#300000241>
  rdf:type owl:Class ;
  rdfs:comment "Aanduiding voor vestigingen met veel grond die meestal worden gebruikt om koeien te laten grazen; groter dan boerderijen."@nl ;
  rdfs:comment "Denotes establishments with extensive landholdings usually for the grazing of cattle; larger than farms."@en ;
  rdfs:isDefinedBy <https://w3id.org/con-tax/zones/aat-buildingSites> ;
  rdfs:label "ranch"@nl ;
  rdfs:label "ranches (agricultural complexes)"@en ;
  rdfs:label "ranches"@nl ;
  rdfs:seeAlso <http://vocab.getty.edu/aat/300000241> ;
  rdfs:seeAlso wd:Q509028 ;
  rdfs:subClassOf <https://w3id.org/con-tax/zones/aat-buildingSites#300125766> ;
.
<https://w3id.org/con-tax/zones/aat-buildingSites#300000243>
  rdf:type owl:Class ;
  rdfs:comment "Ranches devoted primarily to the raising of beef cattle."@en ;
  rdfs:isDefinedBy <https://w3id.org/con-tax/zones/aat-buildingSites> ;
  rdfs:label "cattle ranches"@en ;
  rdfs:label "veefokkerij"@nl ;
  rdfs:label "veefokkerijen"@nl ;
  rdfs:label "vetweiderijen"@nl ;
  rdfs:seeAlso <http://vocab.getty.edu/aat/300000243> ;
  rdfs:seeAlso wd:Q509028 ;
  rdfs:subClassOf <https://w3id.org/con-tax/zones/aat-buildingSites#300000241> ;
.
<https://w3id.org/con-tax/zones/aat-buildingSites#300000245>
  rdf:type owl:Class ;
  rdfs:comment "Ranches that provide entertainment for paying guests and tourists who wish to learn to ride horses or bulls, herd cattle, or do other activities associated with ranching."@en ;
  rdfs:isDefinedBy <https://w3id.org/con-tax/zones/aat-buildingSites> ;
  rdfs:label "dude ranches"@en ;
  rdfs:label "vakantieboerderij"@nl ;
  rdfs:label "vakantieboerderijen"@nl ;
  rdfs:seeAlso <http://vocab.getty.edu/aat/300000245> ;
  rdfs:seeAlso wd:Q5615133 ;
  rdfs:subClassOf <https://w3id.org/con-tax/zones/aat-buildingSites#300000241> ;
  rdfs:subClassOf <https://w3id.org/con-tax/zones/aat-buildingSites#300000510> ;
.
<https://w3id.org/con-tax/zones/aat-buildingSites#300000246>
  rdf:type owl:Class ;
  rdfs:comment "Tracts of land devoted to rearing sheep."@en ;
  rdfs:isDefinedBy <https://w3id.org/con-tax/zones/aat-buildingSites> ;
  rdfs:label "schapenfokkerijen"@nl ;
  rdfs:label "schapenhouderij"@nl ;
  rdfs:label "schapenhouderijen"@nl ;
  rdfs:label "sheep farms"@en ;
  rdfs:seeAlso <http://vocab.getty.edu/aat/300000246> ;
  rdfs:seeAlso wd:Q21550984 ;
  rdfs:subClassOf <https://w3id.org/con-tax/zones/aat-buildingSites#300000206> ;
.
<https://w3id.org/con-tax/zones/aat-buildingSites#300000248>
  rdf:type owl:Class ;
  rdfs:comment "Tracts of land on which grapevines are cultivated; plantations of vines."@en ;
  rdfs:isDefinedBy <https://w3id.org/con-tax/zones/aat-buildingSites> ;
  rdfs:label "vineyards"@en ;
  rdfs:label "wijngaard"@nl ;
  rdfs:label "wijngaarden"@nl ;
  rdfs:seeAlso <http://vocab.getty.edu/aat/300000248> ;
  rdfs:seeAlso wd:Q22715 ;
  rdfs:subClassOf <https://w3id.org/con-tax/zones/aat-buildingSites#300000206> ;
.
<https://w3id.org/con-tax/zones/aat-buildingSites#300000250>
  rdf:type owl:Class ;
  rdfs:comment "Widened streets, neighborhood or town squares, or other mostly open public spaces where booths and stalls may be erected for public sales."@en ;
  rdfs:comment "Wordt gebruikt voor verbrede straten, buurt- of stadspleinen of andere meestal openbare ruimten waar kraampjes en stalletjes kunnen worden opgebouwd voor verkoop."@nl ;
  rdfs:isDefinedBy <https://w3id.org/con-tax/zones/aat-buildingSites> ;
  rdfs:label "marketplaces"@en-us ;
  rdfs:label "markt (plein)"@nl ;
  rdfs:label "markt"@nl ;
  rdfs:label "markten (pleinen)"@nl ;
  rdfs:label "markten"@nl ;
  rdfs:label "marktplaats"@nl ;
  rdfs:label "marktplaatsen"@nl ;
  rdfs:seeAlso <http://vocab.getty.edu/aat/300000250> ;
  rdfs:subClassOf <https://w3id.org/con-tax/zones/aat-buildingSites#300132652> ;
.
<https://w3id.org/con-tax/zones/aat-buildingSites#300000256>
  rdf:type owl:Class ;
  rdfs:comment "Marketplaces, usually consisting of a network of covered streets, stalls, booths, and shops, common in parts of North Africa and West Asia."@en ;
  rdfs:comment "Wordt gebruikt voor marktpleinen, meestal bestaande uit een netwerk van overdekte straten, stallen, kramen en winkels, veelvoorkomend in Noord-Afrika en West-Azië."@nl ;
  rdfs:isDefinedBy <https://w3id.org/con-tax/zones/aat-buildingSites> ;
  rdfs:label "bazaar (marktplein)"@nl ;
  rdfs:label "bazaar"@nl ;
  rdfs:label "bazaars (marketplaces)"@en ;
  rdfs:label "bazaars (marktpleinen)"@nl ;
  rdfs:label "bazaars"@nl ;
  rdfs:seeAlso <http://vocab.getty.edu/aat/300000256> ;
  rdfs:seeAlso wd:Q219760 ;
  rdfs:subClassOf <https://w3id.org/con-tax/zones/aat-buildingSites#300000250> ;
.
<https://w3id.org/con-tax/zones/aat-buildingSites#300000271>
  rdf:type owl:Class ;
  rdfs:comment "Buildings housing the offices, stages, backlots, sound stages, and other studios and operations of a motion picture studio company."@en ;
  rdfs:isDefinedBy <https://w3id.org/con-tax/zones/aat-buildingSites> ;
  rdfs:label "filmstudio"@nl ;
  rdfs:label "filmstudio's"@nl ;
  rdfs:label "motion picture studios (building complexes)"@en ;
  rdfs:seeAlso <http://vocab.getty.edu/aat/300000271> ;
  rdfs:seeAlso wd:Q21550789 ;
  rdfs:subClassOf <https://w3id.org/con-tax/zones/aat-buildingSites#300000202> ;
.
<https://w3id.org/con-tax/zones/aat-buildingSites#300000277>
  rdf:type owl:Class ;
  rdfs:comment "Aanduiding voor interneringscentra die worden opgericht los van het gangbare gevangenissysteem, waarin mensen worden opgesloten met het oog op de militaire of politieke veiligheid of voor bestraffing of exploitatie; mensen worden meestal gevangen gezet per decreet of op militair bevel, vaak ook hele klassen of groepen mensen, zonder rekening te houden met de schuldvraag van ieder individu afzonderlijk."@nl ;
  rdfs:comment "Designates internment centers established outside ordinary detention systems in which persons are confined for military or political security or for punishment or exploitation; persons are generally imprisoned by decree or military order, often including classes or groups of people without regard for their individual culpability."@en ;
  rdfs:isDefinedBy <https://w3id.org/con-tax/zones/aat-buildingSites> ;
  rdfs:label "concentratiekamp"@nl ;
  rdfs:label "concentratiekampen"@nl ;
  rdfs:label "concentration camps"@en ;
  rdfs:seeAlso <http://vocab.getty.edu/aat/300000277> ;
  rdfs:seeAlso wd:Q152081 ;
  rdfs:subClassOf <https://w3id.org/con-tax/zones/aat-buildingSites#300122216> ;
.
<https://w3id.org/con-tax/zones/aat-buildingSites#300000280>
  rdf:type owl:Class ;
  rdfs:comment "Distant or overseas settlements established for punishing criminals by forced labour and isolation from society."@en ;
  rdfs:isDefinedBy <https://w3id.org/con-tax/zones/aat-buildingSites> ;
  rdfs:label "penal colonies"@en ;
  rdfs:label "strafkampen"@nl ;
  rdfs:label "strafkolonie"@nl ;
  rdfs:label "strafkolonies"@nl ;
  rdfs:seeAlso <http://vocab.getty.edu/aat/300000280> ;
  rdfs:seeAlso wd:Q1140316 ;
  rdfs:subClassOf <https://w3id.org/con-tax/zones/aat-buildingSites#300122216> ;
.
<https://w3id.org/con-tax/zones/aat-buildingSites#300000281>
  rdf:type owl:Class ;
  rdfs:comment "Minimum-security facilities where inmates work on, usually government-sponsored, forest, woods, or park conservation or maintenance projects."@en ;
  rdfs:comment "Te gebruiken voor minimaal beveiligde strafinrichtingen waar de gestraften worden ingezet bij onderhoudsprojecten van bossen of parken, die meestal door de overheid worden gefinancierd."@nl ;
  rdfs:isDefinedBy <https://w3id.org/con-tax/zones/aat-buildingSites> ;
  rdfs:label "prison camps"@en ;
  rdfs:label "werkkamp (gevangeniscomplex)"@nl ;
  rdfs:label "werkkamp"@nl ;
  rdfs:label "werkkampen (gevangeniscomplexen)"@nl ;
  rdfs:label "werkkampen"@nl ;
  rdfs:seeAlso <http://vocab.getty.edu/aat/300000281> ;
  rdfs:subClassOf <https://w3id.org/con-tax/zones/aat-buildingSites#300122216> ;
.
<https://w3id.org/con-tax/zones/aat-buildingSites#300000291>
  rdf:type owl:Class ;
  rdfs:comment "Aanduiding voor de woning, het land en de eventuele bijgebouwen, waar een familie woont."@nl ;
  rdfs:comment "Designates the dwelling, land, and outbuildings, if any, where a family lives."@en ;
  rdfs:isDefinedBy <https://w3id.org/con-tax/zones/aat-buildingSites> ;
  rdfs:label "homesteads"@en ;
  rdfs:label "woonstede"@nl ;
  rdfs:label "woonsteden"@nl ;
  rdfs:seeAlso <http://vocab.getty.edu/aat/300000291> ;
  rdfs:subClassOf <https://w3id.org/con-tax/zones/aat-buildingSites#300259362> ;
.
<https://w3id.org/con-tax/zones/aat-buildingSites#300000300>
  rdf:type owl:Class ;
  rdfs:comment "Refers to penal colonies where the prisoners are obliged to undertake heavy labor. Refers also to residential camps for migratory workers. "@en ;
  rdfs:comment "Verwijst naar strafinrichtingen waar de gedetineerden zware arbeid moeten verrichten. Verwijst tevens naar woonkampen voor gastarbeiders."@nl ;
  rdfs:isDefinedBy <https://w3id.org/con-tax/zones/aat-buildingSites> ;
  rdfs:label "labor camps"@en-us ;
  rdfs:label "werkkamp"@nl ;
  rdfs:label "werkkampen"@nl ;
  rdfs:seeAlso <http://vocab.getty.edu/aat/300000300> ;
  rdfs:subClassOf <https://w3id.org/con-tax/zones/aat-buildingSites#300259362> ;
.
<https://w3id.org/con-tax/zones/aat-buildingSites#300000307>
  rdf:type owl:Class ;
  rdfs:comment "Planned residential developments, generally publicly built and operated, intended for low- and moderate-income tenants."@en ;
  rdfs:comment "Wordt gebruikt voor bouwprojecten, doorgaans in opdracht van de overheid gebouwd en beheerd, bedoeld voor huurders met lage inkomens."@nl ;
  rdfs:isDefinedBy <https://w3id.org/con-tax/zones/aat-buildingSites> ;
  rdfs:label "housing projects"@en ;
  rdfs:label "huisvestingsproject"@nl ;
  rdfs:label "huisvestingsprojecten"@nl ;
  rdfs:seeAlso <http://vocab.getty.edu/aat/300000307> ;
  rdfs:seeAlso wd:Q6532502 ;
  rdfs:subClassOf <https://w3id.org/con-tax/zones/aat-buildingSites#300259362> ;
.
<https://w3id.org/con-tax/zones/aat-buildingSites#300000319>
  rdf:type owl:Class ;
  rdfs:comment "The dwellings or buildings of Fourierist communities. The dwellings or buildings of Fourierist communities."@en ;
  rdfs:comment "Werkeenheden waarvan de leden in gemeenschap leven; uitgedacht door Fourier. VDE. De woningen of gebouwen van fourieristische gemeenschappen."@nl ;
  rdfs:isDefinedBy <https://w3id.org/con-tax/zones/aat-buildingSites> ;
  rdfs:label "falanstère"@nl ;
  rdfs:label "falanstères"@nl ;
  rdfs:label "phalansteries"@en ;
  rdfs:seeAlso <http://vocab.getty.edu/aat/300000319> ;
  rdfs:seeAlso wd:Q204767 ;
  rdfs:subClassOf <https://w3id.org/con-tax/zones/aat-buildingSites#300259362> ;
.
<https://w3id.org/con-tax/zones/aat-buildingSites#300000326>
  rdf:type owl:Class ;
  rdfs:comment "Distinguished from \"trailer camps\" by being only for infrequently moved prefabricated structures designed for year-round living."@en ;
  rdfs:comment "Onderscheiden van 'caravanterreinen' doordat ze alleen gebruikt worden voor stacaravans."@nl ;
  rdfs:isDefinedBy <https://w3id.org/con-tax/zones/aat-buildingSites> ;
  rdfs:label "mobile home parks"@en ;
  rdfs:label "stacaravanterrein"@nl ;
  rdfs:label "stacaravanterreinen"@nl ;
  rdfs:seeAlso <http://vocab.getty.edu/aat/300000326> ;
  rdfs:seeAlso wd:Q1426493 ;
  rdfs:subClassOf <https://w3id.org/con-tax/zones/aat-buildingSites#300259362> ;
.
<https://w3id.org/con-tax/zones/aat-buildingSites#300000329>
  rdf:type owl:Class ;
  rdfs:comment "Multistory, multiroom complex dwellings, often built on mesas or in cliffs, common among certain Indian cultures of the southwestern United States; distinguished from \"Great Houses (complexes)\" by their location and agglutinated construction."@en ;
  rdfs:comment "Wordt gebruikt voor wooncomplexen met meerdere verdiepingen en meerdere vertrekken, vaak gebouwd op plateau's of in rotswanden, gangbaar bij bepaalde indiaanse culturen in het zuidwesten van de Verenigde Staten; te onderscheiden van 'Great Houses (complexen)' door hun ligging en samengeklonterde opbouw."@nl ;
  rdfs:isDefinedBy <https://w3id.org/con-tax/zones/aat-buildingSites> ;
  rdfs:label "pueblo"@nl ;
  rdfs:label "pueblo's"@nl ;
  rdfs:label "pueblos (housing complexes)"@en ;
  rdfs:seeAlso <http://vocab.getty.edu/aat/300000329> ;
  rdfs:subClassOf <https://w3id.org/con-tax/zones/aat-buildingSites#300259362> ;
.
<https://w3id.org/con-tax/zones/aat-buildingSites#300000330>
  rdf:type owl:Class ;
  rdfs:comment "Complexen van schoolgebouwen en andere faciliteiten; gebruik een specifiekere term waar mogelijk."@nl ;
  rdfs:comment "Groupings of educational buildings and other facilities; if possible, use a more specific term."@en ;
  rdfs:isDefinedBy <https://w3id.org/con-tax/zones/aat-buildingSites> ;
  rdfs:label "educational complexes"@en ;
  rdfs:label "onderwijscomplex"@nl ;
  rdfs:label "onderwijscomplexen"@nl ;
  rdfs:seeAlso <http://vocab.getty.edu/aat/300000330> ;
  rdfs:seeAlso wd:Q20860083 ;
  rdfs:subClassOf <https://w3id.org/con-tax/zones/aat-buildingSites#300000202> ;
.
<https://w3id.org/con-tax/zones/aat-buildingSites#300000333>
  rdf:type owl:Class ;
  rdfs:comment "De bij universiteiten behorende terreinen (sportvelden enz.), ook de terreinen met gebouwen waar studenten (eventueel ook docenten) wonen."@nl ;
  rdfs:comment "Grounds of colleges or universities, including the open space between or around the buildings. The term is also used to refer to the grounds of other building complexes with layouts similar to colleges."@en ;
  rdfs:isDefinedBy <https://w3id.org/con-tax/zones/aat-buildingSites> ;
  rdfs:label "campus"@nl ;
  rdfs:label "campuses"@en ;
  rdfs:label "campussen"@nl ;
  rdfs:seeAlso <http://vocab.getty.edu/aat/300000333> ;
  rdfs:seeAlso wd:Q209465 ;
  rdfs:subClassOf <https://w3id.org/con-tax/zones/aat-buildingSites#300000330> ;
.
<https://w3id.org/con-tax/zones/aat-buildingSites#300000340>
  rdf:type owl:Class ;
  rdfs:comment "Farms attached to education facilities either for the purpose of teaching agriculture or providing meats and produce to the parent institution. Farms attached to education facilities either for the purpose of teaching agriculture or providing meats and produce to the parent institution."@en ;
  rdfs:comment "Wordt gebruikt voor boerderijen die verbonden zijn aan onderwijsinstellingen en waar les gegeven wordt in landbouw of die de school van levensmiddelen voorzien."@nl ;
  rdfs:isDefinedBy <https://w3id.org/con-tax/zones/aat-buildingSites> ;
  rdfs:label "school farms"@en ;
  rdfs:label "schoolboerderij"@nl ;
  rdfs:label "schoolboerderijen"@nl ;
  rdfs:seeAlso <http://vocab.getty.edu/aat/300000340> ;
  rdfs:subClassOf <https://w3id.org/con-tax/zones/aat-buildingSites#300000206> ;
.
<https://w3id.org/con-tax/zones/aat-buildingSites#300000347>
  rdf:type owl:Class ;
  rdfs:comment "Grounds and complexes designed to educate visitors about animals, plants, weather, and the environment, often including structures for educational activities and outdoor grounds containing native plant communities, wildlife habitats, walking trails, and other facilities."@en ;
  rdfs:isDefinedBy <https://w3id.org/con-tax/zones/aat-buildingSites> ;
  rdfs:label "nature centers"@en-us ;
  rdfs:label "natuurcentra"@nl ;
  rdfs:label "natuurcentrum"@nl ;
  rdfs:seeAlso <http://vocab.getty.edu/aat/300000347> ;
  rdfs:subClassOf <https://w3id.org/con-tax/zones/aat-buildingSites#300000202> ;
.
<https://w3id.org/con-tax/zones/aat-buildingSites#300000348>
  rdf:type owl:Class ;
  rdfs:comment "Gardens, parks, or other grounds in which wild animals, and sometimes also domestic animals, are kept for public exhibition, usually in enclosures. Animals in zoos can generally be given more intensive care than is possible in nature reserves or wildlife refuges. Marine invertebrates, fish, and sometimes marine mammals, are often kept in separate aquariums."@en ;
  rdfs:comment "Publieke tuinen waarin een verzameling (vreemde) dieren wordt onderhouden."@nl ;
  rdfs:isDefinedBy <https://w3id.org/con-tax/zones/aat-buildingSites> ;
  rdfs:label "dierentuin"@nl ;
  rdfs:label "dierentuinen"@nl ;
  rdfs:label "diergaarde"@nl ;
  rdfs:label "diergaarden"@nl ;
  rdfs:label "zoos (built complexes)"@en ;
  rdfs:seeAlso <http://vocab.getty.edu/aat/300000348> ;
  rdfs:seeAlso wd:Q43501 ;
  rdfs:subClassOf <https://w3id.org/con-tax/zones/aat-buildingSites#300000202> ;
.
<https://w3id.org/con-tax/zones/aat-buildingSites#300000351>
  rdf:type owl:Class ;
  rdfs:comment "Zoos designed for the education and enjoyment of children and young adults, often including a petting zoo, animal shows, and exhibits of baby animals."@en ;
  rdfs:isDefinedBy <https://w3id.org/con-tax/zones/aat-buildingSites> ;
  rdfs:label "children's zoos"@en ;
  rdfs:label "kinderdierentuin"@nl ;
  rdfs:label "kinderdierentuinen"@nl ;
  rdfs:seeAlso <http://vocab.getty.edu/aat/300000351> ;
  rdfs:subClassOf <https://w3id.org/con-tax/zones/aat-buildingSites#300000348> ;
.
<https://w3id.org/con-tax/zones/aat-buildingSites#300000353>
  rdf:type owl:Class ;
  rdfs:comment "Plaatsen waar wilde of bijzondere dieren worden gehouden of vertoond."@nl ;
  rdfs:comment "Places where collections of wild or unusual animals are kept or exhibited in cages, particularly the early collections of emperors, kings, or other elite collectors, or 19th- and early 20th-century traveling exhibitions of caged animals. Traveling menageries were distinct from circuses in that the animals did not normally perform tricks."@en ;
  rdfs:isDefinedBy <https://w3id.org/con-tax/zones/aat-buildingSites> ;
  rdfs:label "menagerie"@nl ;
  rdfs:label "menageries"@en ;
  rdfs:label "menagerieën"@nl ;
  rdfs:seeAlso <http://vocab.getty.edu/aat/300000353> ;
  rdfs:seeAlso wd:Q1401536 ;
  rdfs:subClassOf <https://w3id.org/con-tax/zones/aat-buildingSites#300000348> ;
.
<https://w3id.org/con-tax/zones/aat-buildingSites#300000354>
  rdf:type owl:Class ;
  rdfs:comment "Zoos in which many or all of the animals have access to open-air enclosures that resemble the animals' natural habitats, in contrast to early zoos where most animals were confined to relatively small cages. Zoos in which many or all of the animals have access to open-air enclosures that resemble the animals' natural habitats, in contrast to early zoos where most animals were confined to relatively small cages."@en ;
  rdfs:isDefinedBy <https://w3id.org/con-tax/zones/aat-buildingSites> ;
  rdfs:label "open-air zoos"@en ;
  rdfs:label "openluchtdierentuin"@nl ;
  rdfs:label "openluchtdierentuinen"@nl ;
  rdfs:seeAlso <http://vocab.getty.edu/aat/300000354> ;
  rdfs:seeAlso wd:Q21550840 ;
  rdfs:subClassOf <https://w3id.org/con-tax/zones/aat-buildingSites#300000348> ;
.
<https://w3id.org/con-tax/zones/aat-buildingSites#300000357>
  rdf:type owl:Class ;
  rdfs:comment "Distinguished from \"safari parks\" by the complete and planned separation of the visiting public from the animals, who are allowed to roam freely within bounded natural habitats. Distinguished from \"safari parks\" by the complete and planned separation of the visiting public from the animals, who are allowed to roam freely within bounded natural habitats."@en ;
  rdfs:comment "Te onderscheiden van 'safariparken' door de volledige en geplande afscheiding tussen bezoekers en dieren die vrij kunnen rondlopen binnen een begrensde natuurlijke omgeving."@nl ;
  rdfs:isDefinedBy <https://w3id.org/con-tax/zones/aat-buildingSites> ;
  rdfs:label "wild animal parks"@en ;
  rdfs:label "wilde-dierenpark"@nl ;
  rdfs:label "wilde-dierenparken"@nl ;
  rdfs:seeAlso <http://vocab.getty.edu/aat/300000357> ;
  rdfs:seeAlso wd:Q21550840 ;
  rdfs:subClassOf <https://w3id.org/con-tax/zones/aat-buildingSites#300000354> ;
.
<https://w3id.org/con-tax/zones/aat-buildingSites#300000385>
  rdf:type owl:Class ;
  rdfs:comment "Algemene term voor ieder samenstel van verschillende soorten industriële gebouwen en aanverwante voorzieningen."@nl ;
  rdfs:comment "Use generally for any grouping of diversified industrial buildings and related facilities."@en ;
  rdfs:isDefinedBy <https://w3id.org/con-tax/zones/aat-buildingSites> ;
  rdfs:label "industrial complexes"@en ;
  rdfs:label "industrieel complex"@nl ;
  rdfs:label "industriële complexen"@nl ;
  rdfs:seeAlso <http://vocab.getty.edu/aat/300000385> ;
  rdfs:subClassOf <https://w3id.org/con-tax/zones/aat-buildingSites#300000202> ;
.
<https://w3id.org/con-tax/zones/aat-buildingSites#300000403>
  rdf:type owl:Class ;
  rdfs:comment "Plaatsen of ruimten waar boten en schepen worden gebouwd of hersteld."@nl ;
  rdfs:comment "Places or enclosures where ships are built or repaired. For places servicing small vessels, use \"boatyards.\" Places or enclosures where boats or ships are built or repaired."@en ;
  rdfs:isDefinedBy <https://w3id.org/con-tax/zones/aat-buildingSites> ;
  rdfs:label "scheepswerf"@nl ;
  rdfs:label "scheepswerven"@nl ;
  rdfs:label "shipyards"@en ;
  rdfs:seeAlso <http://vocab.getty.edu/aat/300000403> ;
  rdfs:seeAlso wd:Q190928 ;
  rdfs:subClassOf <https://w3id.org/con-tax/zones/aat-buildingSites#300120802> ;
.
<https://w3id.org/con-tax/zones/aat-buildingSites#300000410>
  rdf:type owl:Class ;
  rdfs:comment "Groups of houses or tents and associated facilities designed as a residence for loggers who are temporarily in a forest to cut down and transport timber."@en ;
  rdfs:isDefinedBy <https://w3id.org/con-tax/zones/aat-buildingSites> ;
  rdfs:label "houthakkerskamp"@nl ;
  rdfs:label "houthakkerskampen"@nl ;
  rdfs:label "lumber camps"@en ;
  rdfs:seeAlso <http://vocab.getty.edu/aat/300000410> ;
  rdfs:seeAlso wd:Q21550750 ;
  rdfs:subClassOf <https://w3id.org/con-tax/zones/aat-buildingSites#300259362> ;
.
<https://w3id.org/con-tax/zones/aat-buildingSites#300000411>
  rdf:type owl:Class ;
  rdfs:comment "Refers to areas zoned and planned for so-called clean industries, developed and managed as a unit, where plots are offered fully equipped with transport and installation facilities, often already including a number of multi-use buildings."@en ;
  rdfs:comment "Wordt gebruikt voor gebieden die zijn bestemd en gepland voor zogenaamde schone industrie, en die worden ontwikkeld en beheerd als een eenheid en waar percelen worden aangeboden met alle vervoers- en vestigingsvoorzieningen, doorgaans ook met een aantal multifunctionele gebouwen."@nl ;
  rdfs:isDefinedBy <https://w3id.org/con-tax/zones/aat-buildingSites> ;
  rdfs:label "industrial parks"@en ;
  rdfs:label "industriepark"@nl ;
  rdfs:label "industrieparken"@nl ;
  rdfs:seeAlso <http://vocab.getty.edu/aat/300000411> ;
  rdfs:seeAlso wd:Q329683 ;
  rdfs:subClassOf <https://w3id.org/con-tax/zones/aat-buildingSites#300000385> ;
.
<https://w3id.org/con-tax/zones/aat-buildingSites#300000414>
  rdf:type owl:Class ;
  rdfs:comment "Complexes of buildings and other structures with machinery for generating electricity. For individual buildings in which electricity, or other forms of power, are generated for the operation of machinery or vehicles, or supplying power to other buildings in a complex, use \"powerhouses.\""@en ;
  rdfs:comment "Wordt gebruikt voor complexen van gebouwen of andere bouwwerken met apparatuur voor het opwekken van elektriciteit."@nl ;
  rdfs:isDefinedBy <https://w3id.org/con-tax/zones/aat-buildingSites> ;
  rdfs:label "elektriciteitscentrales"@nl ;
  rdfs:label "elektrische centrales"@nl ;
  rdfs:label "energiecentrales"@nl ;
  rdfs:label "krachtcentrale"@nl ;
  rdfs:label "krachtcentrales"@nl ;
  rdfs:label "power plants"@en-us ;
  rdfs:seeAlso <http://vocab.getty.edu/aat/300000414> ;
  rdfs:subClassOf <https://w3id.org/con-tax/zones/aat-buildingSites#300000385> ;
.
<https://w3id.org/con-tax/zones/aat-buildingSites#300000420>
  rdf:type owl:Class ;
  rdfs:comment "Krachtcentrale waarin gas wordt verbrand met samengeperste lucht of olie, om stoom aangedreven turbines die elektrische energie produceren aan te drijven."@nl ;
  rdfs:comment "Power plants in which gas is burned, with compressed air or oil, to run steam-driven turbines that produce electrical energy."@en ;
  rdfs:isDefinedBy <https://w3id.org/con-tax/zones/aat-buildingSites> ;
  rdfs:label "gas-turbine power plants"@en ;
  rdfs:label "gasturbine-elektriciteitscentrales"@nl ;
  rdfs:label "gasturbinekrachtcentrale"@nl ;
  rdfs:label "gasturbinekrachtcentrales"@nl ;
  rdfs:seeAlso <http://vocab.getty.edu/aat/300000420> ;
  rdfs:seeAlso wd:Q1427536 ;
  rdfs:subClassOf <https://w3id.org/con-tax/zones/aat-buildingSites#300000431> ;
.
<https://w3id.org/con-tax/zones/aat-buildingSites#300000422>
  rdf:type owl:Class ;
  rdfs:comment "Elektriciteitscentrales waar elektriciteit wordt opgewekt met behulp van de energie van stromend water."@nl ;
  rdfs:comment "Power plants in which electricity is produced using the energy of flowing water."@en ;
  rdfs:isDefinedBy <https://w3id.org/con-tax/zones/aat-buildingSites> ;
  rdfs:label "hydroelectric power plants"@en-us ;
  rdfs:label "waterkrachtcentrale"@nl ;
  rdfs:label "waterkrachtcentrales"@nl ;
  rdfs:seeAlso <http://vocab.getty.edu/aat/300000422> ;
  rdfs:subClassOf <https://w3id.org/con-tax/zones/aat-buildingSites#300000414> ;
.
<https://w3id.org/con-tax/zones/aat-buildingSites#300000425>
  rdf:type owl:Class ;
  rdfs:comment "Elektriciteitscentrales waarbij in periodes dat de vraag naar elektriciteit klein is, water naar grote hoogte wordt gepompt en daar wordt opgeslagen tot de vraag naar energie stijgt en dan wordt vrijgelaten waardoor hydraulische turbines worden aangedreven die de benodigde elektriciteit produceren."@nl ;
  rdfs:comment "Power plants using water pumped to and stored at a high elevation during periods of low energy demand, for use when demand is high, when water is released to operate hydraulic turbines to produce needed electricity."@en ;
  rdfs:isDefinedBy <https://w3id.org/con-tax/zones/aat-buildingSites> ;
  rdfs:label "pumped storage power plants"@en ;
  rdfs:label "spaarbekkencentrale"@nl ;
  rdfs:label "spaarbekkencentrales"@nl ;
  rdfs:seeAlso <http://vocab.getty.edu/aat/300000425> ;
  rdfs:seeAlso wd:Q339353 ;
  rdfs:subClassOf <https://w3id.org/con-tax/zones/aat-buildingSites#300000422> ;
.
<https://w3id.org/con-tax/zones/aat-buildingSites#300000426>
  rdf:type owl:Class ;
  rdfs:comment "Elektrische centrales die werken door middel van getijstroom."@nl ;
  rdfs:comment "Facilities designed to extract and store energy, employing one or more of the following methods, or other methods: harnessing energy from the differences between high tides and low tides by employing a \"barrage\" or type of dam to block receding water during ebb periods, the subsequent release of the water through a turbine generating electricity as the tide rises (similar to the workings of hydroelectric dams); using tidal stream power by utilizing ocean currents to drive turbines, particularly in areas around islands or coasts where these currents are fast, including systems that employ tidal fences where turbines are stretched across a channel or tidal turbines that resemble underwater wind turbines; using wave power systems to harness energy from the up-and-down motion of waves to drive energy production, installed in shoreline areas as well as offshore."@en ;
  rdfs:isDefinedBy <https://w3id.org/con-tax/zones/aat-buildingSites> ;
  rdfs:label "getijcentrale"@nl ;
  rdfs:label "getijcentrales"@nl ;
  rdfs:label "tidal power plants"@en ;
  rdfs:seeAlso <http://vocab.getty.edu/aat/300000426> ;
  rdfs:subClassOf <https://w3id.org/con-tax/zones/aat-buildingSites#300000422> ;
.
<https://w3id.org/con-tax/zones/aat-buildingSites#300000428>
  rdf:type owl:Class ;
  rdfs:comment "Facilities that harness and distribute energy derived from the sun's radiation by producing heat, causing chemical reactions, or generating electricity in any of several methods, including but not limited to the following: by the using direct solar radiation to heat air, water, or another carrier fluid; by using arrays of lenses or mirrors as solar collectors to concentrate sunlight to produce high temperatures in a solar furnace; or by using solar cells (photovoltaic cells) to convert solar radiation into electricity when a small electric voltage is generated in the solar cell as light strikes the junction between a metal and a semiconductor (such as silicon) or the junction between two different semiconductors."@en ;
  rdfs:isDefinedBy <https://w3id.org/con-tax/zones/aat-buildingSites> ;
  rdfs:label "solar power plants"@en ;
  rdfs:label "zonne-energiecentrale"@nl ;
  rdfs:label "zonne-energiecentrales"@nl ;
  rdfs:seeAlso <http://vocab.getty.edu/aat/300000428> ;
  rdfs:seeAlso wd:Q1003207 ;
  rdfs:subClassOf <https://w3id.org/con-tax/zones/aat-buildingSites#300000414> ;
.
<https://w3id.org/con-tax/zones/aat-buildingSites#300000430>
  rdf:type owl:Class ;
  rdfs:comment "Elektriciteitscentrales die elektriciteit produceren door gebruik te maken van het temperatuurverschil tussen oppervlaktewater dat wordt verwarmd door de zon en koud water uit de diepte dat naar de oppervlakte wordt gepompt."@nl ;
  rdfs:comment "Power plants producing electricity by utilizing temperature differentials between surface water heated by the sun and deep cold water pumped to the surface. Power plants producing electricity by utilizing temperature differentials between surface water heated by the sun and deep cold water pumped to the surface."@en ;
  rdfs:isDefinedBy <https://w3id.org/con-tax/zones/aat-buildingSites> ;
  rdfs:label "ocean thermal energy conversion plant"@nl ;
  rdfs:label "ocean thermal energy conversion plants"@en ;
  rdfs:label "ocean thermal energy conversion plants"@nl ;
  rdfs:seeAlso <http://vocab.getty.edu/aat/300000430> ;
  rdfs:seeAlso wd:Q20860098 ;
  rdfs:subClassOf <https://w3id.org/con-tax/zones/aat-buildingSites#300000428> ;
.
<https://w3id.org/con-tax/zones/aat-buildingSites#300000431>
  rdf:type owl:Class ;
  rdfs:comment "Gebruikt voor elektriciteitscentrales waarvan de voornaamste aandrijfmechanismen, voornamelijk turbines, verbonden met de generatoren worden aangedreven door stoom om de elektriciteit te genereren."@nl ;
  rdfs:comment "Power plants in which the prime movers, usually turbines, connected to the generators are driven by steam to produce electricity."@en ;
  rdfs:isDefinedBy <https://w3id.org/con-tax/zones/aat-buildingSites> ;
  rdfs:label "steam power plants"@en ;
  rdfs:label "stoom-elektriciteitscentrales"@nl ;
  rdfs:label "stoomkrachtcentrale"@nl ;
  rdfs:label "stoomkrachtcentrales"@nl ;
  rdfs:seeAlso <http://vocab.getty.edu/aat/300000431> ;
  rdfs:seeAlso wd:Q1158818 ;
  rdfs:subClassOf <https://w3id.org/con-tax/zones/aat-buildingSites#300000414> ;
.
<https://w3id.org/con-tax/zones/aat-buildingSites#300000434>
  rdf:type owl:Class ;
  rdfs:comment "Elektriciteitscentrales op stoom, waarbij kolen als voornaamste brandstof wordt gebruikt."@nl ;
  rdfs:comment "Steam-producing, electric power generating plants using coal as the primary fuel."@en ;
  rdfs:isDefinedBy <https://w3id.org/con-tax/zones/aat-buildingSites> ;
  rdfs:label "coal-fired power plants"@en ;
  rdfs:label "kolengestookte centrale"@nl ;
  rdfs:label "kolengestookte centrales"@nl ;
  rdfs:seeAlso <http://vocab.getty.edu/aat/300000434> ;
  rdfs:seeAlso wd:Q6558431 ;
  rdfs:subClassOf <https://w3id.org/con-tax/zones/aat-buildingSites#300000431> ;
.
<https://w3id.org/con-tax/zones/aat-buildingSites#300000438>
  rdf:type owl:Class ;
  rdfs:comment "Elektriciteitscentrales die op stoom uit geothermale bronnen werken, bijvoorbeeld geisers, heetwaterbronnen of vulkanen. LEH."@nl ;
  rdfs:comment "Power plants using steam generated by geothermal sources, such as geysers, hot springs, or volcanoes."@en ;
  rdfs:isDefinedBy <https://w3id.org/con-tax/zones/aat-buildingSites> ;
  rdfs:label "geothermal power plants"@en ;
  rdfs:label "geothermische centrale"@nl ;
  rdfs:label "geothermische centrales"@nl ;
  rdfs:seeAlso <http://vocab.getty.edu/aat/300000438> ;
  rdfs:seeAlso wd:Q30565277 ;
  rdfs:subClassOf <https://w3id.org/con-tax/zones/aat-buildingSites#300000431> ;
.
<https://w3id.org/con-tax/zones/aat-buildingSites#300000439>
  rdf:type owl:Class ;
  rdfs:comment "Facilities that create and distribute power obtained from nuclear reactors, which initiate and control a self-sustaining series of nuclear fissions."@en ;
  rdfs:isDefinedBy <https://w3id.org/con-tax/zones/aat-buildingSites> ;
  rdfs:label "atoomcentrale"@nl ;
  rdfs:label "atoomcentrales"@nl ;
  rdfs:label "kerncentrales"@nl ;
  rdfs:label "kernenergiecentrales"@nl ;
  rdfs:label "nucleaire centrale"@nl ;
  rdfs:label "nucleaire centrales"@nl ;
  rdfs:label "nuclear power plants"@en ;
  rdfs:seeAlso <http://vocab.getty.edu/aat/300000439> ;
  rdfs:seeAlso wd:Q134447 ;
  rdfs:subClassOf <https://w3id.org/con-tax/zones/aat-buildingSites#300000431> ;
.
<https://w3id.org/con-tax/zones/aat-buildingSites#300000444>
  rdf:type owl:Class ;
  rdfs:comment "Large scale energy conversion centers that burn the fossil fuel oil to produce electricity. Large scale energy conversion centers that burn the fossil fuel oil to produce electricity."@en ;
  rdfs:isDefinedBy <https://w3id.org/con-tax/zones/aat-buildingSites> ;
  rdfs:label "oil-fired power plants"@en ;
  rdfs:label "oliegestookte elektriciteitscentrales"@nl ;
  rdfs:label "oliegestookte krachtcentrale"@nl ;
  rdfs:label "oliegestookte krachtcentrales"@nl ;
  rdfs:seeAlso <http://vocab.getty.edu/aat/300000444> ;
  rdfs:subClassOf <https://w3id.org/con-tax/zones/aat-buildingSites#300000431> ;
.
<https://w3id.org/con-tax/zones/aat-buildingSites#300000445>
  rdf:type owl:Class ;
  rdfs:comment "Facilities designed for the creation and distribution of power derived from wind, where turbines convert the kinetic energy of wind into mechanical or electrical energy that can be used for power."@en ;
  rdfs:isDefinedBy <https://w3id.org/con-tax/zones/aat-buildingSites> ;
  rdfs:label "wind power plants"@en ;
  rdfs:label "windkrachtcentrale"@nl ;
  rdfs:label "windkrachtcentrales"@nl ;
  rdfs:seeAlso <http://vocab.getty.edu/aat/300000445> ;
  rdfs:seeAlso wd:Q194356 ;
  rdfs:subClassOf <https://w3id.org/con-tax/zones/aat-buildingSites#300000414> ;
.
<https://w3id.org/con-tax/zones/aat-buildingSites#300000451>
  rdf:type owl:Class ;
  rdfs:comment "Use only for military weapons testing; for small arms target ranges, use \"shooting ranges\" or a more specific term."@en ;
  rdfs:comment "Wordt alleen gebruikt voor het uittesten van militaire wapens; gebruik 'schietterreinen' of een specifiekere term voor oefenterreinen voor kleine vuurwapens."@nl ;
  rdfs:isDefinedBy <https://w3id.org/con-tax/zones/aat-buildingSites> ;
  rdfs:label "firing ranges"@en ;
  rdfs:label "testgebied"@nl ;
  rdfs:label "testgebieden"@nl ;
  rdfs:seeAlso <http://vocab.getty.edu/aat/300000451> ;
  rdfs:seeAlso wd:Q521839 ;
  rdfs:subClassOf <https://w3id.org/con-tax/zones/aat-buildingSites#300000617> ;
.
<https://w3id.org/con-tax/zones/aat-buildingSites#300000455>
  rdf:type owl:Class ;
  rdfs:comment "Use generally in contemporary contexts for permanent centers of operations; use \"military camps\" for contemporary nonpermanent posts."@en ;
  rdfs:comment "Wordt tegenwoordig doorgaans gebruikt voor permanente militaire bases; gebruik 'kampementen' voor tijdelijke posten."@nl ;
  rdfs:isDefinedBy <https://w3id.org/con-tax/zones/aat-buildingSites> ;
  rdfs:label "militaire bases"@nl ;
  rdfs:label "militaire basis"@nl ;
  rdfs:label "military bases"@en ;
  rdfs:seeAlso <http://vocab.getty.edu/aat/300000455> ;
  rdfs:seeAlso wd:Q245016 ;
  rdfs:subClassOf <https://w3id.org/con-tax/zones/aat-buildingSites#300164060> ;
.
<https://w3id.org/con-tax/zones/aat-buildingSites#300000456>
  rdf:type owl:Class ;
  rdfs:comment "Bases for the operation of military aircraft."@en ;
  rdfs:isDefinedBy <https://w3id.org/con-tax/zones/aat-buildingSites> ;
  rdfs:label "air bases"@en ;
  rdfs:label "luchtmachtbases"@nl ;
  rdfs:label "luchtmachtbasis"@nl ;
  rdfs:seeAlso <http://vocab.getty.edu/aat/300000456> ;
  rdfs:seeAlso wd:Q695850 ;
  rdfs:subClassOf <https://w3id.org/con-tax/zones/aat-buildingSites#300000455> ;
.
<https://w3id.org/con-tax/zones/aat-buildingSites#300000459>
  rdf:type owl:Class ;
  rdfs:comment "Land-based military airbases for the military aviation division of the navy of a nation."@en ;
  rdfs:isDefinedBy <https://w3id.org/con-tax/zones/aat-buildingSites> ;
  rdfs:label "marineluchtvaartbases"@nl ;
  rdfs:label "marineluchtvaartbasis"@nl ;
  rdfs:label "naval air bases"@en ;
  rdfs:seeAlso <http://vocab.getty.edu/aat/300000459> ;
  rdfs:subClassOf <https://w3id.org/con-tax/zones/aat-buildingSites#300000456> ;
.
<https://w3id.org/con-tax/zones/aat-buildingSites#300000461>
  rdf:type owl:Class ;
  rdfs:comment "Een permanente militaire bases waar een plaatselijke commandant de leiding heeft, die bestaat uit ondersteunende faciliteiten die nodig zijn bij legeractiviteiten, inclusief beveiliging, interne communicatie en nutssystemen."@nl ;
  rdfs:comment "Permanent group of installations for which a local commander is responsible, consisting of support facilities necessary for army activities, including security, internal communications, and utility systems."@en ;
  rdfs:isDefinedBy <https://w3id.org/con-tax/zones/aat-buildingSites> ;
  rdfs:label "army bases"@en ;
  rdfs:label "legerbases"@nl ;
  rdfs:label "legerbasis"@nl ;
  rdfs:seeAlso <http://vocab.getty.edu/aat/300000461> ;
  rdfs:subClassOf <https://w3id.org/con-tax/zones/aat-buildingSites#300000455> ;
.
<https://w3id.org/con-tax/zones/aat-buildingSites#300000462>
  rdf:type owl:Class ;
  rdfs:comment "Military bases for the storage and deployment of guided missiles, which are self-propelled projectiles used as weapons, including but not limited to long-range ballistic missiles."@en ;
  rdfs:isDefinedBy <https://w3id.org/con-tax/zones/aat-buildingSites> ;
  rdfs:label "guided missile bases"@en ;
  rdfs:label "raketbases (geleide raketten)"@nl ;
  rdfs:label "raketbases"@nl ;
  rdfs:label "raketbasis (geleide raketten)"@nl ;
  rdfs:label "raketbasis"@nl ;
  rdfs:seeAlso <http://vocab.getty.edu/aat/300000462> ;
  rdfs:subClassOf <https://w3id.org/con-tax/zones/aat-buildingSites#300000455> ;
.
<https://w3id.org/con-tax/zones/aat-buildingSites#300000465>
  rdf:type owl:Class ;
  rdfs:comment "Facilities specializing in the training of military personnel, typically including training in the use of weapons, discipline, endurance, and survival training."@en ;
  rdfs:isDefinedBy <https://w3id.org/con-tax/zones/aat-buildingSites> ;
  rdfs:label "militair trainingskamp"@nl ;
  rdfs:label "militaire opleidingskampen"@nl ;
  rdfs:label "militaire trainingskampen"@nl ;
  rdfs:label "military training camps"@en ;
  rdfs:seeAlso <http://vocab.getty.edu/aat/300000465> ;
  rdfs:subClassOf <https://w3id.org/con-tax/zones/aat-buildingSites#300164060> ;
.
<https://w3id.org/con-tax/zones/aat-buildingSites#300000467>
  rdf:type owl:Class ;
  rdfs:comment "Area naval commands normally including a seaport, which integrates shore activities that provide local logistic services to the fleet."@en ;
  rdfs:comment "Marinebasis, meestal met een zeehaven, waar aan wal de plaatselijke logistieke diensten voor de vloot worden verzorgd."@nl ;
  rdfs:isDefinedBy <https://w3id.org/con-tax/zones/aat-buildingSites> ;
  rdfs:label "marinebases"@nl ;
  rdfs:label "marinebasis"@nl ;
  rdfs:label "naval bases"@en ;
  rdfs:seeAlso <http://vocab.getty.edu/aat/300000467> ;
  rdfs:seeAlso wd:Q1324633 ;
  rdfs:subClassOf <https://w3id.org/con-tax/zones/aat-buildingSites#300000455> ;
.
<https://w3id.org/con-tax/zones/aat-buildingSites#300000472>
  rdf:type owl:Class ;
  rdfs:comment "Marinebases waar oorlogsschepen worden gebouwd, hersteld, gedokt of omgebouwd door civiele ingenieurs en arbeiders en die worden beheerd door genie-officieren."@nl ;
  rdfs:comment "Naval bases that build, repair, dock, or convert warships, and are manned by civilian engineers and workers and administered by engineer duty officers."@en ;
  rdfs:isDefinedBy <https://w3id.org/con-tax/zones/aat-buildingSites> ;
  rdfs:label "marinewerf"@nl ;
  rdfs:label "marinewerven"@nl ;
  rdfs:label "naval shipyards"@en ;
  rdfs:seeAlso <http://vocab.getty.edu/aat/300000472> ;
  rdfs:subClassOf <https://w3id.org/con-tax/zones/aat-buildingSites#300000467> ;
.
<https://w3id.org/con-tax/zones/aat-buildingSites#300000475>
  rdf:type owl:Class ;
  rdfs:comment "Military bases that shelter and deploy submarines and personnel."@en ;
  rdfs:comment "Plaatsen, havens waar duikboten gestationeerd zijn, vanwaaruit zij varen."@nl ;
  rdfs:isDefinedBy <https://w3id.org/con-tax/zones/aat-buildingSites> ;
  rdfs:label "duikbootbases"@nl ;
  rdfs:label "duikbootbasis"@nl ;
  rdfs:label "submarine bases"@en ;
  rdfs:seeAlso <http://vocab.getty.edu/aat/300000475> ;
  rdfs:seeAlso wd:Q331367 ;
  rdfs:subClassOf <https://w3id.org/con-tax/zones/aat-buildingSites#300000467> ;
.
<https://w3id.org/con-tax/zones/aat-buildingSites#300000476>
  rdf:type owl:Class ;
  rdfs:comment "In contemporary military contexts this refers to groups of huts, tents, or other shelters set up temporarily for troops. In historical contexts the term connotes permanent or semipermanent places of encampment. Use \"military bases\" for contemporary permanent installations. In contemporary military contexts this refers to groups of huts, tents, or other shelters set up temporarily for troops. In historical contexts the term connotes permanent or semipermanent places of encampment. Use \"military bases\" for contemporary permanent installations."@en ;
  rdfs:comment "Wordt in hedendaags militair verband gebruikt voor groepen hutten, tenten of ander tijdelijk onderdak voor troepen; wordt in historische context gebruikt voor permanenete of semipermanente kampplaatsen; gebruik 'militaire bases' voor hedendaagse permanente legerplaatsen."@nl ;
  rdfs:isDefinedBy <https://w3id.org/con-tax/zones/aat-buildingSites> ;
  rdfs:label "militair kamp"@nl ;
  rdfs:label "militaire kampen"@nl ;
  rdfs:label "military camps"@en ;
  rdfs:seeAlso <http://vocab.getty.edu/aat/300000476> ;
  rdfs:seeAlso wd:Q1198413 ;
  rdfs:subClassOf <https://w3id.org/con-tax/zones/aat-buildingSites#300164060> ;
.
<https://w3id.org/con-tax/zones/aat-buildingSites#300000484>
  rdf:type owl:Class ;
  rdfs:comment "Multifunctional Islamic fortified outposts generally reserved for warriors of the Faith who are committed to defense of frontiers and to proselytizing. Multifunctional Islamic fortified outposts generally reserved for warriors of the Faith who are committed to defense of frontiers and to proselytizing."@en ;
  rdfs:comment "Wordt gebruikt voor multifunctionele, islamitische versterkte buitenposten die meestal zijn alleen zijn bestemd voor strijders voor het Geloof, die zich toeleggen op de verdediging van grenzen en het bekeren van mensen."@nl ;
  rdfs:isDefinedBy <https://w3id.org/con-tax/zones/aat-buildingSites> ;
  rdfs:label "ribat"@nl ;
  rdfs:label "ribats"@en ;
  rdfs:label "ribats"@nl ;
  rdfs:seeAlso <http://vocab.getty.edu/aat/300000484> ;
  rdfs:seeAlso wd:Q1333989 ;
  rdfs:subClassOf <https://w3id.org/con-tax/zones/aat-buildingSites#300000476> ;
.
<https://w3id.org/con-tax/zones/aat-buildingSites#300000485>
  rdf:type owl:Class ;
  rdfs:comment "Target range for guided missiles."@en ;
  rdfs:isDefinedBy <https://w3id.org/con-tax/zones/aat-buildingSites> ;
  rdfs:label "guided missile ranges"@en ;
  rdfs:label "testgebied voor geleide projectielen"@nl ;
  rdfs:label "testgebieden voor geleide projectielen"@nl ;
  rdfs:seeAlso <http://vocab.getty.edu/aat/300000485> ;
  rdfs:subClassOf <https://w3id.org/con-tax/zones/aat-buildingSites#300000617> ;
.
<https://w3id.org/con-tax/zones/aat-buildingSites#300000490>
  rdf:type owl:Class ;
  rdfs:comment "Building complexes that house offices and facilities for the support of the offices."@en ;
  rdfs:isDefinedBy <https://w3id.org/con-tax/zones/aat-buildingSites> ;
  rdfs:label "kantoorcomplex"@nl ;
  rdfs:label "kantoorcomplexen"@nl ;
  rdfs:label "office complexes"@en ;
  rdfs:seeAlso <http://vocab.getty.edu/aat/300000490> ;
  rdfs:subClassOf <https://w3id.org/con-tax/zones/aat-buildingSites#300000202> ;
.
<https://w3id.org/con-tax/zones/aat-buildingSites#300000491>
  rdf:type owl:Class ;
  rdfs:comment "Areas of land or property where many office buildings may be grouped together and developed specifically to attract corporate offices."@en ;
  rdfs:isDefinedBy <https://w3id.org/con-tax/zones/aat-buildingSites> ;
  rdfs:label "kantoorpark"@nl ;
  rdfs:label "kantoorparken"@nl ;
  rdfs:label "office parks"@en ;
  rdfs:seeAlso <http://vocab.getty.edu/aat/300000491> ;
  rdfs:seeAlso wd:Q338313 ;
  rdfs:subClassOf <https://w3id.org/con-tax/zones/aat-buildingSites#300000490> ;
.
<https://w3id.org/con-tax/zones/aat-buildingSites#300000498>
  rdf:type owl:Class ;
  rdfs:comment "Commercially developed real estate tracts commonly consisting of one- to four-unit dwellings."@en ;
  rdfs:comment "Wordt gebruikt voor commerciëel ontwikkelde onroerend-goedgebieden die meestal bestaan uit één- tot vier-kamer woningen."@nl ;
  rdfs:isDefinedBy <https://w3id.org/con-tax/zones/aat-buildingSites> ;
  rdfs:label "housing developments"@en ;
  rdfs:label "nieuwbouwproject"@nl ;
  rdfs:label "nieuwbouwprojecten"@nl ;
  rdfs:seeAlso <http://vocab.getty.edu/aat/300000498> ;
  rdfs:seeAlso wd:Q5916199 ;
  rdfs:subClassOf <https://w3id.org/con-tax/zones/aat-buildingSites#300259362> ;
.
<https://w3id.org/con-tax/zones/aat-buildingSites#300000500>
  rdf:type owl:Class ;
  rdfs:comment "Relatively large-scale real estate projects incorporating several revenue-producing functions, having a highly intensive use of land, and developed from a coherent plan."@en ;
  rdfs:comment "Wordt gebruikt voor vrij grootschalige nieuwbouwprojecten met verschillende inkomsten genererende activiteiten, met een hoogst intensieve gebruikmaking van grond en gebouwd volgens een duidelijk omlijnd plan."@nl ;
  rdfs:isDefinedBy <https://w3id.org/con-tax/zones/aat-buildingSites> ;
  rdfs:label "gemengd nieuwbouwproject"@nl ;
  rdfs:label "gemengde nieuwbouwprojecten"@nl ;
  rdfs:label "mixed-use developments"@en ;
  rdfs:seeAlso <http://vocab.getty.edu/aat/300000500> ;
  rdfs:seeAlso wd:Q4298922 ;
  rdfs:subClassOf <https://w3id.org/con-tax/zones/aat-buildingSites#300000202> ;
.
<https://w3id.org/con-tax/zones/aat-buildingSites#300000506>
  rdf:type owl:Class ;
  rdfs:comment "Aanduiding voor groepen van vooral commerciële ondernemingen, meestal een combinatie van onder andere fast-food restaurants, motels en benzinestations, die direct aan drukke wegen liggen vanwaar ze zeer goed zijn te bereiken; ontworpen om de aandacht van de automobilisten te trekken."@nl ;
  rdfs:comment "Designates groups of mostly commercial enterprises, usually a mix of fast-food restaurants, motels, and service stations, among others, arranged directly alongside well-traveled roads, providing nearly unlimited roadway access, and designed to attract the attention of motorists."@en ;
  rdfs:isDefinedBy <https://w3id.org/con-tax/zones/aat-buildingSites> ;
  rdfs:label "commercial strips"@en ;
  rdfs:label "commerciële zones"@nl ;
  rdfs:seeAlso <http://vocab.getty.edu/aat/300000506> ;
  rdfs:subClassOf <https://w3id.org/con-tax/zones/aat-buildingSites#300000202> ;
.
<https://w3id.org/con-tax/zones/aat-buildingSites#300000508>
  rdf:type owl:Class ;
  rdfs:comment "Areas of land divided into blocks or lots, provided with streets or roads and open spaces, and then offered for sale or lease."@en ;
  rdfs:comment "Stukken land die zijn verdeeld in kavels of percelen, voorzien van straten of wegen en open ruimten, en die vervolgens te koop of te huur worden aangeboden."@nl ;
  rdfs:isDefinedBy <https://w3id.org/con-tax/zones/aat-buildingSites> ;
  rdfs:label "subdivisions (complexes )"@en ;
  rdfs:label "verkaveling"@nl ;
  rdfs:label "verkavelingen"@nl ;
  rdfs:seeAlso <http://vocab.getty.edu/aat/300000508> ;
  rdfs:subClassOf <https://w3id.org/con-tax/zones/aat-buildingSites#300000202> ;
.
<https://w3id.org/con-tax/zones/aat-buildingSites#300000510>
  rdf:type owl:Class ;
  rdfs:comment "Land and water spaces and associated structures set aside for recreation."@en ;
  rdfs:comment "Land- en watergebieden en de daarmee verbonden bouwwerken die zijn bedoeld voor recreatie."@nl ;
  rdfs:isDefinedBy <https://w3id.org/con-tax/zones/aat-buildingSites> ;
  rdfs:label "recreatiegebied"@nl ;
  rdfs:label "recreatiegebieden"@nl ;
  rdfs:label "recreation areas"@en ;
  rdfs:seeAlso <http://vocab.getty.edu/aat/300000510> ;
  rdfs:seeAlso wd:Q2063507 ;
  rdfs:seeAlso wd:Q338112 ;
  rdfs:subClassOf <https://w3id.org/con-tax/zones/aat-buildingSites#300000202> ;
.
<https://w3id.org/con-tax/zones/aat-buildingSites#300000512>
  rdf:type owl:Class ;
  rdfs:comment "Commercially operated areas containing rides, stalls, and shows, and other entertainment attractions intended to attract a large number of visitors. "@en ;
  rdfs:isDefinedBy <https://w3id.org/con-tax/zones/aat-buildingSites> ;
  rdfs:label "amusement parks"@en ;
  rdfs:label "pretpark"@nl ;
  rdfs:label "pretparken"@nl ;
  rdfs:seeAlso <http://vocab.getty.edu/aat/300000512> ;
  rdfs:seeAlso wd:Q194195 ;
  rdfs:subClassOf <https://w3id.org/con-tax/zones/aat-buildingSites#300000510> ;
.
<https://w3id.org/con-tax/zones/aat-buildingSites#300000515>
  rdf:type owl:Class ;
  rdfs:comment "Amusement parks organized round a unifying idea or group of ideas, for example, Medieval castles or science fiction."@en ;
  rdfs:isDefinedBy <https://w3id.org/con-tax/zones/aat-buildingSites> ;
  rdfs:label "themapark"@nl ;
  rdfs:label "themaparken"@nl ;
  rdfs:label "theme parks"@en ;
  rdfs:seeAlso <http://vocab.getty.edu/aat/300000515> ;
  rdfs:seeAlso wd:Q2416723 ;
  rdfs:subClassOf <https://w3id.org/con-tax/zones/aat-buildingSites#300000512> ;
.
<https://w3id.org/con-tax/zones/aat-buildingSites#300000516>
  rdf:type owl:Class ;
  rdfs:comment "In the context of amusement parks, exhibitions, fairs, etc., the central avenues along which the chief exhibits or amusements are placed. In the context of amusement parks, exhibitions, fairs, etc., the central avenues along which the chief exhibits or amusements are placed."@en ;
  rdfs:isDefinedBy <https://w3id.org/con-tax/zones/aat-buildingSites> ;
  rdfs:label "amusementsruimte bij jaarmarkten en tentoonstellingen"@nl ;
  rdfs:label "amusementsruimten bij jaarmarkten en tentoonstellingen"@nl ;
  rdfs:label "midways"@en ;
  rdfs:seeAlso <http://vocab.getty.edu/aat/300000516> ;
  rdfs:subClassOf <https://w3id.org/con-tax/zones/aat-buildingSites#300000510> ;
.
<https://w3id.org/con-tax/zones/aat-buildingSites#300000517>
  rdf:type owl:Class ;
  rdfs:comment "Temporary short-term habitation complexes, with permanent recreational facilities and often offering a structured program of activities. Temporary short-term habitation complexes, with permanent recreational facilities and often offering a structured program of activities."@en ;
  rdfs:comment "Wordt gebruikt voor tijdelijke complexen met vaste recreatievoorzieningen voor bewoning van korte duur."@nl ;
  rdfs:isDefinedBy <https://w3id.org/con-tax/zones/aat-buildingSites> ;
  rdfs:label "camps (recreation areas)"@en ;
  rdfs:label "recreatieterrein"@nl ;
  rdfs:label "recreatieterreinen"@nl ;
  rdfs:seeAlso <http://vocab.getty.edu/aat/300000517> ;
  rdfs:seeAlso wd:Q832778 ;
  rdfs:subClassOf <https://w3id.org/con-tax/zones/aat-buildingSites#300000510> ;
.
<https://w3id.org/con-tax/zones/aat-buildingSites#300000521>
  rdf:type owl:Class ;
  rdfs:comment "Camps providing care and activities for children during daylight hours, usually including outdoor activities during warm seasons, but not including overnight housing."@en ;
  rdfs:isDefinedBy <https://w3id.org/con-tax/zones/aat-buildingSites> ;
  rdfs:label "day camps"@en ;
  rdfs:label "kinderkamp"@nl ;
  rdfs:label "kinderkampen"@nl ;
  rdfs:seeAlso <http://vocab.getty.edu/aat/300000521> ;
  rdfs:seeAlso wd:Q662423 ;
  rdfs:subClassOf <https://w3id.org/con-tax/zones/aat-buildingSites#300000517> ;
.
<https://w3id.org/con-tax/zones/aat-buildingSites#300000522>
  rdf:type owl:Class ;
  rdfs:comment "Permanent or temporary camps where inhabitants engage in indoor and outdoor recreational activites without the restriction of clothing."@en ;
  rdfs:comment "Wordt gebruikt voor tijdelijke of permanente kampen waar de deelnemers naakt meedoen aan binnen- en buitenactiviteiten."@nl ;
  rdfs:isDefinedBy <https://w3id.org/con-tax/zones/aat-buildingSites> ;
  rdfs:label "nudist camps"@en ;
  rdfs:label "nudistenkamp"@nl ;
  rdfs:label "nudistenkampen"@nl ;
  rdfs:seeAlso <http://vocab.getty.edu/aat/300000522> ;
  rdfs:seeAlso wd:Q2945522 ;
  rdfs:subClassOf <https://w3id.org/con-tax/zones/aat-buildingSites#300000517> ;
.
<https://w3id.org/con-tax/zones/aat-buildingSites#300000523>
  rdf:type owl:Class ;
  rdfs:comment "Seating, tents, buildings, or other facilities intended to accommodate religious camp meetings, particularly the type of outdoor revival meetings that were held on the American frontier during the 19th century by various Protestant denominations. Seating, tents, buildings, or other facilities intended to accommodate religious camp meetings, particularly the type of outdoor revival meetings that were held on the American frontier during the 19th century by various Protestant denominations."@en ;
  rdfs:isDefinedBy <https://w3id.org/con-tax/zones/aat-buildingSites> ;
  rdfs:label "religieus kamp"@nl ;
  rdfs:label "religieuze kampen"@nl ;
  rdfs:label "religious camps"@en ;
  rdfs:seeAlso <http://vocab.getty.edu/aat/300000523> ;
  rdfs:subClassOf <https://w3id.org/con-tax/zones/aat-buildingSites#300000517> ;
.
<https://w3id.org/con-tax/zones/aat-buildingSites#300000524>
  rdf:type owl:Class ;
  rdfs:comment "Camps run by a particular religious group and focusing on activities that promote the beliefs of the religion; church camps often cater to children, but may also include adults. The term is often distinguished from \"religious camps,\" which often refers specifically to 19th-century camps for revival meetings on the American frontier."@en ;
  rdfs:isDefinedBy <https://w3id.org/con-tax/zones/aat-buildingSites> ;
  rdfs:label "church camps"@en ;
  rdfs:label "kerkenkamp"@nl ;
  rdfs:label "kerkenkampen"@nl ;
  rdfs:seeAlso <http://vocab.getty.edu/aat/300000524> ;
  rdfs:subClassOf <https://w3id.org/con-tax/zones/aat-buildingSites#300000517> ;
.
<https://w3id.org/con-tax/zones/aat-buildingSites#300000525>
  rdf:type owl:Class ;
  rdfs:comment "Camps run by a particular school, and typically promoting or supplementing the educational program of the school; typical school camps are outdoors and designed for children. Camps run by a particular school, and typically promoting or supplementing the educational program of the school; typical school camps are outdoors and designed for children."@en ;
  rdfs:isDefinedBy <https://w3id.org/con-tax/zones/aat-buildingSites> ;
  rdfs:label "school camps"@en ;
  rdfs:label "schoolkamp"@nl ;
  rdfs:label "schoolkampen"@nl ;
  rdfs:seeAlso <http://vocab.getty.edu/aat/300000525> ;
  rdfs:subClassOf <https://w3id.org/con-tax/zones/aat-buildingSites#300000517> ;
.
<https://w3id.org/con-tax/zones/aat-buildingSites#300000532>
  rdf:type owl:Class ;
  rdfs:comment "Camps providing recreational and sporting facilities during the summer holiday period, usually intended for children and often including overnight accommodations."@en ;
  rdfs:isDefinedBy <https://w3id.org/con-tax/zones/aat-buildingSites> ;
  rdfs:label "summer camps"@en ;
  rdfs:label "zomerkamp"@nl ;
  rdfs:label "zomerkampen"@nl ;
  rdfs:seeAlso <http://vocab.getty.edu/aat/300000532> ;
  rdfs:seeAlso wd:Q876852 ;
  rdfs:subClassOf <https://w3id.org/con-tax/zones/aat-buildingSites#300000517> ;
.
<https://w3id.org/con-tax/zones/aat-buildingSites#300000534>
  rdf:type owl:Class ;
  rdfs:comment "Distinguished from \"mobile home parks\" by being only for the temporary parking of travel trailers, camping trailers, motor homes, or the like, for recreational purposes."@en ;
  rdfs:comment "Te onderscheiden van 'stacaravanterreinen' doordat ze alleen worden gebruikt als tijdelijke staplaats voor caravans, vouwcaravans, campers en dergelijke voor recreatie doeleinden."@nl ;
  rdfs:isDefinedBy <https://w3id.org/con-tax/zones/aat-buildingSites> ;
  rdfs:label "caravanterrein"@nl ;
  rdfs:label "caravanterreinen"@nl ;
  rdfs:label "trailer camps"@en ;
  rdfs:seeAlso <http://vocab.getty.edu/aat/300000534> ;
  rdfs:subClassOf <https://w3id.org/con-tax/zones/aat-buildingSites#300000517> ;
.
<https://w3id.org/con-tax/zones/aat-buildingSites#300000541>
  rdf:type owl:Class ;
  rdfs:comment "Facilities for the congregation of the team and other members of a polo club, which is an association involved with the equestrian team sport of polo. Facilities for the congregation of the team and other members of a polo club, which is an association involved with the equestrian team sport of polo."@en ;
  rdfs:isDefinedBy <https://w3id.org/con-tax/zones/aat-buildingSites> ;
  rdfs:label "polo clubs (built complexes)"@en ;
  rdfs:label "poloclub"@nl ;
  rdfs:label "poloclubs"@nl ;
  rdfs:seeAlso <http://vocab.getty.edu/aat/300000541> ;
  rdfs:subClassOf <https://w3id.org/con-tax/zones/aat-buildingSites#300203159> ;
.
<https://w3id.org/con-tax/zones/aat-buildingSites#300000544>
  rdf:type owl:Class ;
  rdfs:comment "Seaside, lakeshore, or riverside facilities for the congregation of members of a yacht club, which is a group of people involved with the sport of sailing and yachting. Yacht clubs typically include a marina, a delimited section of the beach, safe offshore anchorages, and buildings for the meeting and refreshment of the members. Seaside, lakeshore, or riverside facilities for the congregation of members of a yacht club, which is a group of people involved with the sport of sailing and yachting. Yacht clubs typically include a marina, a delimited section of the beach, safe offshore anchorages, and buildings for the meeting and refreshment of the members."@en ;
  rdfs:isDefinedBy <https://w3id.org/con-tax/zones/aat-buildingSites> ;
  rdfs:label "jachtclub"@nl ;
  rdfs:label "jachtclubs"@nl ;
  rdfs:label "yacht clubs (buliding complexes)"@en ;
  rdfs:label "zeilvereniging"@nl ;
  rdfs:label "zeilverenigingen"@nl ;
  rdfs:seeAlso <http://vocab.getty.edu/aat/300000544> ;
  rdfs:seeAlso wd:Q1855011 ;
  rdfs:subClassOf <https://w3id.org/con-tax/zones/aat-buildingSites#300007205> ;
.
<https://w3id.org/con-tax/zones/aat-buildingSites#300000545>
  rdf:type owl:Class ;
  rdfs:comment "Clubs, including the premises and grounds, that are located in or near the countryside rather than in an urban environment, and that are typically characterized by having a restricted membership and facilities for recreation and social intercourse."@en ;
  rdfs:isDefinedBy <https://w3id.org/con-tax/zones/aat-buildingSites> ;
  rdfs:label "buitensociëteit"@nl ;
  rdfs:label "buitensociëteiten"@nl ;
  rdfs:label "country clubs"@en ;
  rdfs:seeAlso <http://vocab.getty.edu/aat/300000545> ;
  rdfs:seeAlso wd:Q1137210 ;
  rdfs:subClassOf <https://w3id.org/con-tax/zones/aat-buildingSites#300203159> ;
.
<https://w3id.org/con-tax/zones/aat-buildingSites#300000547>
  rdf:type owl:Class ;
  rdfs:comment "Buildings and other facilities located in a  scenic, sporting, or other desirable area, and providing lodgings, entertainment, and other amenities for vacationers."@en ;
  rdfs:isDefinedBy <https://w3id.org/con-tax/zones/aat-buildingSites> ;
  rdfs:label "resorts"@en ;
  rdfs:label "vakantieoord"@nl ;
  rdfs:label "vakantieoorden"@nl ;
  rdfs:seeAlso <http://vocab.getty.edu/aat/300000547> ;
  rdfs:seeAlso wd:Q875157 ;
  rdfs:subClassOf <https://w3id.org/con-tax/zones/aat-buildingSites#300000510> ;
.
<https://w3id.org/con-tax/zones/aat-buildingSites#300000550>
  rdf:type owl:Class ;
  rdfs:comment "Resorts located on the seaside or beach."@en ;
  rdfs:isDefinedBy <https://w3id.org/con-tax/zones/aat-buildingSites> ;
  rdfs:label "badplaats"@nl ;
  rdfs:label "badplaatsen"@nl ;
  rdfs:label "seaside resorts"@en ;
  rdfs:seeAlso <http://vocab.getty.edu/aat/300000550> ;
  rdfs:seeAlso wd:Q1021711 ;
  rdfs:subClassOf <https://w3id.org/con-tax/zones/aat-buildingSites#300000547> ;
.
<https://w3id.org/con-tax/zones/aat-buildingSites#300000553>
  rdf:type owl:Class ;
  rdfs:comment "Resorts specializing in maintaining or improving the health or rejuvination of its clients, often including dietary and exercise instruction, bathing in mineral waters, breathing of fresh air, and formerly, extended exposure to sunshine (which was formerly considered healthy). Resorts specializing in maintaining or improving the health or rejuvination of its clients, often including dietary and exercise instruction, bathing in mineral waters, breathing of fresh air, and formerly, extended exposure to sunshine (which was formerly considered healthy)."@en ;
  rdfs:isDefinedBy <https://w3id.org/con-tax/zones/aat-buildingSites> ;
  rdfs:label "health resorts"@en ;
  rdfs:label "kuuroord"@nl ;
  rdfs:label "kuuroorden"@nl ;
  rdfs:seeAlso <http://vocab.getty.edu/aat/300000553> ;
  rdfs:subClassOf <https://w3id.org/con-tax/zones/aat-buildingSites#300000547> ;
.
<https://w3id.org/con-tax/zones/aat-buildingSites#300000557>
  rdf:type owl:Class ;
  rdfs:comment "Areas of land or water set apart for the protection of natural landscapes or wildlife, or for the rearing of game or fish; in some preserves, limited hunting is permitted."@en ;
  rdfs:comment "Gebieden, beperkt toegankelijk voor bezoekers, die afgeschermd worden om de voortplanting van dieren of vissen te bevorderen en waar beperkte jacht is toegestaan."@nl ;
  rdfs:isDefinedBy <https://w3id.org/con-tax/zones/aat-buildingSites> ;
  rdfs:label "preserves"@en ;
  rdfs:label "reservaat"@nl ;
  rdfs:label "reservaten"@nl ;
  rdfs:seeAlso <http://vocab.getty.edu/aat/300000557> ;
  rdfs:seeAlso wd:Q179049 ;
  rdfs:subClassOf <https://w3id.org/con-tax/zones/aat-buildingSites#300000510> ;
.
<https://w3id.org/con-tax/zones/aat-buildingSites#300000558>
  rdf:type owl:Class ;
  rdfs:comment "Resorts that operate seasonally during the summer months."@en ;
  rdfs:isDefinedBy <https://w3id.org/con-tax/zones/aat-buildingSites> ;
  rdfs:label "summer resorts"@en ;
  rdfs:label "zomervakantieoord"@nl ;
  rdfs:label "zomervakantieoorden"@nl ;
  rdfs:seeAlso <http://vocab.getty.edu/aat/300000558> ;
  rdfs:subClassOf <https://w3id.org/con-tax/zones/aat-buildingSites#300000547> ;
.
<https://w3id.org/con-tax/zones/aat-buildingSites#300000559>
  rdf:type owl:Class ;
  rdfs:comment "Facilities usually located on a mountain or large hill and designed for winter sports, typically skiing, snow boarding, and other such activities."@en ;
  rdfs:isDefinedBy <https://w3id.org/con-tax/zones/aat-buildingSites> ;
  rdfs:label "winter resorts"@en ;
  rdfs:label "wintersportcentra"@nl ;
  rdfs:label "wintersportcentrum"@nl ;
  rdfs:seeAlso <http://vocab.getty.edu/aat/300000559> ;
  rdfs:subClassOf <https://w3id.org/con-tax/zones/aat-buildingSites#300000547> ;
.
<https://w3id.org/con-tax/zones/aat-buildingSites#300000560>
  rdf:type owl:Class ;
  rdfs:comment "Building complexes and associated grounds that are designed for playing sports and the accommodation of large crowds of viewers, including seating or other viewing areas, dining facilities, tracks, pools, or various other playing areas. For inhabited places having sports as a focus, use \"sporting centers (inhabited places).\""@en ;
  rdfs:isDefinedBy <https://w3id.org/con-tax/zones/aat-buildingSites> ;
  rdfs:label "sportcomplexen"@nl ;
  rdfs:label "sports complexes"@en ;
  rdfs:label "sportsportcomplex"@nl ;
  rdfs:seeAlso <http://vocab.getty.edu/aat/300000560> ;
  rdfs:seeAlso wd:Q7579839 ;
  rdfs:subClassOf <https://w3id.org/con-tax/zones/aat-buildingSites#300000510> ;
.
<https://w3id.org/con-tax/zones/aat-buildingSites#300000591>
  rdf:type owl:Class ;
  rdfs:comment "Areas containing an assortment of obstacles to be negotiated, used for sporting events, military training, or animal competitions. Obstacle courses typically include a series of challenging physical obstacles that an individual, team, or animal (often a horse or dog) must navigate while being timed. Obstacles may include water ditches, open ditches, walls, fences, hurdles, and other hazards encountered while the participant is running, jumping, crawling, climbing, or balancing, with the goal of winning a contest, testing endurance or tactical skills, physical training, team building, or problem solving. Runners of the standard obstacle course as a sporting event must negotiate seven water jumps and 28 hurdle jumps."@en ;
  rdfs:isDefinedBy <https://w3id.org/con-tax/zones/aat-buildingSites> ;
  rdfs:label "hindernisbaan"@nl ;
  rdfs:label "hindernisbanen"@nl ;
  rdfs:label "obstacle courses"@en ;
  rdfs:seeAlso <http://vocab.getty.edu/aat/300000591> ;
  rdfs:seeAlso wd:Q933851 ;
  rdfs:subClassOf <https://w3id.org/con-tax/zones/aat-buildingSites#300000560> ;
.
<https://w3id.org/con-tax/zones/aat-buildingSites#300000592>
  rdf:type owl:Class ;
  rdfs:comment "Dorpen of gebouwencomplexen waar de olympische deelnemers verblijven."@nl ;
  rdfs:comment "Self-contained districts within or near a city that is hosting the Olympics sporting events, providing accommodation and amenities for competitors and other people who have an official connection with the Olympic games. Self-contained districts within or near a city that is hosting the Olympics sporting events, providing accommodation and amenities for competitors and other people who have an official connection with the Olympic games."@en ;
  rdfs:isDefinedBy <https://w3id.org/con-tax/zones/aat-buildingSites> ;
  rdfs:label "Olympic villages"@en ;
  rdfs:label "olympisch dorp"@nl ;
  rdfs:label "olympische dorpen"@nl ;
  rdfs:seeAlso <http://vocab.getty.edu/aat/300000592> ;
  rdfs:seeAlso wd:Q866623 ;
  rdfs:subClassOf <https://w3id.org/con-tax/zones/aat-buildingSites#300259362> ;
.
<https://w3id.org/con-tax/zones/aat-buildingSites#300000593>
  rdf:type owl:Class ;
  rdfs:comment "Typically oval courses or tracks on which races of any kind are held, including foot races, bicycle races, horse or dog races, and automobile races. Typically oval courses or tracks on which races of any kind are held, including foot races, bicycle races, horse or dog races, and automobile races."@en ;
  rdfs:isDefinedBy <https://w3id.org/con-tax/zones/aat-buildingSites> ;
  rdfs:label "racetracks (complexes)"@en ;
  rdfs:label "renbaan"@nl ;
  rdfs:label "renbanen"@nl ;
  rdfs:seeAlso <http://vocab.getty.edu/aat/300000593> ;
  rdfs:seeAlso wd:Q1777138 ;
  rdfs:subClassOf <https://w3id.org/con-tax/zones/aat-buildingSites#300000560> ;
.
<https://w3id.org/con-tax/zones/aat-buildingSites#300000597>
  rdf:type owl:Class ;
  rdfs:comment "Tracks, usually oval in shape, designed or used primarily for the racing of automobiles; surfaces may be made of dirt, asphalt, brick, or another material."@en ;
  rdfs:isDefinedBy <https://w3id.org/con-tax/zones/aat-buildingSites> ;
  rdfs:label "automobile racetracks"@en ;
  rdfs:label "racecircuit"@nl ;
  rdfs:label "racecircuits"@nl ;
  rdfs:seeAlso <http://vocab.getty.edu/aat/300000597> ;
  rdfs:subClassOf <https://w3id.org/con-tax/zones/aat-buildingSites#300000593> ;
.
<https://w3id.org/con-tax/zones/aat-buildingSites#300000599>
  rdf:type owl:Class ;
  rdfs:comment "Tracks or strips of road, dry lake beds, or another flat surface used for drag racing, which is an automobile race over a flat, straight course, most commonly 1/4 mile in length.  Drag racing as an organized sport began in the 1930s on dry lake beds in southern California. Tracks or strips of road, dry lake beds, or another flat surface used for drag racing, which is an automobile race over a flat, straight course, most commonly 1/4 mile in length.  Drag racing as an organized sport began in the 1930s on dry lake beds in southern California."@en ;
  rdfs:isDefinedBy <https://w3id.org/con-tax/zones/aat-buildingSites> ;
  rdfs:label "drag strips"@en ;
  rdfs:label "dragracebaan"@nl ;
  rdfs:label "dragracebanen"@nl ;
  rdfs:seeAlso <http://vocab.getty.edu/aat/300000599> ;
  rdfs:seeAlso wd:Q357121 ;
  rdfs:subClassOf <https://w3id.org/con-tax/zones/aat-buildingSites#300000597> ;
.
<https://w3id.org/con-tax/zones/aat-buildingSites#300000600>
  rdf:type owl:Class ;
  rdfs:comment "Arenas designed or used for bicycle racing; modern velodromes comprise a steeply banked oval track having two 180-degree circular bends connected by two straight passages."@en ;
  rdfs:isDefinedBy <https://w3id.org/con-tax/zones/aat-buildingSites> ;
  rdfs:label "velodromes"@en ;
  rdfs:label "velodrooms"@nl ;
  rdfs:label "wielerbaan"@nl ;
  rdfs:label "wielerbanen"@nl ;
  rdfs:seeAlso <http://vocab.getty.edu/aat/300000600> ;
  rdfs:seeAlso wd:Q830528 ;
  rdfs:subClassOf <https://w3id.org/con-tax/zones/aat-buildingSites#300000593> ;
.
<https://w3id.org/con-tax/zones/aat-buildingSites#300000604>
  rdf:type owl:Class ;
  rdfs:comment "Tracks designed or primarily used for the racing of greyhounds or other dogs. Tracks designed or primarily used for the racing of greyhounds or other dogs."@en ;
  rdfs:isDefinedBy <https://w3id.org/con-tax/zones/aat-buildingSites> ;
  rdfs:label "dog tracks"@en ;
  rdfs:label "hondenrenbaan"@nl ;
  rdfs:label "hondenrenbanen"@nl ;
  rdfs:seeAlso <http://vocab.getty.edu/aat/300000604> ;
  rdfs:seeAlso wd:Q778020 ;
  rdfs:subClassOf <https://w3id.org/con-tax/zones/aat-buildingSites#300000593> ;
.
<https://w3id.org/con-tax/zones/aat-buildingSites#300000608>
  rdf:type owl:Class ;
  rdfs:comment "Racetracks designed or used for horse racing. For ancient Greek or Roman oblong structures designed for horse and chariot racing, use \"hippodromes (Greek sports buildings)\" or \"circuses (Roman arenas)\" respectively. Racetracks designed or used for horse racing. For ancient Greek or Roman oblong structures designed for horse and chariot racing, use \"hippodromes (Greek sports buildings)\" or \"circuses (Roman arenas)\" respectively."@en ;
  rdfs:comment "Renbanen die zijn ontworpen of gebruikt worden voor paardenraces.  Gebruik de term 'hippodromen' en 'circussen (renbanen)' voor respectievelijk Griekse en Romeinse ellipsvormige bouwwerken bedoeld voor races met paard en wagen."@nl ;
  rdfs:isDefinedBy <https://w3id.org/con-tax/zones/aat-buildingSites> ;
  rdfs:label "horse racetracks"@en ;
  rdfs:label "paardenrenbaan"@nl ;
  rdfs:label "paardenrenbanen"@nl ;
  rdfs:seeAlso <http://vocab.getty.edu/aat/300000608> ;
  rdfs:subClassOf <https://w3id.org/con-tax/zones/aat-buildingSites#300000593> ;
.
<https://w3id.org/con-tax/zones/aat-buildingSites#300000612>
  rdf:type owl:Class ;
  rdfs:comment "Areas designed or used primarily for the sport of skateboarding, including straight tracks as well as a variety of slopes and banked surfaces for sudden turns and stunts. Areas designed or used primarily for the sport of skateboarding, including straight tracks as well as a variety of slopes and banked surfaces for sudden turns and stunts."@en ;
  rdfs:isDefinedBy <https://w3id.org/con-tax/zones/aat-buildingSites> ;
  rdfs:label "skateboarding parks"@en ;
  rdfs:label "skateboardterrein"@nl ;
  rdfs:label "skateboardterreinen"@nl ;
  rdfs:seeAlso <http://vocab.getty.edu/aat/300000612> ;
  rdfs:seeAlso wd:Q909906 ;
  rdfs:subClassOf <https://w3id.org/con-tax/zones/aat-buildingSites#300000560> ;
.
<https://w3id.org/con-tax/zones/aat-buildingSites#300000617>
  rdf:type owl:Class ;
  rdfs:comment "Areas equipped with targets for practice in shooting weapons; when possible use a more specific term."@en ;
  rdfs:comment "Terreinen uitgerust met doelen voor oefening in het schieten met vuurwapens."@nl ;
  rdfs:isDefinedBy <https://w3id.org/con-tax/zones/aat-buildingSites> ;
  rdfs:label "ranges (complexes)"@en ;
  rdfs:label "schietterrein"@nl ;
  rdfs:label "schietterreinen"@nl ;
  rdfs:seeAlso <http://vocab.getty.edu/aat/300000617> ;
  rdfs:subClassOf <https://w3id.org/con-tax/zones/aat-buildingSites#300000202> ;
.
<https://w3id.org/con-tax/zones/aat-buildingSites#300000618>
  rdf:type owl:Class ;
  rdfs:comment "Areas designed or used primarily the sport of archery, which consists of shooting with bow and arrow at targets."@en ;
  rdfs:isDefinedBy <https://w3id.org/con-tax/zones/aat-buildingSites> ;
  rdfs:label "archery ranges"@en ;
  rdfs:label "boogschietterrein"@nl ;
  rdfs:label "boogschietterreinen"@nl ;
  rdfs:seeAlso <http://vocab.getty.edu/aat/300000618> ;
  rdfs:subClassOf <https://w3id.org/con-tax/zones/aat-buildingSites#300000619> ;
.
<https://w3id.org/con-tax/zones/aat-buildingSites#300000619>
  rdf:type owl:Class ;
  rdfs:comment "Areas or facilities designed or used primarily for shooting guns at targets, whether for sport or as training. Typically the area includes various ranges or distances marked off between the respective firing points and the targets."@en ;
  rdfs:comment "Terreinen, ingericht voor het schieten naar een doel, naar schietschijven."@nl ;
  rdfs:isDefinedBy <https://w3id.org/con-tax/zones/aat-buildingSites> ;
  rdfs:label "schietbaan"@nl ;
  rdfs:label "schietbanen"@nl ;
  rdfs:label "schuttersdoel"@nl ;
  rdfs:label "schuttersdoelen"@nl ;
  rdfs:label "shooting ranges"@en ;
  rdfs:seeAlso <http://vocab.getty.edu/aat/300000619> ;
  rdfs:seeAlso wd:Q521839 ;
  rdfs:subClassOf <https://w3id.org/con-tax/zones/aat-buildingSites#300000617> ;
.
<https://w3id.org/con-tax/zones/aat-buildingSites#300000620>
  rdf:type owl:Class ;
  rdfs:comment "Areas designed or used primarily for the shooting of rifles at targets."@en ;
  rdfs:isDefinedBy <https://w3id.org/con-tax/zones/aat-buildingSites> ;
  rdfs:label "exercitieveld"@nl ;
  rdfs:label "exercitievelden"@nl ;
  rdfs:label "rifle ranges"@en ;
  rdfs:seeAlso <http://vocab.getty.edu/aat/300000620> ;
  rdfs:seeAlso wd:Q7333260 ;
  rdfs:subClassOf <https://w3id.org/con-tax/zones/aat-buildingSites#300000619> ;
.
<https://w3id.org/con-tax/zones/aat-buildingSites#300000621>
  rdf:type owl:Class ;
  rdfs:comment "Semicircular range designed or used primarily for the shooting of skeets, a sport involving clay-pigeon targets projected at a variety of shooting angles. Semicircular range designed or used primarily for the shooting of skeets, a sport involving clay-pigeon targets projected at a variety of shooting angles."@en ;
  rdfs:isDefinedBy <https://w3id.org/con-tax/zones/aat-buildingSites> ;
  rdfs:label "kleiduivenbaan"@nl ;
  rdfs:label "kleiduivenbanen"@nl ;
  rdfs:label "skeet ranges"@en ;
  rdfs:seeAlso <http://vocab.getty.edu/aat/300000621> ;
  rdfs:subClassOf <https://w3id.org/con-tax/zones/aat-buildingSites#300000619> ;
.
<https://w3id.org/con-tax/zones/aat-buildingSites#300000625>
  rdf:type owl:Class ;
  rdfs:comment "Trails or slopes prepared for skiing, particularly trails through the landscape or trees, as distinguished from ski runs that are always downhill, and usually marked, patrolled, and graded according to difficulty."@en ;
  rdfs:isDefinedBy <https://w3id.org/con-tax/zones/aat-buildingSites> ;
  rdfs:label "langlauftrajecten"@nl ;
  rdfs:label "loipe"@nl ;
  rdfs:label "loipes"@nl ;
  rdfs:label "ski trails"@en ;
  rdfs:seeAlso <http://vocab.getty.edu/aat/300000625> ;
  rdfs:subClassOf <https://w3id.org/con-tax/zones/aat-buildingSites#300000626> ;
.
<https://w3id.org/con-tax/zones/aat-buildingSites#300000626>
  rdf:type owl:Class ;
  rdfs:comment "Various types of paths or tracks worn by the passage of persons or animals travelling in a wilderness area, or deliberately maintained for passage through various outdoor environments."@en ;
  rdfs:isDefinedBy <https://w3id.org/con-tax/zones/aat-buildingSites> ;
  rdfs:label "omloop"@nl ;
  rdfs:label "parcoursen"@nl ;
  rdfs:label "recreatieroute"@nl ;
  rdfs:label "recreatieroutes"@nl ;
  rdfs:label "trails (recreation areas)"@en ;
  rdfs:seeAlso <http://vocab.getty.edu/aat/300000626> ;
  rdfs:subClassOf <https://w3id.org/con-tax/zones/aat-buildingSites#300000510> ;
.
<https://w3id.org/con-tax/zones/aat-buildingSites#300000627>
  rdf:type owl:Class ;
  rdfs:comment "Organized and labeled trails laid out to follow points of interest concerning the local history of a region."@en ;
  rdfs:comment "Wordt gebruikt voor uitgezette en aangegeven routes langs cultuurhistorisch interessante plaatsen."@nl ;
  rdfs:isDefinedBy <https://w3id.org/con-tax/zones/aat-buildingSites> ;
  rdfs:label "cultuurhistorische route"@nl ;
  rdfs:label "cultuurhistorische routes"@nl ;
  rdfs:label "heritage trails"@en ;
  rdfs:seeAlso <http://vocab.getty.edu/aat/300000627> ;
  rdfs:subClassOf <https://w3id.org/con-tax/zones/aat-buildingSites#300000626> ;
.
<https://w3id.org/con-tax/zones/aat-buildingSites#300000630>
  rdf:type owl:Class ;
  rdfs:comment "Footpaths through nature reserves or other area of countryside for the observation of plants, animals, and natural phenomena, frequently marked by posted signs and discussed in associated descriptive literature."@en ;
  rdfs:isDefinedBy <https://w3id.org/con-tax/zones/aat-buildingSites> ;
  rdfs:label "nature trails"@en ;
  rdfs:label "natuurpad"@nl ;
  rdfs:label "natuurpaden"@nl ;
  rdfs:seeAlso <http://vocab.getty.edu/aat/300000630> ;
  rdfs:subClassOf <https://w3id.org/con-tax/zones/aat-buildingSites#300000626> ;
.
<https://w3id.org/con-tax/zones/aat-buildingSites#300000632>
  rdf:type owl:Class ;
  rdfs:comment "Facilities for groups of people living together or near each other, and subscribing to the tenets of a particular religion, including those who have taken vows and belong to the structure of a particular order, as well as more loosely organized groups of people. For the religious officials or functionaries of a religion, use \"clergy.\" For the formal, organized groups themselves, use \"religious orders.\""@en ;
  rdfs:isDefinedBy <https://w3id.org/con-tax/zones/aat-buildingSites> ;
  rdfs:label "religieus gemeenschapscomplex"@nl ;
  rdfs:label "religieuze gemeenschapscomplexen"@nl ;
  rdfs:label "religious communities (built complexes)"@en ;
  rdfs:seeAlso <http://vocab.getty.edu/aat/300000632> ;
  rdfs:subClassOf <https://w3id.org/con-tax/zones/aat-buildingSites#300263741> ;
.
<https://w3id.org/con-tax/zones/aat-buildingSites#300000634>
  rdf:type owl:Class ;
  rdfs:comment "Communal facilities established for the sisterhood of Béguines."@en ;
  rdfs:comment "Gemeenschappelijke ruimten voor de zusterorde der Begijnen."@nl ;
  rdfs:isDefinedBy <https://w3id.org/con-tax/zones/aat-buildingSites> ;
  rdfs:label "begijnhof"@nl ;
  rdfs:label "begijnhofje"@nl ;
  rdfs:label "begijnhofjes"@nl ;
  rdfs:label "begijnhoven"@nl ;
  rdfs:label "béguinages"@en ;
  rdfs:seeAlso <http://vocab.getty.edu/aat/300000634> ;
  rdfs:subClassOf <https://w3id.org/con-tax/zones/aat-buildingSites#300000632> ;
.
<https://w3id.org/con-tax/zones/aat-buildingSites#300000635>
  rdf:type owl:Class ;
  rdfs:comment "In common usage, the word \"convent\" is used for the facilities of a company of women living together in the discipline of a religious order and under one superior. For facilities for a company of males, use \"monasteries.\" "@en ;
  rdfs:isDefinedBy <https://w3id.org/con-tax/zones/aat-buildingSites> ;
  rdfs:label "convents (built complexes)"@en ;
  rdfs:label "nonnenklooster"@nl ;
  rdfs:label "nonnenkloosters"@nl ;
  rdfs:seeAlso <http://vocab.getty.edu/aat/300000635> ;
  rdfs:subClassOf <https://w3id.org/con-tax/zones/aat-buildingSites#300000632> ;
.
<https://w3id.org/con-tax/zones/aat-buildingSites#300000640>
  rdf:type owl:Class ;
  rdfs:comment "Dwelling places of solitary hermits or of groups of religious in a relatively secluded setting."@en ;
  rdfs:isDefinedBy <https://w3id.org/con-tax/zones/aat-buildingSites> ;
  rdfs:label "hermitages (religious communities)"@en ;
  rdfs:label "kluizenaarshut"@nl ;
  rdfs:label "kluizenaarshutten"@nl ;
  rdfs:seeAlso <http://vocab.getty.edu/aat/300000640> ;
  rdfs:seeAlso wd:Q513550 ;
  rdfs:subClassOf <https://w3id.org/con-tax/zones/aat-buildingSites#300000632> ;
.
<https://w3id.org/con-tax/zones/aat-buildingSites#300000641>
  rdf:type owl:Class ;
  rdfs:comment "Built complexes for religious retirement or seclusion from the world for monks, who are people living a celibate life according to the rule of a particular religious order and adhering to vows, especially of poverty, chastity, and obedience."@en ;
  rdfs:comment "Plaatsen van religieuze retraite of afzondering van de wereld voor mensen die religieuze geloften hebben afgelegd."@nl ;
  rdfs:isDefinedBy <https://w3id.org/con-tax/zones/aat-buildingSites> ;
  rdfs:label "convent"@nl ;
  rdfs:label "conventen"@nl ;
  rdfs:label "klooster"@nl ;
  rdfs:label "kloosters"@nl ;
  rdfs:label "monasteries (built complexes)"@en ;
  rdfs:seeAlso <http://vocab.getty.edu/aat/300000641> ;
  rdfs:subClassOf <https://w3id.org/con-tax/zones/aat-buildingSites#300000632> ;
.
<https://w3id.org/con-tax/zones/aat-buildingSites#300000642>
  rdf:type owl:Class ;
  rdfs:comment "Designates independent and canonically erected monasteries, ruled by an abbot if occupied by monks and by an abbess if occupied by nuns."@en ;
  rdfs:comment "Kloosters voor mannen of vrouwen, met respectievelijk een abt of abdis als hoofd."@nl ;
  rdfs:isDefinedBy <https://w3id.org/con-tax/zones/aat-buildingSites> ;
  rdfs:label "abbeys (monasteries)"@en ;
  rdfs:label "abdij"@nl ;
  rdfs:label "abdijen"@nl ;
  rdfs:seeAlso <http://vocab.getty.edu/aat/300000642> ;
  rdfs:subClassOf <https://w3id.org/con-tax/zones/aat-buildingSites#300000641> ;
.
<https://w3id.org/con-tax/zones/aat-buildingSites#300000643>
  rdf:type owl:Class ;
  rdfs:comment "Eertijds gehelen van twee kloosters, één voor mannen en één voor vrouwen."@nl ;
  rdfs:comment "Religious houses for communities of both men and women, dwelling in contiguous establishments, united under the rule of one superior."@en ;
  rdfs:isDefinedBy <https://w3id.org/con-tax/zones/aat-buildingSites> ;
  rdfs:label "double monasteries"@en ;
  rdfs:label "dubbelklooster"@nl ;
  rdfs:label "dubbelkloosters"@nl ;
  rdfs:seeAlso <http://vocab.getty.edu/aat/300000643> ;
  rdfs:seeAlso wd:Q1243067 ;
  rdfs:subClassOf <https://w3id.org/con-tax/zones/aat-buildingSites#300000641> ;
.
<https://w3id.org/con-tax/zones/aat-buildingSites#300000644>
  rdf:type owl:Class ;
  rdfs:comment "Buildings and other facilities for friars, a community of men who focus on the sacred ministry of preaching, moving from place to place (in contrast to monks)."@en ;
  rdfs:isDefinedBy <https://w3id.org/con-tax/zones/aat-buildingSites> ;
  rdfs:label "friaries"@en ;
  rdfs:label "monnikenklooster"@nl ;
  rdfs:label "monnikenkloosters"@nl ;
  rdfs:seeAlso <http://vocab.getty.edu/aat/300000644> ;
  rdfs:seeAlso wd:Q20672229 ;
  rdfs:subClassOf <https://w3id.org/con-tax/zones/aat-buildingSites#300000632> ;
.
<https://w3id.org/con-tax/zones/aat-buildingSites#300000645>
  rdf:type owl:Class ;
  rdfs:comment "Religieuze huizen die zich qua rang net onder kloosters staan en waar het gezag in handen is van een prior of een priores."@nl ;
  rdfs:comment "Religious houses that rank immediately below abbeys and are presided over by a prior or prioress."@en ;
  rdfs:isDefinedBy <https://w3id.org/con-tax/zones/aat-buildingSites> ;
  rdfs:label "priories"@en ;
  rdfs:label "priorij"@nl ;
  rdfs:label "priorijen"@nl ;
  rdfs:seeAlso <http://vocab.getty.edu/aat/300000645> ;
  rdfs:seeAlso wd:Q2750108 ;
  rdfs:subClassOf <https://w3id.org/con-tax/zones/aat-buildingSites#300000641> ;
.
<https://w3id.org/con-tax/zones/aat-buildingSites#300000650>
  rdf:type owl:Class ;
  rdfs:comment "Carthusian monasteries."@en ;
  rdfs:comment "Kloosters van Kartuizer monniken."@nl ;
  rdfs:isDefinedBy <https://w3id.org/con-tax/zones/aat-buildingSites> ;
  rdfs:label "charterhouses"@en ;
  rdfs:label "kartuizerklooster"@nl ;
  rdfs:label "kartuizerkloosters"@nl ;
  rdfs:seeAlso <http://vocab.getty.edu/aat/300000650> ;
  rdfs:seeAlso wd:Q44613 ;
  rdfs:subClassOf <https://w3id.org/con-tax/zones/aat-buildingSites#300000641> ;
.
<https://w3id.org/con-tax/zones/aat-buildingSites#300000660>
  rdf:type owl:Class ;
  rdfs:comment "Monastic complexes of the eastern Mediterranean in which hermit monks live in a loosely organized group of cells around a common central complex."@en ;
  rdfs:comment "Wordt gebruikt voor bepaalde kloostercomplexen in het oostelijke Middellandse Zee-gebied waar heremieten leven in een losjes gestructureerde groep cellen rond een gemeenschappelijk centraal complex."@nl ;
  rdfs:isDefinedBy <https://w3id.org/con-tax/zones/aat-buildingSites> ;
  rdfs:label "lavra"@nl ;
  rdfs:label "lavra's"@nl ;
  rdfs:label "lavras"@en ;
  rdfs:seeAlso <http://vocab.getty.edu/aat/300000660> ;
  rdfs:subClassOf <https://w3id.org/con-tax/zones/aat-buildingSites#300000632> ;
.
<https://w3id.org/con-tax/zones/aat-buildingSites#300000661>
  rdf:type owl:Class ;
  rdfs:comment "Kloosters in pre-islamitisch India."@nl ;
  rdfs:comment "Monasteries or convents in pre-Islamic India."@en ;
  rdfs:isDefinedBy <https://w3id.org/con-tax/zones/aat-buildingSites> ;
  rdfs:label "math"@nl ;
  rdfs:label "mathas"@en ;
  rdfs:label "maths"@nl ;
  rdfs:seeAlso <http://vocab.getty.edu/aat/300000661> ;
  rdfs:seeAlso wd:Q2069741 ;
  rdfs:subClassOf <https://w3id.org/con-tax/zones/aat-buildingSites#300000632> ;
  rdfs:subClassOf <https://w3id.org/con-tax/zones/aat-buildingSites#300000635> ;
  rdfs:subClassOf <https://w3id.org/con-tax/zones/aat-buildingSites#300000641> ;
.
<https://w3id.org/con-tax/zones/aat-buildingSites#300000663>
  rdf:type owl:Class ;
  rdfs:comment "Communities of Buddhist monks; may also be used for Jain religious communities."@en ;
  rdfs:comment "Wordt gebruikt voor gemeenschappen van boeddhistische monniken; kan ook gebruikt worden voor jainistische religieuze gemeenschappen."@nl ;
  rdfs:isDefinedBy <https://w3id.org/con-tax/zones/aat-buildingSites> ;
  rdfs:label "sangha"@nl ;
  rdfs:label "sangha's"@nl ;
  rdfs:label "sanghas"@en ;
  rdfs:seeAlso <http://vocab.getty.edu/aat/300000663> ;
  rdfs:subClassOf <https://w3id.org/con-tax/zones/aat-buildingSites#300000632> ;
.
<https://w3id.org/con-tax/zones/aat-buildingSites#300000665>
  rdf:type owl:Class ;
  rdfs:comment "Use only for dervish monasteries; for rest houses for Islamic pilgrims, use \"hospices.\""@en ;
  rdfs:comment "Wordt alleen gebruikt voor derwisj kloosters; gebruik 'hospitiën' voor pleisterplaatsen voor islamitische pelgrims."@nl ;
  rdfs:isDefinedBy <https://w3id.org/con-tax/zones/aat-buildingSites> ;
  rdfs:label "tekke"@nl ;
  rdfs:label "tekkes (monasteries)"@en ;
  rdfs:label "tekkes"@nl ;
  rdfs:seeAlso <http://vocab.getty.edu/aat/300000665> ;
  rdfs:seeAlso wd:Q833913 ;
  rdfs:subClassOf <https://w3id.org/con-tax/zones/aat-buildingSites#300000632> ;
.
<https://w3id.org/con-tax/zones/aat-buildingSites#300000666>
  rdf:type owl:Class ;
  rdfs:comment "Primarily refers to Indian Buddhist monasteries; may also be used for Sinhalese Buddhist temples."@en ;
  rdfs:comment "Wordt vooral gebruikt voor Indiaase boeddhistische kloosters; kan ook gebruikt worden voor boeddhistische tempels op Sri Lanka."@nl ;
  rdfs:isDefinedBy <https://w3id.org/con-tax/zones/aat-buildingSites> ;
  rdfs:label "vihara"@nl ;
  rdfs:label "vihara's"@nl ;
  rdfs:label "viharas (religious communities)"@en ;
  rdfs:seeAlso <http://vocab.getty.edu/aat/300000666> ;
  rdfs:subClassOf <https://w3id.org/con-tax/zones/aat-buildingSites#300000632> ;
.
<https://w3id.org/con-tax/zones/aat-buildingSites#300000667>
  rdf:type owl:Class ;
  rdfs:comment "Siamese Buddhist temples; may also be used for Siamese Buddhist monasteries."@en ;
  rdfs:comment "Thaise boeddhistische tempels; kan ook worden gebruikt voor Thaise boeddhistische kloosters."@nl ;
  rdfs:isDefinedBy <https://w3id.org/con-tax/zones/aat-buildingSites> ;
  rdfs:label "wats"@en ;
  rdfs:label "wats"@nl ;
  rdfs:seeAlso <http://vocab.getty.edu/aat/300000667> ;
  rdfs:subClassOf <https://w3id.org/con-tax/zones/aat-buildingSites#300000641> ;
.
<https://w3id.org/con-tax/zones/aat-buildingSites#300000672>
  rdf:type owl:Class ;
  rdfs:comment "Complexes where testing of weapons or vehicles is conducted under close-hand scrutiny; for locations where weapons are exploded at a distance from observers, use \"test sites.\""@en ;
  rdfs:comment "Wordt gebruikt voor complexen waar wapens en voertuigen worden getest onder scherp toezicht; gebruik 'proefterreinen' voor plaatsen waar wapens tot ontploffing worden gebracht op een afstand van de waarnemers."@nl ;
  rdfs:isDefinedBy <https://w3id.org/con-tax/zones/aat-buildingSites> ;
  rdfs:label "proving grounds"@en ;
  rdfs:label "testterrein"@nl ;
  rdfs:label "testterreinen"@nl ;
  rdfs:seeAlso <http://vocab.getty.edu/aat/300000672> ;
  rdfs:seeAlso wd:Q1778846 ;
  rdfs:subClassOf <https://w3id.org/con-tax/zones/aat-buildingSites#300000202> ;
.
<https://w3id.org/con-tax/zones/aat-buildingSites#300000676>
  rdf:type owl:Class ;
  rdfs:comment "Aanduiding voor gebieden waar een grote hoeveelheid opslagtanks met een grote capaciteit is geplaatst, meestal gebruikt voor ruwe olie of andere olieproducten."@nl ;
  rdfs:comment "Designates areas where a large number of high-capacity storage tanks are located, usually used for crude oil or other petroleum products."@en ;
  rdfs:isDefinedBy <https://w3id.org/con-tax/zones/aat-buildingSites> ;
  rdfs:label "opslagterrein van olietank"@nl ;
  rdfs:label "opslagterreinen van olietanks"@nl ;
  rdfs:label "tank farms"@en ;
  rdfs:seeAlso <http://vocab.getty.edu/aat/300000676> ;
  rdfs:subClassOf <https://w3id.org/con-tax/zones/aat-buildingSites#300000385> ;
.
<https://w3id.org/con-tax/zones/aat-buildingSites#300000677>
  rdf:type owl:Class ;
  rdfs:comment "Buildings or complexes providing transportation facilities or otherwise serving transportation needs."@en ;
  rdfs:isDefinedBy <https://w3id.org/con-tax/zones/aat-buildingSites> ;
  rdfs:label "transportation complexes"@en ;
  rdfs:label "transportcomplex"@nl ;
  rdfs:label "transportcomplexen"@nl ;
  rdfs:seeAlso <http://vocab.getty.edu/aat/300000677> ;
  rdfs:subClassOf <https://w3id.org/con-tax/zones/aat-buildingSites#300000202> ;
.
<https://w3id.org/con-tax/zones/aat-buildingSites#300000678>
  rdf:type owl:Class ;
  rdfs:comment "Complexes containing facilities to accommodate people, functions, and vehicles having to do with air transportation."@en ;
  rdfs:isDefinedBy <https://w3id.org/con-tax/zones/aat-buildingSites> ;
  rdfs:label "air transportation complexes"@en ;
  rdfs:label "luchttransportcomplexen"@nl ;
  rdfs:seeAlso <http://vocab.getty.edu/aat/300000678> ;
  rdfs:subClassOf <https://w3id.org/con-tax/zones/aat-buildingSites#300000677> ;
.
<https://w3id.org/con-tax/zones/aat-buildingSites#300000681>
  rdf:type owl:Class ;
  rdfs:comment "Typically refers to large tracts of open, level land upon which runways, hangars, terminals, and other buildings have been constructed to allow for the takeoffs, landings, loading and unloading, and maintenance of aircraft. For smaller areas that have a runway but no or few additional facilities, see \"airfields.\""@en ;
  rdfs:comment "Verwijst meestal naar grote percelen open, vlak land waarop start- en landingsbanen, hangars, stationsgebouwen en andere bouwwerken zijn verrezen, bestemd voor het opstijgen, landen, laden en lossen en onderhouden van vliegtuigen. Zie 'vliegvelden' voor kleinere complexen die wel een start- en landingsbaan hebben, maar geen of weinig andere voorzieningen."@nl ;
  rdfs:isDefinedBy <https://w3id.org/con-tax/zones/aat-buildingSites> ;
  rdfs:label "airports"@en ;
  rdfs:label "luchthaven"@nl ;
  rdfs:label "luchthavencomplex"@nl ;
  rdfs:label "luchthavencomplexen"@nl ;
  rdfs:label "luchthavens"@nl ;
  rdfs:seeAlso <http://vocab.getty.edu/aat/300000681> ;
  rdfs:seeAlso wd:Q1248784 ;
  rdfs:subClassOf <https://w3id.org/con-tax/zones/aat-buildingSites#300000678> ;
.
<https://w3id.org/con-tax/zones/aat-buildingSites#300000686>
  rdf:type owl:Class ;
  rdfs:comment "Landing places for helicopters."@en ;
  rdfs:isDefinedBy <https://w3id.org/con-tax/zones/aat-buildingSites> ;
  rdfs:label "helihaven"@nl ;
  rdfs:label "helihavens"@nl ;
  rdfs:label "heliport"@nl ;
  rdfs:label "heliports (airports)"@en ;
  rdfs:label "heliports"@nl ;
  rdfs:seeAlso <http://vocab.getty.edu/aat/300000686> ;
  rdfs:seeAlso wd:Q502074 ;
  rdfs:subClassOf <https://w3id.org/con-tax/zones/aat-buildingSites#300000681> ;
.
<https://w3id.org/con-tax/zones/aat-buildingSites#300000688>
  rdf:type owl:Class ;
  rdfs:comment "Facilities at which rocket, missile, or spacecraft launches are conducted, usually having launch pads, equipment, and various buildings."@en ;
  rdfs:isDefinedBy <https://w3id.org/con-tax/zones/aat-buildingSites> ;
  rdfs:label "lanceerbases"@nl ;
  rdfs:label "lanceerbasis"@nl ;
  rdfs:label "launch complexes"@en ;
  rdfs:seeAlso <http://vocab.getty.edu/aat/300000688> ;
  rdfs:subClassOf <https://w3id.org/con-tax/zones/aat-buildingSites#300000678> ;
  rdfs:subClassOf <https://w3id.org/con-tax/zones/aat-buildingSites#300387039> ;
.
<https://w3id.org/con-tax/zones/aat-buildingSites#300000690>
  rdf:type owl:Class ;
  rdfs:comment "Areas consisting of a network of railway tracks, sidings, and sheds for storing, maintaining, and joining engines and railcars."@en ;
  rdfs:comment "Door een spoorwegmaatschappij ingericht en geëxploiteerd terrein."@nl ;
  rdfs:isDefinedBy <https://w3id.org/con-tax/zones/aat-buildingSites> ;
  rdfs:label "railroad yards"@en ;
  rdfs:label "spoorwegemplacement"@nl ;
  rdfs:label "spoorwegemplacementen"@nl ;
  rdfs:seeAlso <http://vocab.getty.edu/aat/300000690> ;
  rdfs:seeAlso wd:Q19563580 ;
  rdfs:subClassOf <https://w3id.org/con-tax/zones/aat-buildingSites#300000677> ;
.
<https://w3id.org/con-tax/zones/aat-buildingSites#300000691>
  rdf:type owl:Class ;
  rdfs:comment "Railroad yards in which trains are assembled from individual cars."@en ;
  rdfs:isDefinedBy <https://w3id.org/con-tax/zones/aat-buildingSites> ;
  rdfs:label "marshalling yards"@en ;
  rdfs:label "rangeerterrein"@nl ;
  rdfs:label "rangeerterreinen"@nl ;
  rdfs:seeAlso <http://vocab.getty.edu/aat/300000691> ;
  rdfs:seeAlso wd:Q519608 ;
  rdfs:subClassOf <https://w3id.org/con-tax/zones/aat-buildingSites#300000690> ;
.
<https://w3id.org/con-tax/zones/aat-buildingSites#300000701>
  rdf:type owl:Class ;
  rdfs:comment "Areas within a city where the principal governmental and cultural buildings are grouped; may also denote building complexes or individual buildings housing such a range of functions, especially when the construction was financed by municipal funds."@en ;
  rdfs:comment "Gebieden in een stad waar de belangrijkste regeringsgebouwen en culturele gebouwen staan; kan ook duiden op gebouwencomplexen of afzonderlijke gebouwen die dat soort functies behuizen, vooral wanneer de bouw werd gefinancierd met gemeentegelden."@nl ;
  rdfs:isDefinedBy <https://w3id.org/con-tax/zones/aat-buildingSites> ;
  rdfs:label "bestuurscentra"@nl ;
  rdfs:label "bestuurscentrum"@nl ;
  rdfs:label "civic centers"@en-us ;
  rdfs:seeAlso <http://vocab.getty.edu/aat/300000701> ;
  rdfs:subClassOf <https://w3id.org/con-tax/zones/aat-buildingSites#300000202> ;
.
<https://w3id.org/con-tax/zones/aat-buildingSites#300000809>
  rdf:type owl:Class ;
  rdfs:comment "Pieces of land or other physical positions on which something is located, particularly where human habitation or activities have taken place. Examples include sites that have archaeological or other historical context."@en ;
  rdfs:comment "Te gebruiken voor zowel de ligging als de locatie van een woonruimte of een bouwconstructie, voornamelijk met betrekking tot de omliggende omgeving, en voor het gebied of stuk grond waarop een specifieke activiteit of activiteiten zijn, waren of worden gesitueerd, voornamelijk in archeologische en andere historische contexten."@nl ;
  rdfs:isDefinedBy <https://w3id.org/con-tax/zones/aat-buildingSites> ;
  rdfs:label "site"@nl ;
  rdfs:label "sites (locations)"@en ;
  rdfs:label "sites"@nl ;
  rdfs:seeAlso <http://vocab.getty.edu/aat/300000809> ;
  rdfs:subClassOf <https://w3id.org/con-tax/zones/aat-buildingSites#300000202> ;
.
<https://w3id.org/con-tax/zones/aat-buildingSites#300000810>
  rdf:type owl:Class ;
  rdfs:comment "Locaties waar ooit menselijke activiteiten hebben plaatsgevonden en waar materiële resten, in wat voor vorm dan ook, zijn achtergebleven."@nl ;
  rdfs:comment "Locations where human activities once took place and some form of material evidence has been left behind, particularly sites where evidence of past activity is being or has been investigated using the discipline of archaeology."@en ;
  rdfs:isDefinedBy <https://w3id.org/con-tax/zones/aat-buildingSites> ;
  rdfs:label "archaeological sites"@en ;
  rdfs:label "archeologische site"@nl ;
  rdfs:label "archeologische sites"@nl ;
  rdfs:label "archeologische vindplaatsen"@nl ;
  rdfs:seeAlso <http://vocab.getty.edu/aat/300000810> ;
  rdfs:seeAlso wd:Q839954 ;
  rdfs:subClassOf <https://w3id.org/con-tax/zones/aat-buildingSites#300000809> ;
.
<https://w3id.org/con-tax/zones/aat-buildingSites#300000811>
  rdf:type owl:Class ;
  rdfs:comment "Places where one or more buildings are located, formerly were located, are under construction, or will be constructed."@en ;
  rdfs:isDefinedBy <https://w3id.org/con-tax/zones/aat-buildingSites> ;
  rdfs:label "bouwterrein"@nl ;
  rdfs:label "bouwterreinen"@nl ;
  rdfs:label "building sites"@en ;
  rdfs:seeAlso <http://vocab.getty.edu/aat/300000811> ;
  rdfs:subClassOf <https://w3id.org/con-tax/zones/aat-buildingSites#300000809> ;
.
<https://w3id.org/con-tax/zones/aat-buildingSites#300000815>
  rdf:type owl:Class ;
  rdfs:comment "Lots or portions of land sufficient for and intended to be used or currently being used as the site of a house."@en ;
  rdfs:isDefinedBy <https://w3id.org/con-tax/zones/aat-buildingSites> ;
  rdfs:label "homesites"@en ;
  rdfs:label "woningbouwterrein"@nl ;
  rdfs:label "woningbouwterreinen"@nl ;
  rdfs:seeAlso <http://vocab.getty.edu/aat/300000815> ;
  rdfs:subClassOf <https://w3id.org/con-tax/zones/aat-buildingSites#300000811> ;
.
<https://w3id.org/con-tax/zones/aat-buildingSites#300000816>
  rdf:type owl:Class ;
  rdfs:comment "Building sites upon which one or more industries are planned or located. For a grouping of industrial buildings, use \"industrial complexes\" or \"industrial parks.\""@en ;
  rdfs:comment "Wordt gebruikt voor terreinen waarop één of meer bedrijven zijn gepland of gebouwd. Gebruik 'fabriekscomplexen' of 'industrieparken' voor groeperingen van industriële gebouwen."@nl ;
  rdfs:isDefinedBy <https://w3id.org/con-tax/zones/aat-buildingSites> ;
  rdfs:label "industrial sites"@en ;
  rdfs:label "industrieterrein"@nl ;
  rdfs:label "industrieterreinen"@nl ;
  rdfs:seeAlso <http://vocab.getty.edu/aat/300000816> ;
  rdfs:subClassOf <https://w3id.org/con-tax/zones/aat-buildingSites#300000811> ;
.
<https://w3id.org/con-tax/zones/aat-buildingSites#300000820>
  rdf:type owl:Class ;
  rdfs:comment "Cleared and bounded areas, devoid of artifacts, and of unknown function found associated with hunter-gatherer camps, especially those of the North American Great Basin. Cleared and bounded areas, devoid of artifacts, and of unknown function found associated with hunter-gatherer camps, especially those of the North American Great Basin."@en ;
  rdfs:comment "Wordt gebruikt voor vrijgemaakte en afgeperkte terreinen, vrij van objecten, waarvan de functie niet bekend is en die worden gevonden rond de kampen van indianenstammen die voedsel verzamelen en jagen, vooral in het Noord-Amerikaanse Grote Bekken."@nl ;
  rdfs:isDefinedBy <https://w3id.org/con-tax/zones/aat-buildingSites> ;
  rdfs:label "dance ground"@nl ;
  rdfs:label "dance grounds"@en ;
  rdfs:label "dance grounds"@nl ;
  rdfs:seeAlso <http://vocab.getty.edu/aat/300000820> ;
  rdfs:subClassOf <https://w3id.org/con-tax/zones/aat-buildingSites#300000810> ;
.
<https://w3id.org/con-tax/zones/aat-buildingSites#300000833>
  rdf:type owl:Class ;
  rdfs:comment "Parcels of land with historic significance due to historic events, architectural, engineering or archaeological activities, etc."@en ;
  rdfs:isDefinedBy <https://w3id.org/con-tax/zones/aat-buildingSites> ;
  rdfs:label "historic sites"@en ;
  rdfs:label "historische site"@nl ;
  rdfs:label "historische sites"@nl ;
  rdfs:seeAlso <http://vocab.getty.edu/aat/300000833> ;
  rdfs:seeAlso wd:Q1081138 ;
  rdfs:subClassOf <https://w3id.org/con-tax/zones/aat-buildingSites#300000809> ;
.
<https://w3id.org/con-tax/zones/aat-buildingSites#300000835>
  rdf:type owl:Class ;
  rdfs:comment "Locations where a hostile meetings of opposing military forces in the course of a war have taken place."@en ;
  rdfs:comment "Wordt gebruikt voor plaatsen die het toneel zijn geweest van veldslagen."@nl ;
  rdfs:isDefinedBy <https://w3id.org/con-tax/zones/aat-buildingSites> ;
  rdfs:label "battlefields"@en ;
  rdfs:label "fronten (terreinen)"@nl ;
  rdfs:label "fronten"@nl ;
  rdfs:label "slagveld"@nl ;
  rdfs:label "slagvelden"@nl ;
  rdfs:label "strijdperken"@nl ;
  rdfs:seeAlso <http://vocab.getty.edu/aat/300000835> ;
  rdfs:seeAlso wd:Q21550389 ;
  rdfs:subClassOf <https://w3id.org/con-tax/zones/aat-buildingSites#300000809> ;
.
<https://w3id.org/con-tax/zones/aat-buildingSites#300004908>
  rdf:type owl:Class ;
  rdfs:comment "Distinguished from \"stables\" by their barnlike appearance and their use as housing primarily for farm stock, feed, and associated maintenance equipment."@en ;
  rdfs:comment "Te onderscheiden van \"stallen\" door schuurachtig uiterlijk en tevens gebruikt voor andere boerderijdieren en opslag van voedsel en gereedschap."@nl ;
  rdfs:isDefinedBy <https://w3id.org/con-tax/zones/aat-buildingSites> ;
  rdfs:label "horse barns"@en ;
  rdfs:label "paardenstal (schuren)"@nl ;
  rdfs:label "paardenstal"@nl ;
  rdfs:label "paardenstallen (schuren)"@nl ;
  rdfs:label "paardenstallen"@nl ;
  rdfs:seeAlso <http://vocab.getty.edu/aat/300004908> ;
  rdfs:seeAlso wd:Q1303167 ;
  rdfs:seeAlso wd:Q214252 ;
  rdfs:subClassOf <https://w3id.org/con-tax/zones/aat-buildingSites#300199033> ;
  rdfs:subClassOf <https://w3id.org/con-tax/zones/aat-buildingSites#300262974> ;
.
<https://w3id.org/con-tax/zones/aat-buildingSites#300005261>
  rdf:type owl:Class ;
  rdfs:comment "Covered pedestrian passageways lined with shops or booths; usually found in urban settings and often linking two or more thoroughfares."@en ;
  rdfs:comment "Wordt gebruikt voor overdekte galerijen met aan weerszijden winkels en kraampjes; bevinden zich meestal in de stad en verbinden vaak twee hoofdstraten."@nl ;
  rdfs:isDefinedBy <https://w3id.org/con-tax/zones/aat-buildingSites> ;
  rdfs:label "shopping arcades"@en ;
  rdfs:label "winkelgalerij"@nl ;
  rdfs:label "winkelgalerijen"@nl ;
  rdfs:seeAlso <http://vocab.getty.edu/aat/300005261> ;
  rdfs:seeAlso wd:Q11315 ;
  rdfs:subClassOf <https://w3id.org/con-tax/zones/aat-buildingSites#300005268> ;
.
<https://w3id.org/con-tax/zones/aat-buildingSites#300005268>
  rdf:type owl:Class ;
  rdfs:comment "Concentratie van winkels, markten en dienstverlenende ondernemingen, samen met parkeergelegenheid en vaak gelegen in een buitenwijk."@nl ;
  rdfs:comment "Concentrations of stores, markets, and service establishments, along with parking facilities, often in a suburban location."@en ;
  rdfs:isDefinedBy <https://w3id.org/con-tax/zones/aat-buildingSites> ;
  rdfs:label "shopping centers"@en-us ;
  rdfs:label "winkelcentra"@nl ;
  rdfs:label "winkelcentrum"@nl ;
  rdfs:seeAlso <http://vocab.getty.edu/aat/300005268> ;
  rdfs:subClassOf <https://w3id.org/con-tax/zones/aat-buildingSites#300132652> ;
.
<https://w3id.org/con-tax/zones/aat-buildingSites#300005270>
  rdf:type owl:Class ;
  rdfs:comment "Structure or series of structures, either under a single roof or in open air, designed to house multiple retail outlets and to allow free passage of pedestrians on one or more levels."@en ;
  rdfs:isDefinedBy <https://w3id.org/con-tax/zones/aat-buildingSites> ;
  rdfs:label "shopping malls"@en ;
  rdfs:label "winkelpromenade"@nl ;
  rdfs:label "winkelpromenades"@nl ;
  rdfs:seeAlso <http://vocab.getty.edu/aat/300005270> ;
  rdfs:seeAlso wd:Q11315 ;
  rdfs:subClassOf <https://w3id.org/con-tax/zones/aat-buildingSites#300005268> ;
.
<https://w3id.org/con-tax/zones/aat-buildingSites#300005272>
  rdf:type owl:Class ;
  rdfs:comment "Shopping centers located underground, typically in an urban environment and often in association with underground subway stations or underground pedestrian passages between and under streets."@en ;
  rdfs:isDefinedBy <https://w3id.org/con-tax/zones/aat-buildingSites> ;
  rdfs:label "ondergronds winkelcentrum"@nl ;
  rdfs:label "ondergrondse winkelcentra"@nl ;
  rdfs:label "underground shopping centers"@en-us ;
  rdfs:seeAlso <http://vocab.getty.edu/aat/300005272> ;
  rdfs:subClassOf <https://w3id.org/con-tax/zones/aat-buildingSites#300005268> ;
.
<https://w3id.org/con-tax/zones/aat-buildingSites#300006448>
  rdf:type owl:Class ;
  rdfs:comment "General term for buildings or groups of buildings in which people accused or convicted of breaking the law may be confined and which may or may not attempt some form of reform or rehabilitative correction of offenders."@en ;
  rdfs:comment "Wordt gebruikt voor gebouwen waarin mensen kunnen worden opgesloten die zijn beschuldigd van of veroordeeld voor het breken van de wet, en waar al of niet een poging wordt gedaan tot verbeterende of rehabiliterende heropvoeding van de misdadigers. Zie 'gevangeniscomplexen' voor groepen van dergelijke gebouwen en 'strafkampen' voor dergelijke inrichtingen in de vorm van kampementen."@nl ;
  rdfs:isDefinedBy <https://w3id.org/con-tax/zones/aat-buildingSites> ;
  rdfs:label "correctional institutions (buildings)"@en ;
  rdfs:label "correctionele instellingen"@nl ;
  rdfs:label "strafrechtelijke instelling"@nl ;
  rdfs:label "strafrechtelijke instellingen"@nl ;
  rdfs:seeAlso <http://vocab.getty.edu/aat/300006448> ;
  rdfs:subClassOf <https://w3id.org/con-tax/zones/aat-buildingSites#300122216> ;
.
<https://w3id.org/con-tax/zones/aat-buildingSites#300006453>
  rdf:type owl:Class ;
  rdfs:comment "Places of relatively short confinement for youthful offenders pending transfer or trial."@en ;
  rdfs:comment "Wordt gebruikt voor plaatsen voor betrekkelijk korte opsluiting van jeugdige overtreders in afwachting van overplaatsing of rechtszaak."@nl ;
  rdfs:isDefinedBy <https://w3id.org/con-tax/zones/aat-buildingSites> ;
  rdfs:label "detention centers"@en-us ;
  rdfs:label "jeugdgevangenis"@nl ;
  rdfs:label "jeugdgevangenissen"@nl ;
  rdfs:seeAlso <http://vocab.getty.edu/aat/300006453> ;
  rdfs:subClassOf <https://w3id.org/con-tax/zones/aat-buildingSites#300006483> ;
.
<https://w3id.org/con-tax/zones/aat-buildingSites#300006457>
  rdf:type owl:Class ;
  rdfs:comment "Buildings that house places of confinement operated by a local government both for temporary detention of sentenced and unsentenced individuals and for persons serving sentences of less than one year; for longer periods of confinement and more secure than lockups, but less confining and for shorter confinements than prisons."@en ;
  rdfs:comment "Wordt gebruikt voor plaatsen van bewaring die worden bestuurd door de plaatselijke regering, voor zowel de tijdelijke hechtenis van veroordeelde of niet-veroordeelde personen en voor mensen die een straf uitzitten van minder dan een jaar; wordt gebruikt voor langere en beter beveiligde opsluiting dan arrestantenhokken, maar zijn minder beperkend en voor kortere straffen dan 'gevangenissen'."@nl ;
  rdfs:isDefinedBy <https://w3id.org/con-tax/zones/aat-buildingSites> ;
  rdfs:label "huis van bewaring"@nl ;
  rdfs:label "huizen van bewaring"@nl ;
  rdfs:label "jails (buildings)"@en ;
  rdfs:seeAlso <http://vocab.getty.edu/aat/300006457> ;
  rdfs:subClassOf <https://w3id.org/con-tax/zones/aat-buildingSites#300006448> ;
.
<https://w3id.org/con-tax/zones/aat-buildingSites#300006460>
  rdf:type owl:Class ;
  rdfs:comment "Buildings or other facilities to which people are legally committed as punishment for a crime or while awaiting trial. In North America, the term specifically denotes a facility run by the state or federal government for those who have been convicted of serious crimes, in contrast to a locally run facility for those awaiting trial or convicted of minor offences. As developed since the late 18th century, prisons are generally characterized by cell and corridor plans with separation by offense and sex, and programs of rehabilitation provided as means toward prisoner reform. Use \"jails (buildings)\" for places for offenders sentenced either for lesser crimes or relatively short terms."@en ;
  rdfs:comment "Gebruik voor plaatsen van verzekerde bewaring beheerd door de staat (of de federale overheid) voor volwassenen die veroordeeld zijn tot straffen (van meer dan een jaar) voor ernstige misdaden. Deze werde sinds de late 18de eeuw ontwikkeld en in het algemeen gekarakteriseerd door cellen en gangenstelsels met scheiding naar misdaad en geslacht. Daarbij werden programma's van rehabilitatie bedacht, als middel voor de heropvoeding van gevangene. Gebruik \"huizen van bewaring\" voor plaatsen voor overtreders die nog niet veroordeeld zijn maar wel in voorlopige hechtenis zijn gesteld."@nl ;
  rdfs:isDefinedBy <https://w3id.org/con-tax/zones/aat-buildingSites> ;
  rdfs:label "gevangenis"@nl ;
  rdfs:label "gevangenissen"@nl ;
  rdfs:label "penitentiaire inrichting"@nl ;
  rdfs:label "penitentiaire inrichtingen"@nl ;
  rdfs:label "prisons (buildings)"@en ;
  rdfs:label "strafinrichting"@nl ;
  rdfs:label "strafinrichtingen"@nl ;
  rdfs:seeAlso <http://vocab.getty.edu/aat/300006460> ;
  rdfs:subClassOf <https://w3id.org/con-tax/zones/aat-buildingSites#300006448> ;
  contax:containsGuideTerm <https://w3id.org/con-tax/zones/aat-buildingSites#300122445> ;
  contax:containsGuideTerm <https://w3id.org/con-tax/zones/aat-buildingSites#300168612> ;
.
<https://w3id.org/con-tax/zones/aat-buildingSites#300006463>
  rdf:type owl:Class ;
  rdfs:comment "Ancient Roman domestic buildings used for the confinement of slave workers."@en ;
  rdfs:comment "Werkhuizen en tuchthuizen voor slaven en soms schuldenaars in het antieke Rome."@nl ;
  rdfs:isDefinedBy <https://w3id.org/con-tax/zones/aat-buildingSites> ;
  rdfs:label "ergastula"@en ;
  rdfs:label "ergastula"@nl ;
  rdfs:label "ergastulum"@nl ;
  rdfs:seeAlso <http://vocab.getty.edu/aat/300006463> ;
  rdfs:seeAlso wd:Q1989526 ;
  rdfs:subClassOf <https://w3id.org/con-tax/zones/aat-buildingSites#300006448> ;
.
<https://w3id.org/con-tax/zones/aat-buildingSites#300006466>
  rdf:type owl:Class ;
  rdfs:comment "Buildings that house prisons populated by prisoners who can be reasonably trusted to not to try to escape; the term is often used in British prison systems."@en ;
  rdfs:isDefinedBy <https://w3id.org/con-tax/zones/aat-buildingSites> ;
  rdfs:label "open gevangenis"@nl ;
  rdfs:label "open gevangenissen"@nl ;
  rdfs:label "open prisons"@en ;
  rdfs:seeAlso <http://vocab.getty.edu/aat/300006466> ;
  rdfs:seeAlso wd:Q319382 ;
  rdfs:subClassOf <https://w3id.org/con-tax/zones/aat-buildingSites#300006460> ;
.
<https://w3id.org/con-tax/zones/aat-buildingSites#300006477>
  rdf:type owl:Class ;
  rdfs:comment "Buildings that house places of detention primarily for debtors."@en ;
  rdfs:comment "Wordt gebruikt voor plaatsen van bewaring die voornamelijk worden gebruikt voor schuldenaren. Geen Nederlands equivalent. Zie 'gevangenissen'."@nl ;
  rdfs:isDefinedBy <https://w3id.org/con-tax/zones/aat-buildingSites> ;
  rdfs:label "debtor's prison"@nl ;
  rdfs:label "debtor's prisons"@nl ;
  rdfs:label "debtors' prisons"@en ;
  rdfs:seeAlso <http://vocab.getty.edu/aat/300006477> ;
  rdfs:subClassOf <https://w3id.org/con-tax/zones/aat-buildingSites#300006460> ;
.
<https://w3id.org/con-tax/zones/aat-buildingSites#300006479>
  rdf:type owl:Class ;
  rdfs:comment "Buildings housing prisons administered by a federal government, in the U.S., those managed by the U.S. Federal Bureau of Prisons."@en ;
  rdfs:isDefinedBy <https://w3id.org/con-tax/zones/aat-buildingSites> ;
  rdfs:label "federal prison"@nl ;
  rdfs:label "federal prisons (buildings)"@en ;
  rdfs:label "federal prisons"@nl ;
  rdfs:seeAlso <http://vocab.getty.edu/aat/300006479> ;
  rdfs:subClassOf <https://w3id.org/con-tax/zones/aat-buildingSites#300006460> ;
.
<https://w3id.org/con-tax/zones/aat-buildingSites#300006481>
  rdf:type owl:Class ;
  rdfs:comment "Buildings that house prisons administered by the state, particularly a state in the U.S."@en ;
  rdfs:isDefinedBy <https://w3id.org/con-tax/zones/aat-buildingSites> ;
  rdfs:label "staatsgevangenis"@nl ;
  rdfs:label "staatsgevangenissen"@nl ;
  rdfs:label "state prisons (buildings)"@en ;
  rdfs:seeAlso <http://vocab.getty.edu/aat/300006481> ;
  rdfs:subClassOf <https://w3id.org/con-tax/zones/aat-buildingSites#300006460> ;
.
<https://w3id.org/con-tax/zones/aat-buildingSites#300006483>
  rdf:type owl:Class ;
  rdfs:comment "Buildings housing penal institutions that provide educational and vocational training among other methods for reforming behavior of youthful offenders or first offenders of minor crimes."@en ;
  rdfs:comment "Wordt gebruikt voor strafinrichtingen voor jeugdige overtreders van tussen de 12 en 19 jaar, of eenmalige overtreders met minder ernstige vergrijpen, waar school- en beroepsonderwijs wordt aangeboden als een middel tot hervorming van gedrag."@nl ;
  rdfs:isDefinedBy <https://w3id.org/con-tax/zones/aat-buildingSites> ;
  rdfs:label "reformatories (buildings)"@en ;
  rdfs:label "tuchtscholen"@nl ;
  rdfs:label "tuchtschool"@nl ;
  rdfs:label "verbeteringsgesticht"@nl ;
  rdfs:label "verbeteringsgestichten"@nl ;
  rdfs:seeAlso <http://vocab.getty.edu/aat/300006483> ;
  rdfs:seeAlso wd:Q7307453 ;
  rdfs:subClassOf <https://w3id.org/con-tax/zones/aat-buildingSites#300006448> ;
.
<https://w3id.org/con-tax/zones/aat-buildingSites#300006490>
  rdf:type owl:Class ;
  rdfs:comment "Buildings that housed places of confinement and labor for paupers, vagrants, and the disabled or elderly poor from the 17th through 19th century in Europe and America. For buildings housing similar institutions intended to provide punishment and reformation of the criminal, use \"houses of correction (buildings).\" For welfare buildings providing charitable care for the poor, use \"almshouses (buildings).\""@en ;
  rdfs:comment "Wordt gebruikt voor plaatsen van bewaring of heropvoeding, in gebruik vanaf de 16e eeuw, die zwaar werk en strenge discipline als hervormende maatregelen gebruiken voor mensen die kleine overtredingen hebben begaan, zwervers en invalide of oudere armen. Gebruik 'armenhuizen' voor bijstandsgebouwen die liefdadige zorg en werk bieden voor armen."@nl ;
  rdfs:isDefinedBy <https://w3id.org/con-tax/zones/aat-buildingSites> ;
  rdfs:label "rasphuis"@nl ;
  rdfs:label "rasphuizen"@nl ;
  rdfs:label "spinhuis"@nl ;
  rdfs:label "spinhuizen"@nl ;
  rdfs:label "tuchthuis"@nl ;
  rdfs:label "tuchthuizen"@nl ;
  rdfs:label "werkhuis"@nl ;
  rdfs:label "werkhuizen"@nl ;
  rdfs:label "werkinrichting"@nl ;
  rdfs:label "werkinrichtingen"@nl ;
  rdfs:label "workhouses (buildings)"@en ;
  rdfs:seeAlso <http://vocab.getty.edu/aat/300006490> ;
  rdfs:seeAlso wd:Q628155 ;
  rdfs:subClassOf <https://w3id.org/con-tax/zones/aat-buildingSites#300006448> ;
.
<https://w3id.org/con-tax/zones/aat-buildingSites#300006737>
  rdf:type owl:Class ;
  rdfs:comment "Resorts or other facilities possessing or located near natural mineral springs or pools that are valued because of the believed restorative or curative powers of the water; also, artificial pools or other aquatic facilities containing waters believed to have restorative powers. The term is derived from the proper name of Spa, Liège province, Belgium, celebrated for the believed curative properties of its mineral springs."@en ;
  rdfs:isDefinedBy <https://w3id.org/con-tax/zones/aat-buildingSites> ;
  rdfs:label "spas (health resorts)"@en ;
  rdfs:label "thermaal kuuroord"@nl ;
  rdfs:label "thermale kuuroorden"@nl ;
  rdfs:seeAlso <http://vocab.getty.edu/aat/300006737> ;
  rdfs:subClassOf <https://w3id.org/con-tax/zones/aat-buildingSites#300000553> ;
.
<https://w3id.org/con-tax/zones/aat-buildingSites#300007204>
  rdf:type owl:Class ;
  rdfs:comment "Buildings or rooms occupied by associations formed to combine the operations of persons interested in the promotion or playing of tennis."@en ;
  rdfs:isDefinedBy <https://w3id.org/con-tax/zones/aat-buildingSites> ;
  rdfs:label "tennis clubs"@en ;
  rdfs:label "tennisclub"@nl ;
  rdfs:label "tennisclubs"@nl ;
  rdfs:seeAlso <http://vocab.getty.edu/aat/300007204> ;
  rdfs:subClassOf <https://w3id.org/con-tax/zones/aat-buildingSites#300203159> ;
.
<https://w3id.org/con-tax/zones/aat-buildingSites#300007205>
  rdf:type owl:Class ;
  rdfs:comment "Water recreation complexes including clubhouse, marina, and associated boating facilities."@en ;
  rdfs:comment "Waterrecreatie complexen met inbegrip van clubgebouw, jachthaven, en de bijbehorende voorzieningen voor boten."@nl ;
  rdfs:isDefinedBy <https://w3id.org/con-tax/zones/aat-buildingSites> ;
  rdfs:label "boat clubs"@en ;
  rdfs:label "bootclub"@nl ;
  rdfs:label "bootclubs"@nl ;
  rdfs:seeAlso <http://vocab.getty.edu/aat/300007205> ;
  rdfs:seeAlso wd:Q4931504 ;
  rdfs:subClassOf <https://w3id.org/con-tax/zones/aat-buildingSites#300203159> ;
.
<https://w3id.org/con-tax/zones/aat-buildingSites#300007752>
  rdf:type owl:Class ;
  rdfs:comment "Complexes providing facilities to accommodate the movement of cargo or passengers among ships or between ships and shore."@en ;
  rdfs:comment "Gebruik voor complexen die faciliteiten bieden die het verkeer van lading of passagiers tussen schepen of tussen schepen en de wal mogelijk maken."@nl ;
  rdfs:isDefinedBy <https://w3id.org/con-tax/zones/aat-buildingSites> ;
  rdfs:label "marine terminals"@en ;
  rdfs:label "terminal (scheepvaart)"@nl ;
  rdfs:label "terminal"@nl ;
  rdfs:label "terminals (scheepvaart)"@nl ;
  rdfs:label "terminals"@nl ;
  rdfs:seeAlso <http://vocab.getty.edu/aat/300007752> ;
  rdfs:subClassOf <https://w3id.org/con-tax/zones/aat-buildingSites#300120802> ;
.
<https://w3id.org/con-tax/zones/aat-buildingSites#300007915>
  rdf:type owl:Class ;
  rdfs:comment "Een doorgaans geasfalteerde strook bij een luchthaven waarover de vliegtuigen taxiën."@nl ;
  rdfs:comment "Usually paved strips for taxiing at an airport."@en ;
  rdfs:isDefinedBy <https://w3id.org/con-tax/zones/aat-buildingSites> ;
  rdfs:label "taxibaan"@nl ;
  rdfs:label "taxibanen"@nl ;
  rdfs:label "taxiways"@en ;
  rdfs:seeAlso <http://vocab.getty.edu/aat/300007915> ;
  rdfs:seeAlso wd:Q910386 ;
  rdfs:subClassOf <https://w3id.org/con-tax/zones/aat-buildingSites#300000681> ;
.
<https://w3id.org/con-tax/zones/aat-buildingSites#300007917>
  rdf:type owl:Class ;
  rdfs:comment "Runways without normal airport facilities."@en ;
  rdfs:comment "Wordt gebruikt voor startbanen zonder normale luchthavenvoorzieningen."@nl ;
  rdfs:isDefinedBy <https://w3id.org/con-tax/zones/aat-buildingSites> ;
  rdfs:label "airstrips"@en-us ;
  rdfs:label "landingsbaan"@nl ;
  rdfs:label "landingsbanen"@nl ;
  rdfs:seeAlso <http://vocab.getty.edu/aat/300007917> ;
  rdfs:subClassOf <https://w3id.org/con-tax/zones/aat-buildingSites#300007918> ;
.
<https://w3id.org/con-tax/zones/aat-buildingSites#300007918>
  rdf:type owl:Class ;
  rdfs:comment "Specially prepared surfaces on an airfield for the taking off and landing of aircraft."@en ;
  rdfs:isDefinedBy <https://w3id.org/con-tax/zones/aat-buildingSites> ;
  rdfs:label "runways (airport runways)"@en ;
  rdfs:label "startbaan"@nl ;
  rdfs:label "startbanen"@nl ;
  rdfs:seeAlso <http://vocab.getty.edu/aat/300007918> ;
  rdfs:subClassOf <https://w3id.org/con-tax/zones/aat-buildingSites#300000681> ;
.
<https://w3id.org/con-tax/zones/aat-buildingSites#300007919>
  rdf:type owl:Class ;
  rdfs:comment "Cleared but unpaved areas at the end of runways offering extra landing roll to an airplane in an emergency."@en ;
  rdfs:comment "Niet geasfalteerde stroken grond aan het einde van landingsbanen die  worden vrijgehouden om extra landingsruimte te bieden aan vliegtuigen in noodsituaties."@nl ;
  rdfs:isDefinedBy <https://w3id.org/con-tax/zones/aat-buildingSites> ;
  rdfs:label "inloopsectie"@nl ;
  rdfs:label "inloopsecties"@nl ;
  rdfs:label "overruns"@en ;
  rdfs:seeAlso <http://vocab.getty.edu/aat/300007919> ;
  rdfs:subClassOf <https://w3id.org/con-tax/zones/aat-buildingSites#300000681> ;
.
<https://w3id.org/con-tax/zones/aat-buildingSites#300008168>
  rdf:type owl:Class ;
  rdfs:comment "Areas comprised of individual camp sites and providing facilities and conveniences for camping."@en ;
  rdfs:comment "Wordt gebruikt voor terreinen of gebieden om te kamperen met de benodigde faciliteiten."@nl ;
  rdfs:isDefinedBy <https://w3id.org/con-tax/zones/aat-buildingSites> ;
  rdfs:label "campgrounds"@en-us ;
  rdfs:label "camping"@nl ;
  rdfs:label "campings"@nl ;
  rdfs:label "kampeerterrein"@nl ;
  rdfs:label "kampeerterreinen"@nl ;
  rdfs:seeAlso <http://vocab.getty.edu/aat/300008168> ;
  rdfs:seeAlso wd:Q832778 ;
  rdfs:subClassOf <https://w3id.org/con-tax/zones/aat-buildingSites#300000510> ;
.
<https://w3id.org/con-tax/zones/aat-buildingSites#300008187>
  rdf:type owl:Class ;
  rdfs:comment "Aanduiding voor bepaalde openbare ruimten met een permanente recreatieve functie die meestal worden gekenmerkt door hun natuurlijke, historische of landschappelijke aspecten en  vaak door overheidsinstanties worden beheerd."@nl ;
  rdfs:comment "Permanently dedicated recreation areas, often open to the public and generally characterized by their natural, historic, or landscape features; often administered by governmental agencies."@en ;
  rdfs:isDefinedBy <https://w3id.org/con-tax/zones/aat-buildingSites> ;
  rdfs:label "park (openbare ruimte)"@nl ;
  rdfs:label "park"@nl ;
  rdfs:label "parken (openbare ruimten)"@nl ;
  rdfs:label "parken"@nl ;
  rdfs:label "parks (public recreation areas)"@en ;
  rdfs:seeAlso <http://vocab.getty.edu/aat/300008187> ;
  rdfs:subClassOf <https://w3id.org/con-tax/zones/aat-buildingSites#300000510> ;
  contax:containsGuideTerm <https://w3id.org/con-tax/zones/aat-buildingSites#300008188> ;
  contax:containsGuideTerm <https://w3id.org/con-tax/zones/aat-buildingSites#300008201> ;
.
<https://w3id.org/con-tax/zones/aat-buildingSites#300008188>
  rdf:type gvp:GuideTerm ;
  rdfs:isDefinedBy <https://w3id.org/con-tax/zones/aat-buildingSites> ;
  rdfs:label "<parken naar locatie of context>"@nl ;
  rdfs:label "<parks by location or context>"@en ;
  rdfs:label "parken naar locatie of context"@nl ;
  rdfs:seeAlso <http://vocab.getty.edu/aat/300008188> ;
  contax:containsConcept <https://w3id.org/con-tax/zones/aat-buildingSites#300008193> ;
  contax:containsConcept <https://w3id.org/con-tax/zones/aat-buildingSites#300008196> ;
  contax:containsConcept <https://w3id.org/con-tax/zones/aat-buildingSites#300008197> ;
  contax:containsConcept <https://w3id.org/con-tax/zones/aat-buildingSites#300065080> ;
  contax:containsConcept <https://w3id.org/con-tax/zones/aat-buildingSites#300072250> ;
  contax:containsConcept <https://w3id.org/con-tax/zones/aat-buildingSites#300151282> ;
  contax:containsConcept <https://w3id.org/con-tax/zones/aat-buildingSites#300265609> ;
  contax:containsConcept <https://w3id.org/con-tax/zones/aat-buildingSites#300379361> ;
  contax:containsConcept <https://w3id.org/con-tax/zones/aat-buildingSites#300380027> ;
  contax:containsConcept <https://w3id.org/con-tax/zones/aat-buildingSites#300380520> ;
  contax:containsConcept <https://w3id.org/con-tax/zones/aat-buildingSites#300386977> ;
  contax:containsConcept <https://w3id.org/con-tax/zones/aat-buildingSites#300386978> ;
  contax:containsConcept <https://w3id.org/con-tax/zones/aat-buildingSites#300386979> ;
.
<https://w3id.org/con-tax/zones/aat-buildingSites#300008189>
  rdf:type owl:Class ;
  rdfs:comment "Afgebakende gebieden met een bijzondere landschappelijke, historische of wetenschappelijke waarde die door  een nationale overheid voor recreatie- of studiedoeleinden worden onderhouden.."@nl ;
  rdfs:comment "Areas of special scenic, historical, or scientific importance set aside and maintained by a national government especially for recreation or study."@en ;
  rdfs:isDefinedBy <https://w3id.org/con-tax/zones/aat-buildingSites> ;
  rdfs:label "nationaal park"@nl ;
  rdfs:label "national parks"@en ;
  rdfs:label "nationale parken"@nl ;
  rdfs:seeAlso <http://vocab.getty.edu/aat/300008189> ;
  rdfs:seeAlso wd:Q46169 ;
  rdfs:subClassOf <https://w3id.org/con-tax/zones/aat-buildingSites#300008187> ;
.
<https://w3id.org/con-tax/zones/aat-buildingSites#300008192>
  rdf:type owl:Class ;
  rdfs:comment "Parks owned or maintained by the state, particularly a U.S. state."@en ;
  rdfs:isDefinedBy <https://w3id.org/con-tax/zones/aat-buildingSites> ;
  rdfs:label "staatspark"@nl ;
  rdfs:label "staatsparken"@nl ;
  rdfs:label "state parks"@en ;
  rdfs:seeAlso <http://vocab.getty.edu/aat/300008192> ;
  rdfs:seeAlso wd:Q1761072 ;
  rdfs:subClassOf <https://w3id.org/con-tax/zones/aat-buildingSites#300008187> ;
.
<https://w3id.org/con-tax/zones/aat-buildingSites#300008193>
  rdf:type owl:Class ;
  rdfs:comment "Parks set aside for the habitual play of residents of urban neighborhoods; usually smaller and with fewer activities than \"community parks.\""@en ;
  rdfs:comment "Te gebruiken voor parken voor de vaste bewoners van stedelijke wijken. Meestal kleiner en met minder voorzieningen dan 'gemeenschapsparken'."@nl ;
  rdfs:isDefinedBy <https://w3id.org/con-tax/zones/aat-buildingSites> ;
  rdfs:label "buurtpark"@nl ;
  rdfs:label "buurtparken"@nl ;
  rdfs:label "neighborhood parks"@en-us ;
  rdfs:seeAlso <http://vocab.getty.edu/aat/300008193> ;
  rdfs:subClassOf <https://w3id.org/con-tax/zones/aat-buildingSites#300008187> ;
.
<https://w3id.org/con-tax/zones/aat-buildingSites#300008195>
  rdf:type owl:Class ;
  rdfs:comment "Openbare parken, bijvoorbeeld in Canada, die worden beheerd door een provinciebestuur."@nl ;
  rdfs:comment "Public parks in Canada administered by the provincial government."@en ;
  rdfs:isDefinedBy <https://w3id.org/con-tax/zones/aat-buildingSites> ;
  rdfs:label "provinciaal park"@nl ;
  rdfs:label "provincial parks"@en ;
  rdfs:label "provinciale parken"@nl ;
  rdfs:seeAlso <http://vocab.getty.edu/aat/300008195> ;
  rdfs:seeAlso wd:Q2006279 ;
  rdfs:subClassOf <https://w3id.org/con-tax/zones/aat-buildingSites#300008187> ;
.
<https://w3id.org/con-tax/zones/aat-buildingSites#300008196>
  rdf:type owl:Class ;
  rdfs:comment "Deze parken, die over het algemeen kleiner zijn dan nationale parken, bieden een breed scala aan recreatievoorzieningen. Bovendien speelt bij de regionale parken de landschappelijke waarde van het gebied een minder grote rol dan bij de nationale parken."@nl ;
  rdfs:comment "Generally refers to parks that are smaller than national parks and providing a wide range of recreation facilities with less emphasis on the landscape value of the area."@en ;
  rdfs:isDefinedBy <https://w3id.org/con-tax/zones/aat-buildingSites> ;
  rdfs:label "regionaal park"@nl ;
  rdfs:label "regional parks"@en ;
  rdfs:label "regionale parken"@nl ;
  rdfs:seeAlso <http://vocab.getty.edu/aat/300008196> ;
  rdfs:seeAlso wd:Q6063204 ;
  rdfs:subClassOf <https://w3id.org/con-tax/zones/aat-buildingSites#300008187> ;
.
<https://w3id.org/con-tax/zones/aat-buildingSites#300008197>
  rdf:type owl:Class ;
  rdfs:comment "Kleine parken in gebieden (bijvoorbeeld in nieuwe steden) die in hoge mate zijn geürbaniseerd; dikwijls bevinden ze zich nabij een zakencentrum of een winkelgebied."@nl ;
  rdfs:comment "Small parks serving central business districts, highly urban areas (including new towns), or commercial districts."@en ;
  rdfs:isDefinedBy <https://w3id.org/con-tax/zones/aat-buildingSites> ;
  rdfs:label "stadspark"@nl ;
  rdfs:label "stadsparken"@nl ;
  rdfs:label "urban parks"@en ;
  rdfs:seeAlso <http://vocab.getty.edu/aat/300008197> ;
  rdfs:subClassOf <https://w3id.org/con-tax/zones/aat-buildingSites#300008187> ;
.
<https://w3id.org/con-tax/zones/aat-buildingSites#300008201>
  rdf:type gvp:GuideTerm ;
  rdfs:isDefinedBy <https://w3id.org/con-tax/zones/aat-buildingSites> ;
  rdfs:label "<park naar eigendom of beheer>"@nl ;
  rdfs:label "<parken naar eigendom of beheer>"@nl ;
  rdfs:label "<parks by ownership or administration>"@en ;
  rdfs:label "park naar eigendom of beheer"@nl ;
  rdfs:label "parken naar eigendom of beheer"@nl ;
  rdfs:seeAlso <http://vocab.getty.edu/aat/300008201> ;
  contax:containsConcept <https://w3id.org/con-tax/zones/aat-buildingSites#300008189> ;
  contax:containsConcept <https://w3id.org/con-tax/zones/aat-buildingSites#300008192> ;
  contax:containsConcept <https://w3id.org/con-tax/zones/aat-buildingSites#300008195> ;
  contax:containsConcept <https://w3id.org/con-tax/zones/aat-buildingSites#300417706> ;
.
<https://w3id.org/con-tax/zones/aat-buildingSites#300008439>
  rdf:type owl:Class ;
  rdfs:comment "Encampments formed by troops for long stays while on a campaign, especially during winter."@en ;
  rdfs:comment "Wordt gebruikt voor kampementen die door troepen worden opgebouwd voor langer verblijf tijdens een veldtocht, vooral in de winter."@nl ;
  rdfs:isDefinedBy <https://w3id.org/con-tax/zones/aat-buildingSites> ;
  rdfs:label "cantonments"@en ;
  rdfs:label "kantonnement"@nl ;
  rdfs:label "kantonnementen"@nl ;
  rdfs:seeAlso <http://vocab.getty.edu/aat/300008439> ;
  rdfs:seeAlso wd:Q2543279 ;
  rdfs:subClassOf <https://w3id.org/con-tax/zones/aat-buildingSites#300000476> ;
.
<https://w3id.org/con-tax/zones/aat-buildingSites#300008440>
  rdf:type owl:Class ;
  rdfs:comment "Permanent ancient Roman military encampments laid out on a grid; may also designate later castles, forts, or fortified towers."@en ;
  rdfs:comment "Wordt gebruikt voor permanente Romeinse militaire kampementen opgezet volgens een rastervormig patroon; ook een aanduiding voor kastelen, forten of versterkte torens."@nl ;
  rdfs:isDefinedBy <https://w3id.org/con-tax/zones/aat-buildingSites> ;
  rdfs:label "castra"@en ;
  rdfs:label "castra"@nl ;
  rdfs:label "castrum"@nl ;
  rdfs:seeAlso <http://vocab.getty.edu/aat/300008440> ;
  rdfs:seeAlso wd:Q88205 ;
  rdfs:subClassOf <https://w3id.org/con-tax/zones/aat-buildingSites#300000476> ;
.
<https://w3id.org/con-tax/zones/aat-buildingSites#300008459>
  rdf:type owl:Class ;
  rdfs:comment "Communities that grew up around or have economies centered on a site of religious pilgrimage and activities associated with the site."@en ;
  rdfs:isDefinedBy <https://w3id.org/con-tax/zones/aat-buildingSites> ;
  rdfs:label "bedevaartsoord"@nl ;
  rdfs:label "bedevaartsoorden"@nl ;
  rdfs:label "bedevaartsplaatsen"@nl ;
  rdfs:label "pilgrimage centers"@en-us ;
  rdfs:seeAlso <http://vocab.getty.edu/aat/300008459> ;
  rdfs:subClassOf <https://w3id.org/con-tax/zones/aat-buildingSites#300000809> ;
.
<https://w3id.org/con-tax/zones/aat-buildingSites#300008505>
  rdf:type owl:Class ;
  rdfs:comment "Residential treatment centers, often in a rural setting, which provide medical and counseling services for children with emotional problems."@en ;
  rdfs:comment "Wordt gebruikt voor behandelcentra, vaak in een landelijke omgeving, waar kinderen met emotionele problemen intern medische zorg en begeleiding krijgen."@nl ;
  rdfs:isDefinedBy <https://w3id.org/con-tax/zones/aat-buildingSites> ;
  rdfs:label "children's villages"@en ;
  rdfs:label "kinderdorp"@nl ;
  rdfs:label "kinderdorpen"@nl ;
  rdfs:seeAlso <http://vocab.getty.edu/aat/300008505> ;
  rdfs:subClassOf <https://w3id.org/con-tax/zones/aat-buildingSites#300000202> ;
.
<https://w3id.org/con-tax/zones/aat-buildingSites#300008528>
  rdf:type owl:Class ;
  rdfs:comment "Russian collective farms."@en ;
  rdfs:comment "Term voor Russische collectieve landbouwbedrijven."@nl ;
  rdfs:isDefinedBy <https://w3id.org/con-tax/zones/aat-buildingSites> ;
  rdfs:label "kolchoze"@nl ;
  rdfs:label "kolchozen"@nl ;
  rdfs:label "kolkhoz"@en ;
  rdfs:seeAlso <http://vocab.getty.edu/aat/300008528> ;
  rdfs:seeAlso wd:Q485016 ;
  rdfs:subClassOf <https://w3id.org/con-tax/zones/aat-buildingSites#300000210> ;
.
<https://w3id.org/con-tax/zones/aat-buildingSites#300008633>
  rdf:type owl:Class ;
  rdfs:comment "Farms, which are complexes where plants or animals are raised for livelihood or commerce, that have been deserted and are no longer functioning."@en ;
  rdfs:isDefinedBy <https://w3id.org/con-tax/zones/aat-buildingSites> ;
  rdfs:label "abandoned farms"@en ;
  rdfs:label "verlaten boerderij"@nl ;
  rdfs:label "verlaten boerderijen"@nl ;
  rdfs:seeAlso <http://vocab.getty.edu/aat/300008633> ;
  rdfs:subClassOf <https://w3id.org/con-tax/zones/aat-buildingSites#300000206> ;
.
<https://w3id.org/con-tax/zones/aat-buildingSites#300008819>
  rdf:type owl:Class ;
  rdfs:comment "Beaches set aside for or used by people immersing themselves in the water and exposing themselves to the sun and air for recreational purposes."@en ;
  rdfs:isDefinedBy <https://w3id.org/con-tax/zones/aat-buildingSites> ;
  rdfs:label "badstranden"@nl ;
  rdfs:label "bathing beaches"@en ;
  rdfs:seeAlso <http://vocab.getty.edu/aat/300008819> ;
  rdfs:subClassOf <https://w3id.org/con-tax/zones/aat-buildingSites#300000510> ;
.
<https://w3id.org/con-tax/zones/aat-buildingSites#300008890>
  rdf:type owl:Class ;
  rdfs:comment "Een fruitkwekerij of boomgaard is een kunstmatig beplant stuk grond waar vruchten- of notenbomen op gekweekt worden om voedsel te produceren."@nl ;
  rdfs:comment "Farms devoted to the cultivation of fruit or nut trees."@en ;
  rdfs:isDefinedBy <https://w3id.org/con-tax/zones/aat-buildingSites> ;
  rdfs:label "boomgaard"@nl ;
  rdfs:label "boomgaarden"@nl ;
  rdfs:label "fruitkwekerij"@nl ;
  rdfs:label "fruitkwekerijen"@nl ;
  rdfs:label "orchards"@en ;
  rdfs:seeAlso <http://vocab.getty.edu/aat/300008890> ;
  rdfs:seeAlso wd:Q236371 ;
  rdfs:subClassOf <https://w3id.org/con-tax/zones/aat-buildingSites#300000206> ;
.
<https://w3id.org/con-tax/zones/aat-buildingSites#300045490>
  rdf:type owl:Class ;
  rdfs:comment "Farm complexes, including living quarters and outbuildings, belonging to a monastery or a feudal lord."@en ;
  rdfs:comment "Wordt gebruikt voor boerderijencomplexen, inclusief woonverblijven en bijgebouwen, die het eigendom zijn van een klooster of een leenheer."@nl ;
  rdfs:isDefinedBy <https://w3id.org/con-tax/zones/aat-buildingSites> ;
  rdfs:label "grange"@nl ;
  rdfs:label "granges (farms)"@en ;
  rdfs:label "granges"@nl ;
  rdfs:seeAlso <http://vocab.getty.edu/aat/300045490> ;
  rdfs:subClassOf <https://w3id.org/con-tax/zones/aat-buildingSites#300000206> ;
.
<https://w3id.org/con-tax/zones/aat-buildingSites#300045498>
  rdf:type owl:Class ;
  rdfs:comment "Refers to enclosed, oval, circular, or rectangular spaces designed and equipped for horseback riding."@en ;
  rdfs:comment "Wordt gebruikt voor omheinde, meestal ronde of ovale ruimten bestemd voor paardrijden."@nl ;
  rdfs:isDefinedBy <https://w3id.org/con-tax/zones/aat-buildingSites> ;
  rdfs:label "piste (paardrijden)"@nl ;
  rdfs:label "piste"@nl ;
  rdfs:label "pistes (paardrijden)"@nl ;
  rdfs:label "pistes"@nl ;
  rdfs:label "riding rings"@en ;
  rdfs:seeAlso <http://vocab.getty.edu/aat/300045498> ;
  rdfs:subClassOf <https://w3id.org/con-tax/zones/aat-buildingSites#300262974> ;
.
<https://w3id.org/con-tax/zones/aat-buildingSites#300048698>
  rdf:type owl:Class ;
  rdfs:comment "Complexes designed to board horses and accommodate equestrian events such as competitions, dressage, and recreational riding."@en ;
  rdfs:isDefinedBy <https://w3id.org/con-tax/zones/aat-buildingSites> ;
  rdfs:label "riding clubs"@en ;
  rdfs:label "ruiterclub"@nl ;
  rdfs:label "ruiterclubs"@nl ;
  rdfs:seeAlso <http://vocab.getty.edu/aat/300048698> ;
  rdfs:subClassOf <https://w3id.org/con-tax/zones/aat-buildingSites#300203159> ;
.
<https://w3id.org/con-tax/zones/aat-buildingSites#300065080>
  rdf:type owl:Class ;
  rdfs:comment "Very small city parks, directly adjacent to and usually between buildings in a densely built area."@en ;
  rdfs:comment "Zeer kleine stadsparken, in de directe nabijheid en meestal te midden van gebouwen in een dichtbebouwde omgeving."@nl ;
  rdfs:isDefinedBy <https://w3id.org/con-tax/zones/aat-buildingSites> ;
  rdfs:label "miniatuurpark"@nl ;
  rdfs:label "miniatuurparken"@nl ;
  rdfs:label "vest-pocket parks"@en ;
  rdfs:seeAlso <http://vocab.getty.edu/aat/300065080> ;
  rdfs:seeAlso wd:Q1470855 ;
  rdfs:subClassOf <https://w3id.org/con-tax/zones/aat-buildingSites#300008187> ;
.
<https://w3id.org/con-tax/zones/aat-buildingSites#300065090>
  rdf:type owl:Class ;
  rdfs:comment "Buildings that house prisons having the highest level of security for dangerous inmates or those likely to escape."@en ;
  rdfs:isDefinedBy <https://w3id.org/con-tax/zones/aat-buildingSites> ;
  rdfs:label "ebi's"@nl ;
  rdfs:label "extra beveiligde inrichtingen"@nl ;
  rdfs:label "maximum-security prisons"@en ;
  rdfs:label "streng beveiligde gevangenis"@nl ;
  rdfs:label "streng beveiligde gevangenissen"@nl ;
  rdfs:seeAlso <http://vocab.getty.edu/aat/300065090> ;
  rdfs:subClassOf <https://w3id.org/con-tax/zones/aat-buildingSites#300006460> ;
.
<https://w3id.org/con-tax/zones/aat-buildingSites#300069806>
  rdf:type owl:Class ;
  rdfs:comment "Rooms in or attached to a horse barn or stable for the storage and maintenance of riding tack and often of stud records or for the display of prizes or other honors of the stable."@en ;
  rdfs:comment "Ruimten in of aan paardenstallen, voor de opslag en het onderhoud van zadels en tuig en waar vaak ook stoeterijgegevens, prijzen en ander eerbetoon aan de stoeterij worden bewaard."@nl ;
  rdfs:isDefinedBy <https://w3id.org/con-tax/zones/aat-buildingSites> ;
  rdfs:label "tack rooms"@en ;
  rdfs:label "zadelkamer"@nl ;
  rdfs:label "zadelkamers"@nl ;
  rdfs:seeAlso <http://vocab.getty.edu/aat/300069806> ;
  rdfs:subClassOf <https://w3id.org/con-tax/zones/aat-buildingSites#300262974> ;
.
<https://w3id.org/con-tax/zones/aat-buildingSites#300072250>
  rdf:type owl:Class ;
  rdfs:comment "Tracts set aside for recreation and located on land in contact with the sea, in submerged areas, along sea beds, or on emerged land areas near the sea coast."@en ;
  rdfs:comment "Wordt gebruikt voor allerlei gebieden die permanent worden beschermd. Hierbij kan het gaan om stukken land die in contact staan met de zee, maar ook om overstroomde gebieden, zeebeddingen of gebieden die dichtbij een kust zijn drooggevallen."@nl ;
  rdfs:isDefinedBy <https://w3id.org/con-tax/zones/aat-buildingSites> ;
  rdfs:label "mariene park"@nl ;
  rdfs:label "mariene parken"@nl ;
  rdfs:label "marine parks"@en ;
  rdfs:seeAlso <http://vocab.getty.edu/aat/300072250> ;
  rdfs:subClassOf <https://w3id.org/con-tax/zones/aat-buildingSites#300008187> ;
.
<https://w3id.org/con-tax/zones/aat-buildingSites#300108407>
  rdf:type owl:Class ;
  rdfs:comment "Distinguished from \"wild animal parks\" by the lack of restrictions on animal movement and by the mingling of animals and the visiting public, who generally drive through the parks in their own vehicles."@en ;
  rdfs:comment "Te onderscheiden van 'dierenparken' door het gebrek aan beperking van de bewegingsvrijheid van de dieren en door het samenbrengen van dieren en bezoekers, die meestal door de parken rijden in hun eigen voertuigen."@nl ;
  rdfs:isDefinedBy <https://w3id.org/con-tax/zones/aat-buildingSites> ;
  rdfs:label "safari parks"@en ;
  rdfs:label "safaripark"@nl ;
  rdfs:label "safariparken"@nl ;
  rdfs:label "wildparken"@nl ;
  rdfs:seeAlso <http://vocab.getty.edu/aat/300108407> ;
  rdfs:seeAlso wd:Q642682 ;
  rdfs:subClassOf <https://w3id.org/con-tax/zones/aat-buildingSites#300000354> ;
.
<https://w3id.org/con-tax/zones/aat-buildingSites#300111990>
  rdf:type owl:Class ;
  rdfs:comment "An alignment of at least five neolithic sites in less than ten miles."@en ;
  rdfs:comment "Een groepering van tenminste vijf neolithische vindplaatsen in een gebied van minder dan zestien kilometer."@nl ;
  rdfs:isDefinedBy <https://w3id.org/con-tax/zones/aat-buildingSites> ;
  rdfs:label "leys (archaeological sites)"@en ;
  rdfs:label "leys"@nl ;
  rdfs:seeAlso <http://vocab.getty.edu/aat/300111990> ;
  rdfs:subClassOf <https://w3id.org/con-tax/zones/aat-buildingSites#300000810> ;
.
<https://w3id.org/con-tax/zones/aat-buildingSites#300116926>
  rdf:type owl:Class ;
  rdfs:comment "Complexes designed as unified sites that include a mix of building types and uses, common open space, and controlled density increases, rather than lot-by-lot schemes."@en ;
  rdfs:comment "Wordt gebruikt voor complexen die zijn ontworpen als verenigde terreinen met verschillende soorten gebouwen, gemeenschappelijke open ruimten en waar de toename van de bevolkingsdichtheid wordt beheerst, in tegenstelling tot kavel-voor-kavel planning."@nl ;
  rdfs:isDefinedBy <https://w3id.org/con-tax/zones/aat-buildingSites> ;
  rdfs:label "collectief geïntegreerd ontwikkelingsproject"@nl ;
  rdfs:label "collectief geïntegreerde ontwikkelingsprojecten"@nl ;
  rdfs:label "planned unit developments"@en ;
  rdfs:seeAlso <http://vocab.getty.edu/aat/300116926> ;
  rdfs:subClassOf <https://w3id.org/con-tax/zones/aat-buildingSites#300259362> ;
.
<https://w3id.org/con-tax/zones/aat-buildingSites#300120676>
  rdf:type owl:Class ;
  rdfs:comment "Temporary and often spontaneously established, settlements of displaced peoples along borders of neighboring or nearby countries, generally having minimal shelter, supplies, and sanitary facilities and created without the granting of technical asylum."@en ;
  rdfs:comment "Wordt gebruikt voor tijdelijke, langs de grenzen van naburige landen , vaak spontaan opgerichte nederzettingen van vluchtelingen, die doorgaans  niet veel onderdak bieden, waar voorraden en sanitaire voorzieningen beperkt zijn en die zijn opgebouwd zonder dat er formeel asiel is verleend."@nl ;
  rdfs:isDefinedBy <https://w3id.org/con-tax/zones/aat-buildingSites> ;
  rdfs:label "refugee camps"@en ;
  rdfs:label "vluchtelingenkamp"@nl ;
  rdfs:label "vluchtelingenkampen"@nl ;
  rdfs:seeAlso <http://vocab.getty.edu/aat/300120676> ;
  rdfs:subClassOf <https://w3id.org/con-tax/zones/aat-buildingSites#300259362> ;
.
<https://w3id.org/con-tax/zones/aat-buildingSites#300120802>
  rdf:type owl:Class ;
  rdfs:comment "Complexes built for use related to water transportation. "@en ;
  rdfs:isDefinedBy <https://w3id.org/con-tax/zones/aat-buildingSites> ;
  rdfs:label "water transportation complexes"@en ;
  rdfs:label "watertransportcomplexen"@nl ;
  rdfs:seeAlso <http://vocab.getty.edu/aat/300120802> ;
  rdfs:seeAlso wd:Q21710839 ;
  rdfs:subClassOf <https://w3id.org/con-tax/zones/aat-buildingSites#300000677> ;
.
<https://w3id.org/con-tax/zones/aat-buildingSites#300120803>
  rdf:type owl:Class ;
  rdfs:comment "Spacious enclosures, usually adjoining a sea or river, in which ships are repaired or built, and where ships' stores are prepared or brought together. The term is often reserved for government establishments of this character."@en ;
  rdfs:isDefinedBy <https://w3id.org/con-tax/zones/aat-buildingSites> ;
  rdfs:label "dockyards"@en ;
  rdfs:label "haventerrein"@nl ;
  rdfs:label "haventerreinen"@nl ;
  rdfs:seeAlso <http://vocab.getty.edu/aat/300120803> ;
  rdfs:seeAlso wd:Q190928 ;
  rdfs:subClassOf <https://w3id.org/con-tax/zones/aat-buildingSites#300120802> ;
.
<https://w3id.org/con-tax/zones/aat-buildingSites#300120804>
  rdf:type owl:Class ;
  rdfs:comment "Watercraft complexes facilitating the operation of air-cushion vehicles."@en ;
  rdfs:comment "Wordt gebruikt voor havens die zijn uitgerust voor het gebruik van vaartuigen met luchtkussens."@nl ;
  rdfs:isDefinedBy <https://w3id.org/con-tax/zones/aat-buildingSites> ;
  rdfs:label "hovercrafthaven"@nl ;
  rdfs:label "hovercrafthavens"@nl ;
  rdfs:label "hoverports"@en ;
  rdfs:seeAlso <http://vocab.getty.edu/aat/300120804> ;
  rdfs:seeAlso wd:Q5917104 ;
  rdfs:subClassOf <https://w3id.org/con-tax/zones/aat-buildingSites#300120802> ;
.
<https://w3id.org/con-tax/zones/aat-buildingSites#300120824>
  rdf:type owl:Class ;
  rdfs:comment "Ligplaatsvoorzieningen voornamelijk voor kleine recreatievaartuigen."@nl ;
  rdfs:comment "Secure mooring facilities primarily for yachts and other recreational small craft."@en ;
  rdfs:isDefinedBy <https://w3id.org/con-tax/zones/aat-buildingSites> ;
  rdfs:label "jachthaven"@nl ;
  rdfs:label "jachthavens"@nl ;
  rdfs:label "marinas (water transportation complexes)"@en ;
  rdfs:seeAlso <http://vocab.getty.edu/aat/300120824> ;
  rdfs:seeAlso wd:Q721207 ;
  rdfs:subClassOf <https://w3id.org/con-tax/zones/aat-buildingSites#300120802> ;
.
<https://w3id.org/con-tax/zones/aat-buildingSites#300122216>
  rdf:type owl:Class ;
  rdfs:comment "Buildings or complexes where people are detained for various reasons."@en ;
  rdfs:isDefinedBy <https://w3id.org/con-tax/zones/aat-buildingSites> ;
  rdfs:label "detention complexes"@en ;
  rdfs:label "gevangeniscomplexen"@nl ;
  rdfs:seeAlso <http://vocab.getty.edu/aat/300122216> ;
  rdfs:subClassOf <https://w3id.org/con-tax/zones/aat-buildingSites#300000202> ;
.
<https://w3id.org/con-tax/zones/aat-buildingSites#300122445>
  rdf:type gvp:GuideTerm ;
  rdfs:isDefinedBy <https://w3id.org/con-tax/zones/aat-buildingSites> ;
  rdfs:label "<gevangenis naar vorm of functie>"@nl ;
  rdfs:label "<gevangenissen naar vorm of functie>"@nl ;
  rdfs:label "<prison buildings by form or function>"@en ;
  rdfs:label "gevangenis naar vorm of functie"@nl ;
  rdfs:label "gevangenissen naar vorm of functie"@nl ;
  rdfs:seeAlso <http://vocab.getty.edu/aat/300122445> ;
  contax:containsConcept <https://w3id.org/con-tax/zones/aat-buildingSites#300006466> ;
  contax:containsConcept <https://w3id.org/con-tax/zones/aat-buildingSites#300006477> ;
  contax:containsConcept <https://w3id.org/con-tax/zones/aat-buildingSites#300065090> ;
  contax:containsConcept <https://w3id.org/con-tax/zones/aat-buildingSites#300169231> ;
  contax:containsConcept <https://w3id.org/con-tax/zones/aat-buildingSites#300169239> ;
  contax:containsConcept <https://w3id.org/con-tax/zones/aat-buildingSites#300312257> ;
.
<https://w3id.org/con-tax/zones/aat-buildingSites#300125766>
  rdf:type owl:Class ;
  rdfs:comment "Buildings or complexes constructed for or serving agricultural purposes."@en ;
  rdfs:isDefinedBy <https://w3id.org/con-tax/zones/aat-buildingSites> ;
  rdfs:label "agricultural complexes"@en ;
  rdfs:label "landbouwcomplexen"@nl ;
  rdfs:seeAlso <http://vocab.getty.edu/aat/300125766> ;
  rdfs:seeAlso wd:Q21550355 ;
  rdfs:subClassOf <https://w3id.org/con-tax/zones/aat-buildingSites#300000202> ;
.
<https://w3id.org/con-tax/zones/aat-buildingSites#300126335>
  rdf:type owl:Class ;
  rdfs:comment "Complexes of shops, restaurants, kiosks, and pushcarts featuring music and other entertainment, generally built downtown to revitalize an urban center; coined in the 1970s."@en ;
  rdfs:comment "Wordt gebruikt voor complexen bestaande uit o.a. winkels, restaurants, kiosken en handkarren waarop amusement o.a. in de vorm van muziek gebracht wordt, meestal gebouwd in een binnenstad om een stadscentrum nieuw leven in te blazen; bedacht in de jaren zeventig."@nl ;
  rdfs:isDefinedBy <https://w3id.org/con-tax/zones/aat-buildingSites> ;
  rdfs:label "festival marketplaces"@en ;
  rdfs:label "uitgaanscentra"@nl ;
  rdfs:label "uitgaanscentrum"@nl ;
  rdfs:seeAlso <http://vocab.getty.edu/aat/300126335> ;
  rdfs:seeAlso wd:Q5445768 ;
  rdfs:subClassOf <https://w3id.org/con-tax/zones/aat-buildingSites#300000250> ;
.
<https://w3id.org/con-tax/zones/aat-buildingSites#300128200>
  rdf:type gvp:GuideTerm ;
  rdfs:isDefinedBy <https://w3id.org/con-tax/zones/aat-buildingSites> ;
  rdfs:label "<complexen naar ontwikkelingstraject>"@nl ;
  rdfs:label "<complexes by development practice>"@en ;
  rdfs:label "complexen naar ontwikkelingstraject"@nl ;
  rdfs:seeAlso <http://vocab.getty.edu/aat/300128200> ;
  contax:containsConcept <https://w3id.org/con-tax/zones/aat-buildingSites#300000500> ;
  contax:containsConcept <https://w3id.org/con-tax/zones/aat-buildingSites#300000506> ;
  contax:containsConcept <https://w3id.org/con-tax/zones/aat-buildingSites#300000508> ;
.
<https://w3id.org/con-tax/zones/aat-buildingSites#300132652>
  rdf:type owl:Class ;
  rdfs:comment "Buildings or complexes constructed for or serving businesses, merchants, and other commercial purposes."@en ;
  rdfs:isDefinedBy <https://w3id.org/con-tax/zones/aat-buildingSites> ;
  rdfs:label "commercial complexes"@en ;
  rdfs:label "commerciële complexen"@nl ;
  rdfs:seeAlso <http://vocab.getty.edu/aat/300132652> ;
  rdfs:subClassOf <https://w3id.org/con-tax/zones/aat-buildingSites#300000202> ;
.
<https://w3id.org/con-tax/zones/aat-buildingSites#300133150>
  rdf:type owl:Class ;
  rdfs:comment "Buildings housing institutions tasked to hold and detain members of the armed forces, in the U.S. particularly who have been convicted of violations of the Uniform Code of Military Justice."@en ;
  rdfs:comment "Instellingen die zijn bedoeld voor het in verzekerde bewaring stellen van leden van de krijgsmacht die zijn veroordeeld voor overtredingen van militaire wetten."@nl ;
  rdfs:isDefinedBy <https://w3id.org/con-tax/zones/aat-buildingSites> ;
  rdfs:label "militaire gevangenis"@nl ;
  rdfs:label "militaire gevangenissen"@nl ;
  rdfs:label "military prisons (buildings)"@en ;
  rdfs:seeAlso <http://vocab.getty.edu/aat/300133150> ;
  rdfs:seeAlso wd:Q683992 ;
  rdfs:subClassOf <https://w3id.org/con-tax/zones/aat-buildingSites#300006460> ;
.
<https://w3id.org/con-tax/zones/aat-buildingSites#300133154>
  rdf:type owl:Class ;
  rdfs:comment "Refers to open spaces, buildings, or other structures that are of historic or environmental significance and threatened with development or demolition."@en ;
  rdfs:comment "Wordt gebruikt voor doorgaans historische open ruimten, gebouwen of andere bouwwerken die worden bedreigd met sloop of waar nieuwbouwprojecten zijn gepland."@nl ;
  rdfs:isDefinedBy <https://w3id.org/con-tax/zones/aat-buildingSites> ;
  rdfs:label "bedreigde plaatsen"@nl ;
  rdfs:label "endangered places"@en ;
  rdfs:seeAlso <http://vocab.getty.edu/aat/300133154> ;
  rdfs:subClassOf <https://w3id.org/con-tax/zones/aat-buildingSites#300000809> ;
.
<https://w3id.org/con-tax/zones/aat-buildingSites#300137340>
  rdf:type owl:Class ;
  rdfs:comment "Locaties waar meestal erg verwoestende wapens tot ontploffing worden gebracht op een afstand van het waarnemingspunt; wordt ook gebruikt voor plaatsen waar wetenschappelijk veldonderzoek wordt uitgevoerd, zoals  bijvoorbeeld in de archeologie of geologie. Gebruik 'testterreinen' voor complexen waar wapens worden uitgetest onder scherp toezicht."@nl ;
  rdfs:comment "Locations where, usually very destructive, weapons are exploded distant from an observation point; also, where scientific field explorations or investigations are conducted, as in archaeology or geology. For complexes where weapons are tested under close scrutiny, use \"proving grounds.\""@en ;
  rdfs:isDefinedBy <https://w3id.org/con-tax/zones/aat-buildingSites> ;
  rdfs:label "proefterrein"@nl ;
  rdfs:label "proefterreinen"@nl ;
  rdfs:label "test sites"@en ;
  rdfs:seeAlso <http://vocab.getty.edu/aat/300137340> ;
  rdfs:subClassOf <https://w3id.org/con-tax/zones/aat-buildingSites#300000809> ;
.
<https://w3id.org/con-tax/zones/aat-buildingSites#300137343>
  rdf:type owl:Class ;
  rdfs:comment "Locations where nuclear devices are experimentally exploded."@en ;
  rdfs:comment "Wordt gebruikt voor locaties waar nucleaire ladignen tot ontploffing worden gebracht voor proefnemingen."@nl ;
  rdfs:isDefinedBy <https://w3id.org/con-tax/zones/aat-buildingSites> ;
  rdfs:label "kernproefterrein"@nl ;
  rdfs:label "kernproefterreinen"@nl ;
  rdfs:label "nuclear test sites"@en ;
  rdfs:seeAlso <http://vocab.getty.edu/aat/300137343> ;
  rdfs:subClassOf <https://w3id.org/con-tax/zones/aat-buildingSites#300137340> ;
.
<https://w3id.org/con-tax/zones/aat-buildingSites#300151282>
  rdf:type owl:Class ;
  rdfs:comment "Parks, usually over 20 acres in extent, offering a wider range of activities and considerably more open space than \"neighborhood parks.\""@en ;
  rdfs:comment "Te gebruiken voor parken, meestal groter dan 80.000 m2, met een grote verscheidenheid aan voorzieningen en aanmerkelijk meer open ruimte dan 'buurtparken'."@nl ;
  rdfs:isDefinedBy <https://w3id.org/con-tax/zones/aat-buildingSites> ;
  rdfs:label "community parks"@en ;
  rdfs:label "gemeenschapspark"@nl ;
  rdfs:label "gemeenschapsparken"@nl ;
  rdfs:seeAlso <http://vocab.getty.edu/aat/300151282> ;
  rdfs:subClassOf <https://w3id.org/con-tax/zones/aat-buildingSites#300008187> ;
.
<https://w3id.org/con-tax/zones/aat-buildingSites#300159932>
  rdf:type owl:Class ;
  rdfs:comment "Complexes of schools, usually ranging from kindergarten through high school or two-year college, that draw students from a metropolitan area and are intended to minimize the effects of segregation."@en ;
  rdfs:comment "Schoolcomplexen doorgaans bestaande uit een kleuter-, basis- en middelbare school, die leerlingen aantrekken uit een grootstedelijk gebied en die bedoeld zijn om de gevolgen van etnische scheiding te minimaliseren."@nl ;
  rdfs:isDefinedBy <https://w3id.org/con-tax/zones/aat-buildingSites> ;
  rdfs:label "educational park"@nl ;
  rdfs:label "educational parks"@en ;
  rdfs:label "educational parks"@nl ;
  rdfs:seeAlso <http://vocab.getty.edu/aat/300159932> ;
  rdfs:subClassOf <https://w3id.org/con-tax/zones/aat-buildingSites#300000330> ;
.
<https://w3id.org/con-tax/zones/aat-buildingSites#300161281>
  rdf:type owl:Class ;
  rdfs:comment "Relatively buildings or sets of buildings containing a relatively small number of retail units with interconnecting walkways, generally having only one or a small number of stories, often located outdoors in a suburban area, and typically arranged in a single row facing a shared parking lot. For larger, more elaborate structures housing a larger number of retail units, often under a roof with indoor walkways, use \"shopping malls.\""@en ;
  rdfs:isDefinedBy <https://w3id.org/con-tax/zones/aat-buildingSites> ;
  rdfs:label "overdekt winkelcentrum"@nl ;
  rdfs:label "overdekte winkelcentra"@nl ;
  rdfs:label "shopping plazas"@en ;
  rdfs:seeAlso <http://vocab.getty.edu/aat/300161281> ;
  rdfs:subClassOf <https://w3id.org/con-tax/zones/aat-buildingSites#300005268> ;
.
<https://w3id.org/con-tax/zones/aat-buildingSites#300164060>
  rdf:type owl:Class ;
  rdfs:comment "Areas reserved for the training and rapid deployment of military forces."@en ;
  rdfs:isDefinedBy <https://w3id.org/con-tax/zones/aat-buildingSites> ;
  rdfs:label "militaire vestiging"@nl ;
  rdfs:label "militaire vestigingen"@nl ;
  rdfs:label "military installations"@en ;
  rdfs:seeAlso <http://vocab.getty.edu/aat/300164060> ;
  rdfs:subClassOf <https://w3id.org/con-tax/zones/aat-buildingSites#300000202> ;
.
<https://w3id.org/con-tax/zones/aat-buildingSites#300164113>
  rdf:type owl:Class ;
  rdfs:comment "Military training camps for new recruits, where intensive and harshly disciplined training is carried out. Originally the term referred to United States Marine Corps training, but is extended to any United States Military initial training camp."@en ;
  rdfs:isDefinedBy <https://w3id.org/con-tax/zones/aat-buildingSites> ;
  rdfs:label "boot camps"@en ;
  rdfs:label "opleidingskamp voor mariniers"@nl ;
  rdfs:label "opleidingskampen voor mariniers"@nl ;
  rdfs:seeAlso <http://vocab.getty.edu/aat/300164113> ;
  rdfs:subClassOf <https://w3id.org/con-tax/zones/aat-buildingSites#300000465> ;
.
<https://w3id.org/con-tax/zones/aat-buildingSites#300164117>
  rdf:type owl:Class ;
  rdfs:comment "Military camps where army soldiers are stationed when training for, or fighting, a war. "@en ;
  rdfs:isDefinedBy <https://w3id.org/con-tax/zones/aat-buildingSites> ;
  rdfs:label "army camps"@en ;
  rdfs:label "legerkamp"@nl ;
  rdfs:label "legerkampen"@nl ;
  rdfs:seeAlso <http://vocab.getty.edu/aat/300164117> ;
  rdfs:subClassOf <https://w3id.org/con-tax/zones/aat-buildingSites#300000476> ;
.
<https://w3id.org/con-tax/zones/aat-buildingSites#300168612>
  rdf:type gvp:GuideTerm ;
  rdfs:isDefinedBy <https://w3id.org/con-tax/zones/aat-buildingSites> ;
  rdfs:label "<gevangenissen naar beheer>"@nl ;
  rdfs:label "<prison buildings by administration>"@en ;
  rdfs:label "gevangenissen naar beheer"@nl ;
  rdfs:seeAlso <http://vocab.getty.edu/aat/300168612> ;
  contax:containsConcept <https://w3id.org/con-tax/zones/aat-buildingSites#300006479> ;
  contax:containsConcept <https://w3id.org/con-tax/zones/aat-buildingSites#300006481> ;
  contax:containsConcept <https://w3id.org/con-tax/zones/aat-buildingSites#300133150> ;
.
<https://w3id.org/con-tax/zones/aat-buildingSites#300169222>
  rdf:type owl:Class ;
  rdfs:comment "Aanduiding voor lokale huizen van bewaring voor armen, zwervers of mensen die op hun rechtszaak wachten; werden gebruikt in Groot-Brittannië tussen de 11e en de 18e eeuw. Geen Nederlands equivalent. Zie 'huizen van bewaring'."@nl ;
  rdfs:comment "Buildings that house local places of detention for the poor, vagrants, or those awaiting trial; usually spefically for such structures used in Britain between the 11th and 18th centuries."@en ;
  rdfs:isDefinedBy <https://w3id.org/con-tax/zones/aat-buildingSites> ;
  rdfs:label "gaol"@nl ;
  rdfs:label "gaols"@en ;
  rdfs:label "gaols"@nl ;
  rdfs:seeAlso <http://vocab.getty.edu/aat/300169222> ;
  rdfs:seeAlso wd:Q40357 ;
  rdfs:subClassOf <https://w3id.org/con-tax/zones/aat-buildingSites#300006457> ;
.
<https://w3id.org/con-tax/zones/aat-buildingSites#300169231>
  rdf:type owl:Class ;
  rdfs:comment "Buildings that house prisons that house primarily non-violent offenders; the term is often used in the U.S. prison system."@en ;
  rdfs:isDefinedBy <https://w3id.org/con-tax/zones/aat-buildingSites> ;
  rdfs:label "halfopen inrichting"@nl ;
  rdfs:label "halfopen inrichtingen"@nl ;
  rdfs:label "minimum-security prisons"@en ;
  rdfs:seeAlso <http://vocab.getty.edu/aat/300169231> ;
  rdfs:subClassOf <https://w3id.org/con-tax/zones/aat-buildingSites#300006460> ;
.
<https://w3id.org/con-tax/zones/aat-buildingSites#300169239>
  rdf:type owl:Class ;
  rdfs:comment "Buildings that house prisons where the security level is less than maximum security; the inmates may sleep in dormitories and have other communal facilities, with generally less supervision over the internal movements than in a maximum-security prison."@en ;
  rdfs:isDefinedBy <https://w3id.org/con-tax/zones/aat-buildingSites> ;
  rdfs:label "gesloten inrichting"@nl ;
  rdfs:label "gesloten inrichtingen"@nl ;
  rdfs:label "medium-security prisons"@en ;
  rdfs:seeAlso <http://vocab.getty.edu/aat/300169239> ;
  rdfs:subClassOf <https://w3id.org/con-tax/zones/aat-buildingSites#300006460> ;
.
<https://w3id.org/con-tax/zones/aat-buildingSites#300169247>
  rdf:type owl:Class ;
  rdfs:comment "Buildings that house temporary holding places, as in police stations or courthouses, for persons awaiting trials or hearings; for shorter periods of confinement than jails."@en ;
  rdfs:comment "Wordt gebruikt voor tijdelijke plaatsen van bewaring, bijvoorbeeld op politiebureaus of in gerechtsgebouwen, voor mensen die op een rechtszaak of een hoorzitting wachten; wordt gebruikt voor kortere opsluitingen dan gevangenissen."@nl ;
  rdfs:isDefinedBy <https://w3id.org/con-tax/zones/aat-buildingSites> ;
  rdfs:label "arrestantenhokken"@nl ;
  rdfs:label "arrestantenlokaal"@nl ;
  rdfs:label "arrestantenlokalen"@nl ;
  rdfs:label "cachotten"@nl ;
  rdfs:label "lockups"@en-us ;
  rdfs:seeAlso <http://vocab.getty.edu/aat/300169247> ;
  rdfs:subClassOf <https://w3id.org/con-tax/zones/aat-buildingSites#300006448> ;
.
<https://w3id.org/con-tax/zones/aat-buildingSites#300178783>
  rdf:type owl:Class ;
  rdfs:comment "A type of small communal housing development, designed and managed by the occupants, in which each resident family owns a home and shares with the group common facilities, such as kitchens, child care centers, and laundry rooms, and their associated tasks. The modern method of cohousing originated in Denmark in the 1960s."@en ;
  rdfs:comment "Een project met kleine gemeenschapshuizen die worden ontworpen en beheerd door de bewoners, waarbij iedere inwonende familie een eigen woning heeft en gebruikt maakt van de gemeenschappelijke voorzieningen, zoals keukens, kinderopvang en wasmachines en iedereen een deel van de bijbehorende taken verricht."@nl ;
  rdfs:isDefinedBy <https://w3id.org/con-tax/zones/aat-buildingSites> ;
  rdfs:label "cohousing"@en ;
  rdfs:label "woongemeenschappen"@nl ;
  rdfs:label "woongroep"@nl ;
  rdfs:label "woongroepen"@nl ;
  rdfs:seeAlso <http://vocab.getty.edu/aat/300178783> ;
  rdfs:seeAlso wd:Q1107167 ;
  rdfs:subClassOf <https://w3id.org/con-tax/zones/aat-buildingSites#300259362> ;
.
<https://w3id.org/con-tax/zones/aat-buildingSites#300188636>
  rdf:type owl:Class ;
  rdfs:comment "Power plants that simultaneously generate from the same source electrical energy and useful heat energy."@en ;
  rdfs:comment "Wordt gebruikt voor elektriciteitscentrales die uit een en dezelfde bron zowel elektriciteit als bruikbare warmte-energie opwekken."@nl ;
  rdfs:isDefinedBy <https://w3id.org/con-tax/zones/aat-buildingSites> ;
  rdfs:label "cogeneration plants"@en-us ;
  rdfs:label "warmtekrachtcentrale"@nl ;
  rdfs:label "warmtekrachtcentrales"@nl ;
  rdfs:seeAlso <http://vocab.getty.edu/aat/300188636> ;
  rdfs:subClassOf <https://w3id.org/con-tax/zones/aat-buildingSites#300000414> ;
.
<https://w3id.org/con-tax/zones/aat-buildingSites#300195087>
  rdf:type owl:Class ;
  rdfs:comment "Aquatic recreation facilities with attractions based on fast-moving, rather than static, water."@en ;
  rdfs:comment "Voorzieningen voor waterrecreatie met attracties die zijn gebaseerd op snelstromend water, in plaats van stilstaand water."@nl ;
  rdfs:isDefinedBy <https://w3id.org/con-tax/zones/aat-buildingSites> ;
  rdfs:label "waterparks"@en ;
  rdfs:label "waterrecreatiepark"@nl ;
  rdfs:label "waterrecreatieparken"@nl ;
  rdfs:seeAlso <http://vocab.getty.edu/aat/300195087> ;
  rdfs:subClassOf <https://w3id.org/con-tax/zones/aat-buildingSites#300000515> ;
.
<https://w3id.org/con-tax/zones/aat-buildingSites#300199033>
  rdf:type owl:Class ;
  rdfs:comment "Farms primarily engaged in the keeping, feeding, or breeding of horses for by-products, livestock increase, or investment."@en ;
  rdfs:comment "Gebruik voor boerderijen die zich voornamelijk bezighouden met het houden, voeden, of het fokken van paarden voor bij-producten, toename van de veestapel, of als investering."@nl ;
  rdfs:isDefinedBy <https://w3id.org/con-tax/zones/aat-buildingSites> ;
  rdfs:label "horse farms"@en ;
  rdfs:label "paardenfokkerij"@nl ;
  rdfs:label "paardenfokkerijen"@nl ;
  rdfs:label "stoeterij"@nl ;
  rdfs:label "stoeterijen"@nl ;
  rdfs:seeAlso <http://vocab.getty.edu/aat/300199033> ;
  rdfs:subClassOf <https://w3id.org/con-tax/zones/aat-buildingSites#300000206> ;
.
<https://w3id.org/con-tax/zones/aat-buildingSites#300203159>
  rdf:type owl:Class ;
  rdfs:comment "Recreation complexes that are meeting places for associations."@en ;
  rdfs:isDefinedBy <https://w3id.org/con-tax/zones/aat-buildingSites> ;
  rdfs:label "club complexes"@en ;
  rdfs:label "sportterreinen"@nl ;
  rdfs:seeAlso <http://vocab.getty.edu/aat/300203159> ;
  rdfs:subClassOf <https://w3id.org/con-tax/zones/aat-buildingSites#300000510> ;
.
<https://w3id.org/con-tax/zones/aat-buildingSites#300229352>
  rdf:type owl:Class ;
  rdfs:comment "Sites located under water, including both those that have been flooded and those that were originally underwater."@en ;
  rdfs:comment "Wordt gebruikt voor locaties die zich onder water bevinden."@nl ;
  rdfs:isDefinedBy <https://w3id.org/con-tax/zones/aat-buildingSites> ;
  rdfs:label "onderwaterlocatie"@nl ;
  rdfs:label "onderwaterlocaties"@nl ;
  rdfs:label "underwater sites"@en ;
  rdfs:seeAlso <http://vocab.getty.edu/aat/300229352> ;
  rdfs:subClassOf <https://w3id.org/con-tax/zones/aat-buildingSites#300000809> ;
.
<https://w3id.org/con-tax/zones/aat-buildingSites#300229359>
  rdf:type owl:Class ;
  rdfs:comment "Sites located under bodies of salt water, particularly in oceans or seas."@en ;
  rdfs:comment "Wordt gebruikt voor locaties die zich onder zout water bevinden."@nl ;
  rdfs:isDefinedBy <https://w3id.org/con-tax/zones/aat-buildingSites> ;
  rdfs:label "mariene locatie"@nl ;
  rdfs:label "mariene locaties"@nl ;
  rdfs:label "marine sites"@en ;
  rdfs:seeAlso <http://vocab.getty.edu/aat/300229359> ;
  rdfs:subClassOf <https://w3id.org/con-tax/zones/aat-buildingSites#300229352> ;
.
<https://w3id.org/con-tax/zones/aat-buildingSites#300235049>
  rdf:type owl:Class ;
  rdfs:comment "Industrial parks whose facilities are devoted primarily to research and development."@en ;
  rdfs:comment "Industrieparken waarvan de faciliteiten in de eerste plaats zijn bedoeld voor onderzoek en ontwikkeling."@nl ;
  rdfs:isDefinedBy <https://w3id.org/con-tax/zones/aat-buildingSites> ;
  rdfs:label "research parks"@en ;
  rdfs:label "researchcentra (industrieparken)"@nl ;
  rdfs:label "researchcentra"@nl ;
  rdfs:label "researchcentrum (industriepark)"@nl ;
  rdfs:label "researchcentrum"@nl ;
  rdfs:seeAlso <http://vocab.getty.edu/aat/300235049> ;
  rdfs:subClassOf <https://w3id.org/con-tax/zones/aat-buildingSites#300000411> ;
.
<https://w3id.org/con-tax/zones/aat-buildingSites#300235959>
  rdf:type owl:Class ;
  rdfs:comment "Resorts specializing primarily in snow skiing."@en ;
  rdfs:comment "Wintersportcentra waar men zich vooral richt op skiën."@nl ;
  rdfs:isDefinedBy <https://w3id.org/con-tax/zones/aat-buildingSites> ;
  rdfs:label "ski resorts"@en ;
  rdfs:label "skigebied"@nl ;
  rdfs:label "skigebieden"@nl ;
  rdfs:seeAlso <http://vocab.getty.edu/aat/300235959> ;
  rdfs:seeAlso wd:Q130003 ;
  rdfs:subClassOf <https://w3id.org/con-tax/zones/aat-buildingSites#300000559> ;
.
<https://w3id.org/con-tax/zones/aat-buildingSites#300248842>
  rdf:type owl:Class ;
  rdfs:comment "Farms of wealthy landlords employing the latest and best agricultural techniques and technologies and designed by architects, often built as exemplars for local farmers; found, especially in England, from the late 18th century to the mid-19th century."@en ;
  rdfs:comment "Wordt gebruikt voor boerderijen van rijke landheren die de nieuwste en beste agrarische technieken en technologieën gebruiken, vaak gebouwd als voorbeeld voor plaatselijke boeren; kwam onder andere veel voor in de eerste helft van de 19e eeuw in Engeland."@nl ;
  rdfs:isDefinedBy <https://w3id.org/con-tax/zones/aat-buildingSites> ;
  rdfs:label "model farms"@en ;
  rdfs:label "modelboerderij"@nl ;
  rdfs:label "modelboerderijen"@nl ;
  rdfs:seeAlso <http://vocab.getty.edu/aat/300248842> ;
  rdfs:subClassOf <https://w3id.org/con-tax/zones/aat-buildingSites#300000206> ;
.
<https://w3id.org/con-tax/zones/aat-buildingSites#300250994>
  rdf:type owl:Class ;
  rdfs:comment "Recreation complexes where golf is played, comprising golf courses, clubhouses, and associated facilities and often restricting use to members."@en ;
  rdfs:comment "Wordt gebruikt voor recreatiecomplexen waar golf wordt gespeeld, bestaande uit golfterreinen, clubhuizen en aanverwante faciliteiten; vaak alleen toegankelijk voor leden."@nl ;
  rdfs:isDefinedBy <https://w3id.org/con-tax/zones/aat-buildingSites> ;
  rdfs:label "golf clubs (built complexes)"@en ;
  rdfs:label "golfterrein"@nl ;
  rdfs:label "golfterreinen"@nl ;
  rdfs:seeAlso <http://vocab.getty.edu/aat/300250994> ;
  rdfs:subClassOf <https://w3id.org/con-tax/zones/aat-buildingSites#300203159> ;
.
<https://w3id.org/con-tax/zones/aat-buildingSites#300252504>
  rdf:type owl:Class ;
  rdfs:comment "Large, multistory, multiroom complex dwellings of the Ancestral Puebloan and Hohokam periods, mostly dating from 950 to 1150 CE; distinguished from \"pueblos (housing complexes)\" by their often D-shaped outline, cohesive planned design, and location in the San Juan Basin, New Mexico, and parts of Arizona."@en ;
  rdfs:comment "Wordt gebruikt voor grote wooncomplexen met meerdere verdiepingen en meerdere vertrekken uit de Anasazi en Hohokam-tijdperken; zijn voornamelijk gebouwd in de periode tussen 950 en 1150 en zijn te onderscheiden van 'pueblo's' door hun vaak D-vormige omtrek, het samenhangend ontwerp en de ligging in het San Juan Basin, Nieuw Mexico en delen van Arizona."@nl ;
  rdfs:isDefinedBy <https://w3id.org/con-tax/zones/aat-buildingSites> ;
  rdfs:label "Great House"@nl ;
  rdfs:label "Great Houses (Amerindian complexes)"@en ;
  rdfs:label "Great Houses"@nl ;
  rdfs:seeAlso <http://vocab.getty.edu/aat/300252504> ;
  rdfs:subClassOf <https://w3id.org/con-tax/zones/aat-buildingSites#300259362> ;
.
<https://w3id.org/con-tax/zones/aat-buildingSites#300253565>
  rdf:type owl:Class ;
  rdfs:comment "Ranches dedicated primarly to raising horses."@en ;
  rdfs:isDefinedBy <https://w3id.org/con-tax/zones/aat-buildingSites> ;
  rdfs:label "horse ranches"@en ;
  rdfs:seeAlso <http://vocab.getty.edu/aat/300253565> ;
  rdfs:subClassOf <https://w3id.org/con-tax/zones/aat-buildingSites#300000241> ;
.
<https://w3id.org/con-tax/zones/aat-buildingSites#300253567>
  rdf:type owl:Class ;
  rdfs:comment "Out-of-town shopping developments, usually containing a number of large chain stores."@en ;
  rdfs:isDefinedBy <https://w3id.org/con-tax/zones/aat-buildingSites> ;
  rdfs:label "retail parks"@en ;
  rdfs:seeAlso <http://vocab.getty.edu/aat/300253567> ;
  rdfs:subClassOf <https://w3id.org/con-tax/zones/aat-buildingSites#300132652> ;
.
<https://w3id.org/con-tax/zones/aat-buildingSites#300257640>
  rdf:type owl:Class ;
  rdfs:comment "Kustcomplexen waarin walvissen worden verwerkt, bestaande uit voorzieningen voor het verwerken en verblijven voor de arbeiders. Gebruik voor de vaartuigen bij de verwerking van de walvissen op zee \"fabrieksschepen\"."@nl ;
  rdfs:comment "Shore complexes to which whales are taken for processing, consisting of processing facilities and quarters for the workers. For the watercraft used in the processing of whales at sea, use \"factory ships.\""@en ;
  rdfs:isDefinedBy <https://w3id.org/con-tax/zones/aat-buildingSites> ;
  rdfs:label "walvisstation"@nl ;
  rdfs:label "walvisstations"@nl ;
  rdfs:label "whaling stations"@en ;
  rdfs:seeAlso <http://vocab.getty.edu/aat/300257640> ;
  rdfs:seeAlso wd:Q3497366 ;
  rdfs:subClassOf <https://w3id.org/con-tax/zones/aat-buildingSites#300000385> ;
.
<https://w3id.org/con-tax/zones/aat-buildingSites#300259288>
  rdf:type owl:Class ;
  rdfs:comment "Discrete housing complexes closed off to nonresidents by gates and fences or walls; may or may not also have guards or other surveillance and security installations."@en ;
  rdfs:comment "Te gebruiken voor wooncomplexen die voor niet-bewoners zijn afgesloten met hekken of muren voorzien van toegangspoorten; zijn soms ook voorzien van bewakers of andere vormen van surveillance en beveiliging."@nl ;
  rdfs:isDefinedBy <https://w3id.org/con-tax/zones/aat-buildingSites> ;
  rdfs:label "gated communities"@en ;
  rdfs:label "gated community's"@nl ;
  rdfs:seeAlso <http://vocab.getty.edu/aat/300259288> ;
  rdfs:seeAlso wd:Q75848 ;
  rdfs:subClassOf <https://w3id.org/con-tax/zones/aat-buildingSites#300259362> ;
.
<https://w3id.org/con-tax/zones/aat-buildingSites#300259362>
  rdf:type owl:Class ;
  rdfs:comment "Buildings or complexes providing housing and related facilities."@en ;
  rdfs:comment "Gebouwen of complexen die huisvesting en gerelateerde faciliteiten bieden."@nl ;
  rdfs:isDefinedBy <https://w3id.org/con-tax/zones/aat-buildingSites> ;
  rdfs:label "housing complexes"@en ;
  rdfs:label "huisvestingscomplexen"@nl ;
  rdfs:seeAlso <http://vocab.getty.edu/aat/300259362> ;
  rdfs:subClassOf <https://w3id.org/con-tax/zones/aat-buildingSites#300000202> ;
  contax:containsGuideTerm <https://w3id.org/con-tax/zones/aat-buildingSites#300259363> ;
  contax:containsGuideTerm <https://w3id.org/con-tax/zones/aat-buildingSites#300259364> ;
  contax:containsGuideTerm <https://w3id.org/con-tax/zones/aat-buildingSites#300259365> ;
  contax:containsGuideTerm <https://w3id.org/con-tax/zones/aat-buildingSites#300259366> ;
  contax:containsGuideTerm <https://w3id.org/con-tax/zones/aat-buildingSites#300259367> ;
.
<https://w3id.org/con-tax/zones/aat-buildingSites#300259363>
  rdf:type gvp:GuideTerm ;
  rdfs:isDefinedBy <https://w3id.org/con-tax/zones/aat-buildingSites> ;
  rdfs:label "<housing complexes by form>"@en ;
  rdfs:label "<huisvestingscomplexen naar vorm>"@nl ;
  rdfs:label "huisvestingscomplexen naar vorm"@nl ;
  rdfs:seeAlso <http://vocab.getty.edu/aat/300259363> ;
  contax:containsConcept <https://w3id.org/con-tax/zones/aat-buildingSites#300000291> ;
  contax:containsConcept <https://w3id.org/con-tax/zones/aat-buildingSites#300000329> ;
  contax:containsConcept <https://w3id.org/con-tax/zones/aat-buildingSites#300252504> ;
  contax:containsConcept <https://w3id.org/con-tax/zones/aat-buildingSites#300264006> ;
.
<https://w3id.org/con-tax/zones/aat-buildingSites#300259364>
  rdf:type gvp:GuideTerm ;
  rdfs:isDefinedBy <https://w3id.org/con-tax/zones/aat-buildingSites> ;
  rdfs:label "<housing complexes by function>"@en ;
  rdfs:label "<huisvestingscomplexen naar functie>"@nl ;
  rdfs:label "huisvestingscomplexen naar functie"@nl ;
  rdfs:seeAlso <http://vocab.getty.edu/aat/300259364> ;
  contax:containsConcept <https://w3id.org/con-tax/zones/aat-buildingSites#300000300> ;
  contax:containsConcept <https://w3id.org/con-tax/zones/aat-buildingSites#300000410> ;
.
<https://w3id.org/con-tax/zones/aat-buildingSites#300259365>
  rdf:type gvp:GuideTerm ;
  rdfs:isDefinedBy <https://w3id.org/con-tax/zones/aat-buildingSites> ;
  rdfs:label "<housing complexes by development practice>"@en ;
  rdfs:label "<huisvestingscomplexen naar ontwikkelingstraject>"@nl ;
  rdfs:label "huisvestingscomplexen naar ontwikkelingstraject"@nl ;
  rdfs:seeAlso <http://vocab.getty.edu/aat/300259365> ;
  contax:containsConcept <https://w3id.org/con-tax/zones/aat-buildingSites#300000307> ;
  contax:containsConcept <https://w3id.org/con-tax/zones/aat-buildingSites#300000326> ;
  contax:containsConcept <https://w3id.org/con-tax/zones/aat-buildingSites#300000498> ;
  contax:containsConcept <https://w3id.org/con-tax/zones/aat-buildingSites#300116926> ;
  contax:containsConcept <https://w3id.org/con-tax/zones/aat-buildingSites#300259288> ;
.
<https://w3id.org/con-tax/zones/aat-buildingSites#300259366>
  rdf:type gvp:GuideTerm ;
  rdfs:isDefinedBy <https://w3id.org/con-tax/zones/aat-buildingSites> ;
  rdfs:label "<housing complexes by occupants>"@en ;
  rdfs:label "<huisvestingscomplexen naar bewoners>"@nl ;
  rdfs:label "huisvestingscomplexen naar bewoners"@nl ;
  rdfs:seeAlso <http://vocab.getty.edu/aat/300259366> ;
  contax:containsConcept <https://w3id.org/con-tax/zones/aat-buildingSites#300000592> ;
  contax:containsConcept <https://w3id.org/con-tax/zones/aat-buildingSites#300120676> ;
.
<https://w3id.org/con-tax/zones/aat-buildingSites#300259367>
  rdf:type gvp:GuideTerm ;
  rdfs:isDefinedBy <https://w3id.org/con-tax/zones/aat-buildingSites> ;
  rdfs:label "<housing complexes by ownership>"@en ;
  rdfs:label "<huisvestingscomplexen naar eigenaar>"@nl ;
  rdfs:label "huisvestingscomplexen naar eigenaar"@nl ;
  rdfs:seeAlso <http://vocab.getty.edu/aat/300259367> ;
  contax:containsConcept <https://w3id.org/con-tax/zones/aat-buildingSites#300000319> ;
  contax:containsConcept <https://w3id.org/con-tax/zones/aat-buildingSites#300178783> ;
  contax:containsConcept <https://w3id.org/con-tax/zones/aat-buildingSites#300404837> ;
.
<https://w3id.org/con-tax/zones/aat-buildingSites#300259534>
  rdf:type owl:Class ;
  rdfs:comment "Places where residential garbage and commercial wastes are collected, compacted, or baled for transport to a processing facility or landfill; may be fixed or mobile."@en ;
  rdfs:comment "Te gebruiken voor punten waar huishoudelijk en industrieel afval wordt verzameld, samengeperst of in balen verpakt voor vervoer naar een verwerkingsinstallatie of stortplaats; kunnen vast of mobiel zijn."@nl ;
  rdfs:isDefinedBy <https://w3id.org/con-tax/zones/aat-buildingSites> ;
  rdfs:label "overslagstations"@nl ;
  rdfs:label "transfer stations"@en ;
  rdfs:seeAlso <http://vocab.getty.edu/aat/300259534> ;
  rdfs:seeAlso wd:Q1147171 ;
  rdfs:subClassOf <https://w3id.org/con-tax/zones/aat-buildingSites#300000809> ;
.
<https://w3id.org/con-tax/zones/aat-buildingSites#300260689>
  rdf:type owl:Class ;
  rdfs:comment "Sites considered for development that already have some form of development on them or that are derelict and thus would require clearance before redevelopment could take place."@en ;
  rdfs:comment "Te gebruiken voor terreinen die in aanmerking komen voor bebouwing maar waarop al enige vorm van ontwikkeling heeft plaatsgevonden of die vervallen zijn, zodat er eerst moet worden ontruimd of gesloopt voordat nieuwbouw kan plaatsvinden."@nl ;
  rdfs:isDefinedBy <https://w3id.org/con-tax/zones/aat-buildingSites> ;
  rdfs:label "brownfield sites"@en ;
  rdfs:label "inbreidingsgebied"@nl ;
  rdfs:seeAlso <http://vocab.getty.edu/aat/300260689> ;
  rdfs:seeAlso wd:Q896586 ;
  rdfs:subClassOf <https://w3id.org/con-tax/zones/aat-buildingSites#300000809> ;
.
<https://w3id.org/con-tax/zones/aat-buildingSites#300262710>
  rdf:type owl:Class ;
  rdfs:comment "Complexen die meestal een huis van bewaring, een politiebureau en een rechtbank omvatten, waar diensten worden verleend zoals educatieve en behandelprogramma's ter verbetering van delinquenten."@nl ;
  rdfs:comment "Complexes typically comprising a jail, police station, and courthouse, which provide services such as educational classes and treatment programs as means of reform."@en ;
  rdfs:isDefinedBy <https://w3id.org/con-tax/zones/aat-buildingSites> ;
  rdfs:label "justice centers"@en ;
  rdfs:label "justitiële centra"@nl ;
  rdfs:seeAlso <http://vocab.getty.edu/aat/300262710> ;
  rdfs:subClassOf <https://w3id.org/con-tax/zones/aat-buildingSites#300000202> ;
.
<https://w3id.org/con-tax/zones/aat-buildingSites#300262766>
  rdf:type owl:Class ;
  rdfs:comment "Buildings that house justice centers used for the custody and treatment of juvenile offenders."@en ;
  rdfs:comment "Justitiële centra die worden gebruikt voor de verzekerde bewaring en behandeling van jeugddelinquenten."@nl ;
  rdfs:isDefinedBy <https://w3id.org/con-tax/zones/aat-buildingSites> ;
  rdfs:label "justitiële jeugdcentra"@nl ;
  rdfs:label "juvenile justice centers"@en ;
  rdfs:seeAlso <http://vocab.getty.edu/aat/300262766> ;
  rdfs:subClassOf <https://w3id.org/con-tax/zones/aat-buildingSites#300006448> ;
  rdfs:subClassOf <https://w3id.org/con-tax/zones/aat-buildingSites#300006453> ;
  rdfs:subClassOf <https://w3id.org/con-tax/zones/aat-buildingSites#300262710> ;
.
<https://w3id.org/con-tax/zones/aat-buildingSites#300262911>
  rdf:type owl:Class ;
  rdfs:comment "Complexen bestaande uit een vuurtoren en verschillende bijgebouwen en constructies, zoals verblijven voor wachters, boothuizen, rooksignaalinstallaties, waterreservoirs en werkplaatsen."@nl ;
  rdfs:comment "Complexes consisting of a light house and various support buildings and structures, such as keepers quarters, boathouses, fog signals, cisterns, and workshops."@en ;
  rdfs:isDefinedBy <https://w3id.org/con-tax/zones/aat-buildingSites> ;
  rdfs:label "light stations"@en ;
  rdfs:label "vuurtorencomplexen"@nl ;
  rdfs:seeAlso <http://vocab.getty.edu/aat/300262911> ;
  rdfs:seeAlso wd:Q27193297 ;
  rdfs:subClassOf <https://w3id.org/con-tax/zones/aat-buildingSites#300120802> ;
.
<https://w3id.org/con-tax/zones/aat-buildingSites#300262974>
  rdf:type owl:Class ;
  rdfs:comment "Faciliteiten voor training, onderdak en zorg voor ruitersporters, meestal met renbanen, schuren, stallen en dierenhospitalen. Gebruik 'ruiterscholen' voor scholen waar de ruiterkunst wordt onderwezen."@nl ;
  rdfs:comment "Facilities offering equestrian training, board, and care, typically comprising race tracks, barns, stables, and veterinary hospitals. For schools where equitation is taught, use \"riding schools.\""@en ;
  rdfs:isDefinedBy <https://w3id.org/con-tax/zones/aat-buildingSites> ;
  rdfs:label "equestrian centers"@en-us ;
  rdfs:label "hippisch centrum"@nl ;
  rdfs:label "hippische centra"@nl ;
  rdfs:label "ruitersportcentra"@nl ;
  rdfs:label "ruitersportcentrum"@nl ;
  rdfs:seeAlso <http://vocab.getty.edu/aat/300262974> ;
  rdfs:subClassOf <https://w3id.org/con-tax/zones/aat-buildingSites#300000560> ;
.
<https://w3id.org/con-tax/zones/aat-buildingSites#300263063>
  rdf:type owl:Class ;
  rdfs:comment "Entities, including a site, building, city, complex, desert, forest, island, lake, monument, or mountain designated by the United Nations Educational, Scientific and Cultural Organization (UNESCO) as exceptional examples of cultural values or natural phenomena."@en ;
  rdfs:comment "Locaties die zijn aangewezen door de United Nations Educational, Scientific and Cultural Organization (UNESCO), als uitzonderlijke voorbeelden van culturele waarden of natuurlijke fenomenen."@nl ;
  rdfs:isDefinedBy <https://w3id.org/con-tax/zones/aat-buildingSites> ;
  rdfs:label "Werelderfgoedsite"@nl ;
  rdfs:label "Werelderfgoedsites"@nl ;
  rdfs:label "World Heritage Sites"@en ;
  rdfs:seeAlso <http://vocab.getty.edu/aat/300263063> ;
  rdfs:seeAlso wd:Q9259 ;
  rdfs:subClassOf <https://w3id.org/con-tax/zones/aat-buildingSites#300000809> ;
.
<https://w3id.org/con-tax/zones/aat-buildingSites#300263166>
  rdf:type owl:Class ;
  rdfs:comment "Outdoor trails equipped with a series of stations where joggers or walkers stop and perform exercises on the apparatus provided."@en ;
  rdfs:comment "Paden in de buitenlucht die zijn voorzien van een aantal haltes, waar joggers of wandelaars oefeningen kunnen uitvoeren met het beschikbare toestel."@nl ;
  rdfs:isDefinedBy <https://w3id.org/con-tax/zones/aat-buildingSites> ;
  rdfs:label "fitness trails"@en ;
  rdfs:label "fitness-circuits"@nl ;
  rdfs:label "fitness-parcours"@nl ;
  rdfs:label "fitness-parcoursen"@nl ;
  rdfs:seeAlso <http://vocab.getty.edu/aat/300263166> ;
  rdfs:seeAlso wd:Q443006 ;
  rdfs:subClassOf <https://w3id.org/con-tax/zones/aat-buildingSites#300000626> ;
.
<https://w3id.org/con-tax/zones/aat-buildingSites#300263276>
  rdf:type owl:Class ;
  rdfs:comment "Buildings within a religious community complex in which novices are housed and trained during their period of probation."@en ;
  rdfs:comment "Gebouwen binnen het complex van een religieuze gemeenschap, waar novicen worden ondergebracht en opgeleid tijdens hun proeftijd."@nl ;
  rdfs:isDefinedBy <https://w3id.org/con-tax/zones/aat-buildingSites> ;
  rdfs:label "novicenhuis"@nl ;
  rdfs:label "novicenhuizen"@nl ;
  rdfs:label "noviciaat"@nl ;
  rdfs:label "noviciaten"@nl ;
  rdfs:label "novitiates (dwellings)"@en ;
  rdfs:seeAlso <http://vocab.getty.edu/aat/300263276> ;
  rdfs:subClassOf <https://w3id.org/con-tax/zones/aat-buildingSites#300000632> ;
.
<https://w3id.org/con-tax/zones/aat-buildingSites#300263521>
  rdf:type owl:Class ;
  rdfs:comment "Fortified sanctuaries used as a refuge in times of war, situated on hilltops in eastern Kenya among the Mijikenda and related peoples. Many kayas are regarded as sacred sites."@en ;
  rdfs:comment "Versterkte wijkplaatsen die als toevluchtsoord worden gebruikt in tijden van oorlog, gebouwd op heuveltoppen in het oosten van Kenia door de Mijikenda en verwante volkeren. Veel kaya's worden als heilige plaatsen beschouwd."@nl ;
  rdfs:isDefinedBy <https://w3id.org/con-tax/zones/aat-buildingSites> ;
  rdfs:label "kaya's"@nl ;
  rdfs:label "kayas (sites)"@en ;
  rdfs:seeAlso <http://vocab.getty.edu/aat/300263521> ;
  rdfs:subClassOf <https://w3id.org/con-tax/zones/aat-buildingSites#300000809> ;
.
<https://w3id.org/con-tax/zones/aat-buildingSites#300263741>
  rdf:type owl:Class ;
  rdfs:comment "Groupings of diversified religious buildings and related facilities."@en ;
  rdfs:isDefinedBy <https://w3id.org/con-tax/zones/aat-buildingSites> ;
  rdfs:label "religieuze complexen"@nl ;
  rdfs:label "religious complexes"@en ;
  rdfs:seeAlso <http://vocab.getty.edu/aat/300263741> ;
  rdfs:subClassOf <https://w3id.org/con-tax/zones/aat-buildingSites#300000202> ;
.
<https://w3id.org/con-tax/zones/aat-buildingSites#300263742>
  rdf:type owl:Class ;
  rdfs:comment "Religieuze complexen die doorgaans bestaan uit een structuur voor geloofsaanbidding, bijvoorbeeld een moskee of tempel, torens, en kleinere heiligdommen of tempels; typerend voor de religieuze architectuur van Zuidoost-Azië, India en het Midden-Oosten."@nl ;
  rdfs:comment "Religious complexes generally comprised of a structure of worship, such as a mosque or temple, towers, and subsidiary sancturaries or temples; characteristic of Southeast Asian, Indian, and Middle Eastern religious architecture."@en ;
  rdfs:isDefinedBy <https://w3id.org/con-tax/zones/aat-buildingSites> ;
  rdfs:label "kalan"@en ;
  rdfs:label "kalan"@nl ;
  rdfs:seeAlso <http://vocab.getty.edu/aat/300263742> ;
  rdfs:subClassOf <https://w3id.org/con-tax/zones/aat-buildingSites#300263741> ;
.
<https://w3id.org/con-tax/zones/aat-buildingSites#300264006>
  rdf:type owl:Class ;
  rdfs:comment "Housing complexes typically of African origin, comprised of enclosed single or multi-unit family dwellings with communal spaces, adjacent outbuildings or structures."@en ;
  rdfs:comment "Huisvestingscomplexen, meestal in Afrika, die bestaan uit omheinde familieverblijven voor één of meerdere families met gemeenschappelijke ruimten en aangrenzende bijgebouwen of structuren."@nl ;
  rdfs:isDefinedBy <https://w3id.org/con-tax/zones/aat-buildingSites> ;
  rdfs:label "compounds (housing complexes)"@en ;
  rdfs:label "kralen (huisvestingscomplexen)"@nl ;
  rdfs:label "kralen"@nl ;
  rdfs:seeAlso <http://vocab.getty.edu/aat/300264006> ;
  rdfs:subClassOf <https://w3id.org/con-tax/zones/aat-buildingSites#300259362> ;
.
<https://w3id.org/con-tax/zones/aat-buildingSites#300264040>
  rdf:type owl:Class ;
  rdfs:comment "Hill top resorts and places of refuge, especially in Asia, built by colonial administrators as an escape from the hot climates or politally unstable conditions."@en ;
  rdfs:comment "Woonverblijven op heuveltoppen en toevluchtsoorden, met name in Azië, die door koloniale ambtenaren zijn gebouwd om het warme klimaat of politiek instabiele situaties te ontvluchten."@nl ;
  rdfs:isDefinedBy <https://w3id.org/con-tax/zones/aat-buildingSites> ;
  rdfs:label "hill stations"@en ;
  rdfs:label "koloniale bergstations"@nl ;
  rdfs:seeAlso <http://vocab.getty.edu/aat/300264040> ;
  rdfs:seeAlso wd:Q2393184 ;
  rdfs:subClassOf <https://w3id.org/con-tax/zones/aat-buildingSites#300000547> ;
.
<https://w3id.org/con-tax/zones/aat-buildingSites#300264323>
  rdf:type owl:Class ;
  rdfs:comment "Refers to Indian religious communities whose members focus on religious study and meditation and lead lives of austere self-discipline. Such communities or retreats are usually secluded and center around a Hindu philosopher or religious teacher."@en ;
  rdfs:comment "Verwijst naar Indiase geloofsgemeenschappen waarvan de leden zich intensief bezighouden met religieuze studie en meditatie, en strenge, ascetische leefregels in acht nemen. Dergelijke gemeenschappen of retraites hebben doorgaans een afgezonderd karakter en functioneren rondom een hindoeïstische wijsgeer of geloofsleraar."@nl ;
  rdfs:isDefinedBy <https://w3id.org/con-tax/zones/aat-buildingSites> ;
  rdfs:label "ashrams"@en ;
  rdfs:label "ashrams"@nl ;
  rdfs:seeAlso <http://vocab.getty.edu/aat/300264323> ;
  rdfs:seeAlso wd:Q466449 ;
  rdfs:subClassOf <https://w3id.org/con-tax/zones/aat-buildingSites#300000632> ;
.
<https://w3id.org/con-tax/zones/aat-buildingSites#300265609>
  rdf:type owl:Class ;
  rdfs:comment "Openbare ruimten met beeldhouwwerken, earthworks of andere kunstvormen geïntegreerd in het ontwerp en beoogd gebruik."@nl ;
  rdfs:comment "Public spaces that feature sculpture, earthworks, or other art-forms as an integral part of their design and use."@en ;
  rdfs:isDefinedBy <https://w3id.org/con-tax/zones/aat-buildingSites> ;
  rdfs:label "art parks"@en ;
  rdfs:label "kunstparken"@nl ;
  rdfs:seeAlso <http://vocab.getty.edu/aat/300265609> ;
  rdfs:subClassOf <https://w3id.org/con-tax/zones/aat-buildingSites#300008187> ;
.
<https://w3id.org/con-tax/zones/aat-buildingSites#300265732>
  rdf:type owl:Class ;
  rdfs:comment "A nursery for breeding silkworms."@en ;
  rdfs:comment "Plaats waar zijdewormen worden gekweekt."@nl ;
  rdfs:isDefinedBy <https://w3id.org/con-tax/zones/aat-buildingSites> ;
  rdfs:label "magnaneries"@en ;
  rdfs:label "zijdewormkwekerijen"@nl ;
  rdfs:seeAlso <http://vocab.getty.edu/aat/300265732> ;
  rdfs:seeAlso wd:Q3277069 ;
  rdfs:subClassOf <https://w3id.org/con-tax/zones/aat-buildingSites#300000206> ;
.
<https://w3id.org/con-tax/zones/aat-buildingSites#300266151>
  rdf:type owl:Class ;
  rdfs:comment "Locaties waar wordt gegraven of op een andere wijze grondonderzoek wordt gedaan naar sporen van oude bewoning, zoals artefacten van menselijke activiteiten, fossielen, bevroren overblijfselen of andere geconserveerde resten."@nl ;
  rdfs:comment "Locations where there is digging or other uncovering of evidence of ancient life, including artifacts of human activity, fossils, frozen remains, or other preserved evidence."@en ;
  rdfs:isDefinedBy <https://w3id.org/con-tax/zones/aat-buildingSites> ;
  rdfs:label "excavations (sites)"@en ;
  rdfs:label "opgravingen (sites)"@nl ;
  rdfs:label "opgravingen"@nl ;
  rdfs:seeAlso <http://vocab.getty.edu/aat/300266151> ;
  rdfs:subClassOf <https://w3id.org/con-tax/zones/aat-buildingSites#300000810> ;
  rdfs:subClassOf <https://w3id.org/con-tax/zones/aat-buildingSites#300266152> ;
.
<https://w3id.org/con-tax/zones/aat-buildingSites#300266152>
  rdf:type owl:Class ;
  rdfs:comment "Sites waar sporen zijn aangetroffen van levensvormen die in vroegere geologische tijdvakken hebben bestaan. Gebruik 'archeologische sites' voor sites waar sporen van menselijke activiteit zijn gevonden."@nl ;
  rdfs:comment "Sites where there is evidence of forms of life that existed in former geologic periods. For sites where evidence of human activity exists, use \"archaeological sites.\""@en ;
  rdfs:isDefinedBy <https://w3id.org/con-tax/zones/aat-buildingSites> ;
  rdfs:label "paleontological sites"@en ;
  rdfs:label "paleontologische sites"@nl ;
  rdfs:seeAlso <http://vocab.getty.edu/aat/300266152> ;
  rdfs:subClassOf <https://w3id.org/con-tax/zones/aat-buildingSites#300000809> ;
.
<https://w3id.org/con-tax/zones/aat-buildingSites#300312088>
  rdf:type owl:Class ;
  rdfs:comment "Downhill paths on a mountain or large hill that are maintained for snow skiing, snowboarding, or other mountain sports,  usually marked, patrolled, and graded according to difficulty."@en ;
  rdfs:comment "Helling van een berg of een grote heuvel die men prepareert voor skiërs, snowboarders, enzovoort. Gewoonlijk zijn ze voorzien van markeringen en wordt de moeilijkheidsgraad aangegeven. Op skipistes wordt doorgaans toezicht gehouden."@nl ;
  rdfs:isDefinedBy <https://w3id.org/con-tax/zones/aat-buildingSites> ;
  rdfs:label "ski runs"@en ;
  rdfs:label "skipiste"@nl ;
  rdfs:label "skipistes"@nl ;
  rdfs:seeAlso <http://vocab.getty.edu/aat/300312088> ;
  rdfs:subClassOf <https://w3id.org/con-tax/zones/aat-buildingSites#300000626> ;
.
<https://w3id.org/con-tax/zones/aat-buildingSites#300312090>
  rdf:type owl:Class ;
  rdfs:comment "Places where construction is occurring, particularly construction of a building. For the more general meaning of a site where a building is or was located, whether or not the building is under construction, use \"building sites.\" "@en ;
  rdfs:comment "Plekken waar gebouwd wordt, waarbij het met name gebouwen betreft."@nl ;
  rdfs:isDefinedBy <https://w3id.org/con-tax/zones/aat-buildingSites> ;
  rdfs:label "bouwterrein"@nl ;
  rdfs:label "bouwterreinen"@nl ;
  rdfs:label "construction sites"@en ;
  rdfs:seeAlso <http://vocab.getty.edu/aat/300312090> ;
  rdfs:subClassOf <https://w3id.org/con-tax/zones/aat-buildingSites#300000809> ;
.
<https://w3id.org/con-tax/zones/aat-buildingSites#300312183>
  rdf:type owl:Class ;
  rdfs:comment "Afkomstig van het Italiaanse woord 'galleria', dat oorspronkelijk verwees naar zuilengangen met winkels in Italiaanse steden, op basis van de antieke stoa's. Verwijst nu naar winkelcentra die qua architectuur lijken of geïnspireerd zijn op de Italiaanse galleria's. De term wordt ook gebruikt voor gebieden van een winkelcentrum die zo ontworpen zijn dat het lijkt alsof ze uit een aantal afzonderlijke winkels bestaan."@nl ;
  rdfs:comment "Originally referred to a distinctive type of arcade of shops in Italian cities, descendents of the ancient stoas. Now refers to covered shopping malls that architecturally resemble or were inspired by Italian gallerias. The term is also used to describe areas of a department store that are designed so as to appear to contain a number of separate shops."@en ;
  rdfs:isDefinedBy <https://w3id.org/con-tax/zones/aat-buildingSites> ;
  rdfs:label "gallerias (shopping centers)"@en ;
  rdfs:label "winkelgalerij"@nl ;
  rdfs:label "winkelgalerijen (winkelcentra)"@nl ;
  rdfs:label "winkelgalerijen"@nl ;
  rdfs:seeAlso <http://vocab.getty.edu/aat/300312183> ;
  rdfs:subClassOf <https://w3id.org/con-tax/zones/aat-buildingSites#300005268> ;
.
<https://w3id.org/con-tax/zones/aat-buildingSites#300312239>
  rdf:type owl:Class ;
  rdfs:comment "Buildings that housed urban prisons for debtors, particularly those in London, Southwark, Exeter, and other English cities."@en ;
  rdfs:comment "Gebouwen met stedelijke gevangenissen voor schuldenaren, met name in Londen, Southwark, Exeter en andere Engels steden. "@nl ;
  rdfs:isDefinedBy <https://w3id.org/con-tax/zones/aat-buildingSites> ;
  rdfs:label "compter"@nl ;
  rdfs:label "compters"@en ;
  rdfs:label "compters"@nl ;
  rdfs:seeAlso <http://vocab.getty.edu/aat/300312239> ;
  rdfs:seeAlso wd:Q5157122 ;
  rdfs:subClassOf <https://w3id.org/con-tax/zones/aat-buildingSites#300006477> ;
.
<https://w3id.org/con-tax/zones/aat-buildingSites#300312257>
  rdf:type owl:Class ;
  rdfs:comment "Generally refers to buildings housing prisons for those convicted of major crimes. "@en ;
  rdfs:comment "Verwijst in het algemeen naar gebouwen voor gevangenissen voor mensen die voor grote misdrijven zijn veroordeeld."@nl ;
  rdfs:isDefinedBy <https://w3id.org/con-tax/zones/aat-buildingSites> ;
  rdfs:label "penitentiaries (buildings)"@en ;
  rdfs:label "strafinrichting"@nl ;
  rdfs:label "strafinrichtingen"@nl ;
  rdfs:seeAlso <http://vocab.getty.edu/aat/300312257> ;
  rdfs:subClassOf <https://w3id.org/con-tax/zones/aat-buildingSites#300006460> ;
.
<https://w3id.org/con-tax/zones/aat-buildingSites#300312258>
  rdf:type owl:Class ;
  rdfs:comment "Onderaardse ruimtes of constructies met cellen of andere kamers met zeer stevige muren waarin mensen kunnen worden opgesloten."@nl ;
  rdfs:comment "Subterranean rooms or structures that comprise strongly fortified cells or other rooms of confinement; the term originally derived from such areas below the keep or donjon of a castle."@en ;
  rdfs:isDefinedBy <https://w3id.org/con-tax/zones/aat-buildingSites> ;
  rdfs:label "dungeons (jails)"@en ;
  rdfs:label "kerker"@nl ;
  rdfs:label "kerkers (gevangenissen)"@nl ;
  rdfs:label "kerkers"@nl ;
  rdfs:seeAlso <http://vocab.getty.edu/aat/300312258> ;
  rdfs:subClassOf <https://w3id.org/con-tax/zones/aat-buildingSites#300006457> ;
.
<https://w3id.org/con-tax/zones/aat-buildingSites#300343477>
  rdf:type owl:Class ;
  rdfs:comment "Buildings that house institutions of confinement and correction, using hard labor and strict discipline with a view to reformation of the inmates; especially those dating to the 16th century and later in Europe and colonial America. For general reference to buildings housing any institution of correction, use \"correctional institutions (buildings).\""@en ;
  rdfs:comment "Gebouwen met daarin instellingen voor opsluiting en verbetering, waarin met hard werk en strenge discipline wordt geprobeerd te ingezetenen te verbeteren. Vooral gebruikt voor dergelijke gebouwen vanaf de 16e eeuw in Europa en koloniaal Amerika. Gebruik 'strafrechtelijke instellingen (gebouwen)' om in het algemeen te verwijzen naar verbeteringsgestichten."@nl ;
  rdfs:isDefinedBy <https://w3id.org/con-tax/zones/aat-buildingSites> ;
  rdfs:label "houses of correction (buildings)"@en ;
  rdfs:label "tuchtscholen (gebouwen)"@nl ;
  rdfs:label "tuchtscholen"@nl ;
  rdfs:label "tuchtschool"@nl ;
  rdfs:seeAlso <http://vocab.getty.edu/aat/300343477> ;
  rdfs:subClassOf <https://w3id.org/con-tax/zones/aat-buildingSites#300006448> ;
.
<https://w3id.org/con-tax/zones/aat-buildingSites#300375113>
  rdf:type owl:Class ;
  rdfs:comment "Class of circular or radiating boulder outlines built by ancient North American Indian peoples of the Great Plains. These enigmatic archaeological features are believed to have some religious, astronomical, territorial, or calendrical significance."@en ;
  rdfs:isDefinedBy <https://w3id.org/con-tax/zones/aat-buildingSites> ;
  rdfs:label "medicine wheels"@en ;
  rdfs:seeAlso <http://vocab.getty.edu/aat/300375113> ;
  rdfs:subClassOf <https://w3id.org/con-tax/zones/aat-buildingSites#300000809> ;
.
<https://w3id.org/con-tax/zones/aat-buildingSites#300379361>
  rdf:type owl:Class ;
  rdfs:comment "Archaeological sites that accomodate tourism and public use."@en ;
  rdfs:isDefinedBy <https://w3id.org/con-tax/zones/aat-buildingSites> ;
  rdfs:label "archaeological parks"@en ;
  rdfs:seeAlso <http://vocab.getty.edu/aat/300379361> ;
  rdfs:subClassOf <https://w3id.org/con-tax/zones/aat-buildingSites#300008187> ;
.
<https://w3id.org/con-tax/zones/aat-buildingSites#300379656>
  rdf:type owl:Class ;
  rdfs:comment "In archaeology, refers to all water-saturated archaeological sites. "@en ;
  rdfs:isDefinedBy <https://w3id.org/con-tax/zones/aat-buildingSites> ;
  rdfs:label "wet sites"@en ;
  rdfs:seeAlso <http://vocab.getty.edu/aat/300379656> ;
  rdfs:subClassOf <https://w3id.org/con-tax/zones/aat-buildingSites#300000810> ;
.
<https://w3id.org/con-tax/zones/aat-buildingSites#300380027>
  rdf:type owl:Class ;
  rdfs:comment "Heritage sites and the lands related to them committed to providing a cultural, recreational, and cultural resource for the public at large."@en ;
  rdfs:isDefinedBy <https://w3id.org/con-tax/zones/aat-buildingSites> ;
  rdfs:label "cultural parks"@en ;
  rdfs:seeAlso <http://vocab.getty.edu/aat/300380027> ;
  rdfs:subClassOf <https://w3id.org/con-tax/zones/aat-buildingSites#300008187> ;
.
<https://w3id.org/con-tax/zones/aat-buildingSites#300380313>
  rdf:type owl:Class ;
  rdfs:comment "Detention camps for enemy combatants captured in time of war."@en ;
  rdfs:isDefinedBy <https://w3id.org/con-tax/zones/aat-buildingSites> ;
  rdfs:label "prisoner-of-war camps"@en ;
  rdfs:seeAlso <http://vocab.getty.edu/aat/300380313> ;
  rdfs:seeAlso wd:Q1070290 ;
  rdfs:subClassOf <https://w3id.org/con-tax/zones/aat-buildingSites#300000476> ;
.
<https://w3id.org/con-tax/zones/aat-buildingSites#300380520>
  rdf:type owl:Class ;
  rdfs:comment "UNESCO designation and brand for unified areas with outstanding geological heritage of international significance, where low impact recreation, scientific research, and educational activities can be pursued. "@en ;
  rdfs:isDefinedBy <https://w3id.org/con-tax/zones/aat-buildingSites> ;
  rdfs:label "geoparks"@en ;
  rdfs:seeAlso <http://vocab.getty.edu/aat/300380520> ;
  rdfs:seeAlso wd:Q1324355 ;
  rdfs:subClassOf <https://w3id.org/con-tax/zones/aat-buildingSites#300008187> ;
.
<https://w3id.org/con-tax/zones/aat-buildingSites#300386092>
  rdf:type owl:Class ;
  rdfs:comment "A type of religious complex that houses Buddhist monks and serves the greater community during festivals and other occasions."@en ;
  rdfs:isDefinedBy <https://w3id.org/con-tax/zones/aat-buildingSites> ;
  rdfs:label "kyaungs"@en ;
  rdfs:seeAlso <http://vocab.getty.edu/aat/300386092> ;
  rdfs:subClassOf <https://w3id.org/con-tax/zones/aat-buildingSites#300000641> ;
.
<https://w3id.org/con-tax/zones/aat-buildingSites#300386889>
  rdf:type owl:Class ;
  rdfs:comment "Exposed forests on the earth's surface that have been fossilized by geologic activity."@en ;
  rdfs:isDefinedBy <https://w3id.org/con-tax/zones/aat-buildingSites> ;
  rdfs:label "fossilized forests"@en ;
  rdfs:seeAlso <http://vocab.getty.edu/aat/300386889> ;
  rdfs:subClassOf <https://w3id.org/con-tax/zones/aat-buildingSites#300000809> ;
.
<https://w3id.org/con-tax/zones/aat-buildingSites#300386973>
  rdf:type owl:Class ;
  rdfs:comment "Sites of the remains of wrecked vessels. "@en ;
  rdfs:isDefinedBy <https://w3id.org/con-tax/zones/aat-buildingSites> ;
  rdfs:label "wrecks (sites)"@en ;
  rdfs:seeAlso <http://vocab.getty.edu/aat/300386973> ;
  rdfs:subClassOf <https://w3id.org/con-tax/zones/aat-buildingSites#300000809> ;
.
<https://w3id.org/con-tax/zones/aat-buildingSites#300386977>
  rdf:type owl:Class ;
  rdfs:comment "Areas containing properties and buildings of historical significance, and extending to include significant natural features as well."@en ;
  rdfs:isDefinedBy <https://w3id.org/con-tax/zones/aat-buildingSites> ;
  rdfs:label "historical parks"@en ;
  rdfs:seeAlso <http://vocab.getty.edu/aat/300386977> ;
  rdfs:subClassOf <https://w3id.org/con-tax/zones/aat-buildingSites#300008187> ;
.
<https://w3id.org/con-tax/zones/aat-buildingSites#300386978>
  rdf:type owl:Class ;
  rdfs:comment "General term for parks that preserve areas associated with military history."@en ;
  rdfs:isDefinedBy <https://w3id.org/con-tax/zones/aat-buildingSites> ;
  rdfs:label "military parks"@en ;
  rdfs:seeAlso <http://vocab.getty.edu/aat/300386978> ;
  rdfs:subClassOf <https://w3id.org/con-tax/zones/aat-buildingSites#300008187> ;
.
<https://w3id.org/con-tax/zones/aat-buildingSites#300386979>
  rdf:type owl:Class ;
  rdfs:comment "Historic sites where significant battles are memorialized; used specifically in reference to Civil War battlefield sites in the United States, some of which are also National Parks. "@en ;
  rdfs:isDefinedBy <https://w3id.org/con-tax/zones/aat-buildingSites> ;
  rdfs:label "battlefield parks"@en ;
  rdfs:seeAlso <http://vocab.getty.edu/aat/300386979> ;
  rdfs:subClassOf <https://w3id.org/con-tax/zones/aat-buildingSites#300008187> ;
.
<https://w3id.org/con-tax/zones/aat-buildingSites#300386984>
  rdf:type owl:Class ;
  rdfs:comment "Complexes, which are aggregations of buildings, other structures, and/or open spaces, that were formerly occupied but are now deserted by former inhabitants."@en ;
  rdfs:isDefinedBy <https://w3id.org/con-tax/zones/aat-buildingSites> ;
  rdfs:label "abandoned complexes"@en ;
  rdfs:seeAlso <http://vocab.getty.edu/aat/300386984> ;
  rdfs:subClassOf <https://w3id.org/con-tax/zones/aat-buildingSites#300000202> ;
.
<https://w3id.org/con-tax/zones/aat-buildingSites#300386994>
  rdf:type owl:Class ;
  rdfs:comment "Military installations or reservations, or defense-related industries. "@en ;
  rdfs:isDefinedBy <https://w3id.org/con-tax/zones/aat-buildingSites> ;
  rdfs:label "defense installations"@en ;
  rdfs:seeAlso <http://vocab.getty.edu/aat/300386994> ;
  rdfs:subClassOf <https://w3id.org/con-tax/zones/aat-buildingSites#300164060> ;
.
<https://w3id.org/con-tax/zones/aat-buildingSites#300386996>
  rdf:type owl:Class ;
  rdfs:comment "General term for government facilities or complexes. "@en ;
  rdfs:isDefinedBy <https://w3id.org/con-tax/zones/aat-buildingSites> ;
  rdfs:label "governmental installations"@en ;
  rdfs:seeAlso <http://vocab.getty.edu/aat/300386996> ;
  rdfs:subClassOf <https://w3id.org/con-tax/zones/aat-buildingSites#300000202> ;
.
<https://w3id.org/con-tax/zones/aat-buildingSites#300386998>
  rdf:type owl:Class ;
  rdfs:comment "Sites considered in the past or present as consecrated or important to a deity or a religion; sites include natural features, such as springs and caves, as well as sites upon which built works have been constructed, such as standing stones and pilgrimage churches."@en ;
  rdfs:isDefinedBy <https://w3id.org/con-tax/zones/aat-buildingSites> ;
  rdfs:label "sacred sites"@en ;
  rdfs:seeAlso <http://vocab.getty.edu/aat/300386998> ;
  rdfs:subClassOf <https://w3id.org/con-tax/zones/aat-buildingSites#300000809> ;
.
<https://w3id.org/con-tax/zones/aat-buildingSites#300387000>
  rdf:type owl:Class ;
  rdfs:comment "Sites that are used for ceremonial purposes; often an ancient site, sometimes the purpose of which is unknown."@en ;
  rdfs:isDefinedBy <https://w3id.org/con-tax/zones/aat-buildingSites> ;
  rdfs:label "ceremonial sites"@en ;
  rdfs:seeAlso <http://vocab.getty.edu/aat/300387000> ;
  rdfs:subClassOf <https://w3id.org/con-tax/zones/aat-buildingSites#300000809> ;
.
<https://w3id.org/con-tax/zones/aat-buildingSites#300387001>
  rdf:type owl:Class ;
  rdfs:comment "Consecrated grounds that surround religious sites or places of worship."@en ;
  rdfs:isDefinedBy <https://w3id.org/con-tax/zones/aat-buildingSites> ;
  rdfs:label "holy precincts"@en ;
  rdfs:seeAlso <http://vocab.getty.edu/aat/300387001> ;
  rdfs:subClassOf <https://w3id.org/con-tax/zones/aat-buildingSites#300000809> ;
.
<https://w3id.org/con-tax/zones/aat-buildingSites#300387004>
  rdf:type owl:Class ;
  rdfs:comment "Any place where burials have taken place, generally restricted to human or other hominin burials."@en ;
  rdfs:isDefinedBy <https://w3id.org/con-tax/zones/aat-buildingSites> ;
  rdfs:label "burial sites"@en ;
  rdfs:seeAlso <http://vocab.getty.edu/aat/300387004> ;
  rdfs:subClassOf <https://w3id.org/con-tax/zones/aat-buildingSites#300000809> ;
.
<https://w3id.org/con-tax/zones/aat-buildingSites#300387005>
  rdf:type owl:Class ;
  rdfs:comment "Sites that contain prehistoric, megalithic monuments."@en ;
  rdfs:isDefinedBy <https://w3id.org/con-tax/zones/aat-buildingSites> ;
  rdfs:label "megalithic sites"@en ;
  rdfs:seeAlso <http://vocab.getty.edu/aat/300387005> ;
  rdfs:subClassOf <https://w3id.org/con-tax/zones/aat-buildingSites#300000809> ;
.
<https://w3id.org/con-tax/zones/aat-buildingSites#300387006>
  rdf:type owl:Class ;
  rdfs:comment "Sites that contain evidence of prehistoric human activity, often through archaeological investigation. "@en ;
  rdfs:isDefinedBy <https://w3id.org/con-tax/zones/aat-buildingSites> ;
  rdfs:label "prehistoric sites"@en ;
  rdfs:seeAlso <http://vocab.getty.edu/aat/300387006> ;
  rdfs:subClassOf <https://w3id.org/con-tax/zones/aat-buildingSites#300000809> ;
.
<https://w3id.org/con-tax/zones/aat-buildingSites#300387007>
  rdf:type owl:Class ;
  rdfs:comment "General term for relatively small and contained places where archeological remains, old structures, or cultural artifacts are or were located."@en ;
  rdfs:isDefinedBy <https://w3id.org/con-tax/zones/aat-buildingSites> ;
  rdfs:label "ancient sites"@en ;
  rdfs:seeAlso <http://vocab.getty.edu/aat/300387007> ;
  rdfs:seeAlso wd:Q839954 ;
  rdfs:subClassOf <https://w3id.org/con-tax/zones/aat-buildingSites#300000809> ;
.
<https://w3id.org/con-tax/zones/aat-buildingSites#300387009>
  rdf:type owl:Class ;
  rdfs:comment "Sites that contain evidence of protohistoric human activity, often through archaeological investigation. "@en ;
  rdfs:isDefinedBy <https://w3id.org/con-tax/zones/aat-buildingSites> ;
  rdfs:label "protohistoric sites"@en ;
  rdfs:seeAlso <http://vocab.getty.edu/aat/300387009> ;
  rdfs:subClassOf <https://w3id.org/con-tax/zones/aat-buildingSites#300000809> ;
.
<https://w3id.org/con-tax/zones/aat-buildingSites#300387027>
  rdf:type owl:Class ;
  rdfs:comment "Building or complex where activities having to do with any branch of science take place."@en ;
  rdfs:isDefinedBy <https://w3id.org/con-tax/zones/aat-buildingSites> ;
  rdfs:label "scientific facilities"@en ;
  rdfs:seeAlso <http://vocab.getty.edu/aat/300387027> ;
  rdfs:subClassOf <https://w3id.org/con-tax/zones/aat-buildingSites#300000202> ;
.
<https://w3id.org/con-tax/zones/aat-buildingSites#300387031>
  rdf:type owl:Class ;
  rdfs:comment "Scientific facilities used as bases from which research is carried out or monitored."@en ;
  rdfs:isDefinedBy <https://w3id.org/con-tax/zones/aat-buildingSites> ;
  rdfs:label "scientific research bases (facilities)"@en ;
  rdfs:seeAlso <http://vocab.getty.edu/aat/300387031> ;
  rdfs:subClassOf <https://w3id.org/con-tax/zones/aat-buildingSites#300387027> ;
.
<https://w3id.org/con-tax/zones/aat-buildingSites#300387039>
  rdf:type owl:Class ;
  rdfs:comment "Complexes or structures having as a main purpose the launching of vehicles or rockets into the atmosphere or space, or having other functions having to do with space or air travel, for example designing testing space vehicles."@en ;
  rdfs:isDefinedBy <https://w3id.org/con-tax/zones/aat-buildingSites> ;
  rdfs:label "aerospace facilities"@en ;
  rdfs:seeAlso <http://vocab.getty.edu/aat/300387039> ;
  rdfs:subClassOf <https://w3id.org/con-tax/zones/aat-buildingSites#300000678> ;
  rdfs:subClassOf <https://w3id.org/con-tax/zones/aat-buildingSites#300387027> ;
.
<https://w3id.org/con-tax/zones/aat-buildingSites#300387201>
  rdf:type owl:Class ;
  rdfs:comment "Administrative centers of operation. Used often to refer to military headquarters or installations. "@en ;
  rdfs:isDefinedBy <https://w3id.org/con-tax/zones/aat-buildingSites> ;
  rdfs:label "bases (operational centers)"@en ;
  rdfs:seeAlso <http://vocab.getty.edu/aat/300387201> ;
  rdfs:subClassOf <https://w3id.org/con-tax/zones/aat-buildingSites#300000202> ;
.
<https://w3id.org/con-tax/zones/aat-buildingSites#300387230>
  rdf:type owl:Class ;
  rdfs:comment "Temporary settlements used for laborers during railroad construction."@en ;
  rdfs:isDefinedBy <https://w3id.org/con-tax/zones/aat-buildingSites> ;
  rdfs:label "railroad camps"@en ;
  rdfs:seeAlso <http://vocab.getty.edu/aat/300387230> ;
  rdfs:subClassOf <https://w3id.org/con-tax/zones/aat-buildingSites#300000300> ;
.
<https://w3id.org/con-tax/zones/aat-buildingSites#300387251>
  rdf:type owl:Class ;
  rdfs:comment "Places on land, beside a body of water, where fishermen gather or otherwise from which fishing is practiced. For hydrographic features where fishing is done offshore, use \"fishing areas.\""@en ;
  rdfs:isDefinedBy <https://w3id.org/con-tax/zones/aat-buildingSites> ;
  rdfs:label "fishing spots (sites)"@en ;
  rdfs:seeAlso <http://vocab.getty.edu/aat/300387251> ;
  rdfs:subClassOf <https://w3id.org/con-tax/zones/aat-buildingSites#300000809> ;
.
<https://w3id.org/con-tax/zones/aat-buildingSites#300387268>
  rdf:type owl:Class ;
  rdfs:comment "Locations that were or are the site of a concentration camp internment center."@en ;
  rdfs:isDefinedBy <https://w3id.org/con-tax/zones/aat-buildingSites> ;
  rdfs:label "concentration camp sites"@en ;
  rdfs:seeAlso <http://vocab.getty.edu/aat/300387268> ;
  rdfs:subClassOf <https://w3id.org/con-tax/zones/aat-buildingSites#300000809> ;
.
<https://w3id.org/con-tax/zones/aat-buildingSites#300387307>
  rdf:type owl:Class ;
  rdfs:comment "Sites where an oil well is located."@en ;
  rdfs:isDefinedBy <https://w3id.org/con-tax/zones/aat-buildingSites> ;
  rdfs:label "oil field sites"@en-us ;
  rdfs:seeAlso <http://vocab.getty.edu/aat/300387307> ;
  rdfs:subClassOf <https://w3id.org/con-tax/zones/aat-buildingSites#300000809> ;
.
<https://w3id.org/con-tax/zones/aat-buildingSites#300387322>
  rdf:type owl:Class ;
  rdfs:comment "Operational centers of any size used for activities surrounding hunting; may be contemporary or prehistoric."@en ;
  rdfs:isDefinedBy <https://w3id.org/con-tax/zones/aat-buildingSites> ;
  rdfs:label "hunting bases"@en ;
  rdfs:seeAlso <http://vocab.getty.edu/aat/300387322> ;
  rdfs:subClassOf <https://w3id.org/con-tax/zones/aat-buildingSites#300000809> ;
.
<https://w3id.org/con-tax/zones/aat-buildingSites#300387501>
  rdf:type owl:Class ;
  rdfs:comment "Waterside facilities for servicing, repairing, and building small vessels."@en ;
  rdfs:isDefinedBy <https://w3id.org/con-tax/zones/aat-buildingSites> ;
  rdfs:label "boatyards"@en ;
  rdfs:seeAlso <http://vocab.getty.edu/aat/300387501> ;
  rdfs:subClassOf <https://w3id.org/con-tax/zones/aat-buildingSites#300120802> ;
.
<https://w3id.org/con-tax/zones/aat-buildingSites#300387502>
  rdf:type owl:Class ;
  rdfs:comment "Large, usually commercialized, agricultural landholdings with associated buildings and other facilities. The term is often used for former European colonial land holdings, similar to plantations. For landholdings that are intended primarily or in large part as the residence of the private owner, even if there are crops and tenant farmers, use \"estates (residential complexes).\" Meaning and usage of \"estates\" overlap with \"plantations,\" although plantations are usually larger enterprises than agricultural estates."@en ;
  rdfs:isDefinedBy <https://w3id.org/con-tax/zones/aat-buildingSites> ;
  rdfs:label "estates (commercial agricultural holding)"@en ;
  rdfs:seeAlso <http://vocab.getty.edu/aat/300387502> ;
  rdfs:subClassOf <https://w3id.org/con-tax/zones/aat-buildingSites#300125766> ;
.
<https://w3id.org/con-tax/zones/aat-buildingSites#300387535>
  rdf:type owl:Class ;
  rdfs:comment "Sites that are underwater and where archaeological excavations or exploration takes place. Included are shipwrecks, harbor and dock remains, fishing structures, and flooded land sites."@en ;
  rdfs:isDefinedBy <https://w3id.org/con-tax/zones/aat-buildingSites> ;
  rdfs:label "underwater archaeological sites"@en ;
  rdfs:seeAlso <http://vocab.getty.edu/aat/300387535> ;
  rdfs:subClassOf <https://w3id.org/con-tax/zones/aat-buildingSites#300000810> ;
  rdfs:subClassOf <https://w3id.org/con-tax/zones/aat-buildingSites#300229352> ;
.
<https://w3id.org/con-tax/zones/aat-buildingSites#300387655>
  rdf:type owl:Class ;
  rdfs:comment "Sites that were originally on dry land but have been submerged or flooded."@en ;
  rdfs:isDefinedBy <https://w3id.org/con-tax/zones/aat-buildingSites> ;
  rdfs:label "submerged sites"@en ;
  rdfs:seeAlso <http://vocab.getty.edu/aat/300387655> ;
  rdfs:subClassOf <https://w3id.org/con-tax/zones/aat-buildingSites#300229352> ;
.
<https://w3id.org/con-tax/zones/aat-buildingSites#300389664>
  rdf:type owl:Class ;
  rdfs:comment "Heritage trails having an emphasis primarily on more ancient history, including archaelogical remains and sites. The trail itself may also be of archaeological significance."@en ;
  rdfs:isDefinedBy <https://w3id.org/con-tax/zones/aat-buildingSites> ;
  rdfs:label "archaeological trails"@en ;
  rdfs:seeAlso <http://vocab.getty.edu/aat/300389664> ;
  rdfs:subClassOf <https://w3id.org/con-tax/zones/aat-buildingSites#300000627> ;
.
<https://w3id.org/con-tax/zones/aat-buildingSites#300389859>
  rdf:type owl:Class ;
  rdfs:comment "During the Iron Age, settlements were the settings for ritual activities which included the making of special deposits. A series of rectangular ditched enclosures known as Viereckschanzen is concentrated in the temperate regions of central Europe. Many include deposits of iron weapons and tools in the ditches."@en ;
  rdfs:isDefinedBy <https://w3id.org/con-tax/zones/aat-buildingSites> ;
  rdfs:label "Viereckschanzen"@en ;
  rdfs:seeAlso <http://vocab.getty.edu/aat/300389859> ;
  rdfs:subClassOf <https://w3id.org/con-tax/zones/aat-buildingSites#300000810> ;
  rdfs:subClassOf <https://w3id.org/con-tax/zones/aat-buildingSites#300387000> ;
.
<https://w3id.org/con-tax/zones/aat-buildingSites#300391489>
  rdf:type owl:Class ;
  rdfs:comment "In archaeology, geology, and related disciplines, sites having features or characteristics that are used to define, or are paradigmatic of, a culture, stratigraphic level, or other pertinent feature or characteristic. For example, in archaeology, a type site could contain artifacts in an assemblage that are typical of that culture. The type site is often the eponym for the culture or feature, that is, the site after which the culture or feature is named."@en ;
  rdfs:isDefinedBy <https://w3id.org/con-tax/zones/aat-buildingSites> ;
  rdfs:label "type sites"@en ;
  rdfs:seeAlso <http://vocab.getty.edu/aat/300391489> ;
  rdfs:seeAlso wd:Q3247173 ;
  rdfs:subClassOf <https://w3id.org/con-tax/zones/aat-buildingSites#300000809> ;
.
<https://w3id.org/con-tax/zones/aat-buildingSites#300393260>
  rdf:type owl:Class ;
  rdfs:comment "Ceremonial mens' houses with highly symbolic decorative elements that are located in Papua New Guinea. They are used as meeting places for ceremonies, rituals, production workshops for making ritual objects, and sacred housing for ritual objects. Traditionally, women and uninitiated men were not allowed access to haus tambaran."@en ;
  rdfs:isDefinedBy <https://w3id.org/con-tax/zones/aat-buildingSites> ;
  rdfs:label "haus tambaran"@en ;
  rdfs:seeAlso <http://vocab.getty.edu/aat/300393260> ;
  rdfs:seeAlso wd:Q3128371 ;
  rdfs:subClassOf <https://w3id.org/con-tax/zones/aat-buildingSites#300000632> ;
.
<https://w3id.org/con-tax/zones/aat-buildingSites#300395666>
  rdf:type owl:Class ;
  rdfs:comment "Hindu places of pilgrimage that are natural features, usually associatied with a river or lake."@en ;
  rdfs:isDefinedBy <https://w3id.org/con-tax/zones/aat-buildingSites> ;
  rdfs:label "tirthas"@en ;
  rdfs:seeAlso <http://vocab.getty.edu/aat/300395666> ;
  rdfs:subClassOf <https://w3id.org/con-tax/zones/aat-buildingSites#300000809> ;
.
<https://w3id.org/con-tax/zones/aat-buildingSites#300403957>
  rdf:type owl:Class ;
  rdfs:comment "Areas set aside for the propagation of game for hunters, specifically for shooting."@en ;
  rdfs:isDefinedBy <https://w3id.org/con-tax/zones/aat-buildingSites> ;
  rdfs:label "shooting preserves"@en ;
  rdfs:seeAlso <http://vocab.getty.edu/aat/300403957> ;
  rdfs:subClassOf <https://w3id.org/con-tax/zones/aat-buildingSites#300000557> ;
.
<https://w3id.org/con-tax/zones/aat-buildingSites#300403958>
  rdf:type owl:Class ;
  rdfs:comment "Areas set aside for the propagation of game, especially in historical usage. For modern areas set aside for shooting with guns, use \"shooting preserves.\""@en ;
  rdfs:isDefinedBy <https://w3id.org/con-tax/zones/aat-buildingSites> ;
  rdfs:label "game reserves"@en ;
  rdfs:seeAlso <http://vocab.getty.edu/aat/300403958> ;
  rdfs:subClassOf <https://w3id.org/con-tax/zones/aat-buildingSites#300000557> ;
.
<https://w3id.org/con-tax/zones/aat-buildingSites#300403982>
  rdf:type owl:Class ;
  rdfs:comment "Fields where wet rice is grown."@en ;
  rdfs:isDefinedBy <https://w3id.org/con-tax/zones/aat-buildingSites> ;
  rdfs:label "rice paddies"@en ;
  rdfs:seeAlso <http://vocab.getty.edu/aat/300403982> ;
  rdfs:subClassOf <https://w3id.org/con-tax/zones/aat-buildingSites#300125766> ;
.
<https://w3id.org/con-tax/zones/aat-buildingSites#300404009>
  rdf:type owl:Class ;
  rdfs:comment "Complexes built for the purpose of docking ferries, for the embarking or disembarking of passengers, or cargo. "@en ;
  rdfs:isDefinedBy <https://w3id.org/con-tax/zones/aat-buildingSites> ;
  rdfs:label "ferry terminals"@en ;
  rdfs:seeAlso <http://vocab.getty.edu/aat/300404009> ;
  rdfs:subClassOf <https://w3id.org/con-tax/zones/aat-buildingSites#300007752> ;
.
<https://w3id.org/con-tax/zones/aat-buildingSites#300404177>
  rdf:type owl:Class ;
  rdfs:comment "Facilities for producing fertilizer."@en ;
  rdfs:isDefinedBy <https://w3id.org/con-tax/zones/aat-buildingSites> ;
  rdfs:label "phosphate works"@en ;
  rdfs:seeAlso <http://vocab.getty.edu/aat/300404177> ;
  rdfs:subClassOf <https://w3id.org/con-tax/zones/aat-buildingSites#300125766> ;
.
<https://w3id.org/con-tax/zones/aat-buildingSites#300404837>
  rdf:type owl:Class ;
  rdfs:comment """Grondeigendommen, meestal van aanzienlijke afmetingen, met vaak een groot huis en bijgebouwen, en soms met land waarop gewassen worden verbouwd. Soms verzorgen huurders de landbouwgronden. Gebruik 'landgoederen (landbouwcomplexen)' voor commerciële landbouwgrond, met name wanneer ze op plantages lijken en zich in Europese koloniale gebieden bevinden.
"""@nl ;
  rdfs:comment "Landed properties, usually of considerable extent, which typically have a grand house and outbuildings, and which may, but not necessarily must, have certain land on which a crop is cultivated; may have tenants who operate the agricultural lands. For commercial agricultural lands, particularly those similar to plantations and located in European colonial areas, use \"estates (commercial agricultural holdings).\""@en ;
  rdfs:isDefinedBy <https://w3id.org/con-tax/zones/aat-buildingSites> ;
  rdfs:label "estates (residential complexes)"@en ;
  rdfs:label "landgoed (wooncomplex)"@nl ;
  rdfs:label "landgoed"@nl ;
  rdfs:label "landgoederen (wooncomplexen)"@nl ;
  rdfs:label "landgoederen"@nl ;
  rdfs:seeAlso <http://vocab.getty.edu/aat/300404837> ;
  rdfs:subClassOf <https://w3id.org/con-tax/zones/aat-buildingSites#300259362> ;
.
<https://w3id.org/con-tax/zones/aat-buildingSites#300404840>
  rdf:type owl:Class ;
  rdfs:comment "Sites upon which one building is built, altered through major accretion to become a different building, or rebuilt as a different building over time, but still retaining the same function and often the same name. The term is often, but not exclusively, used for archaeological sites having this characteristic; refers to both the site and the sum of structures that have occupied the site over time. Examples include the Aztec Templo Mayor, which was rebuilt six times on the same site, and the Temple of Jerusalem, also rebuilt several times on the same site, and Stonehenge, altered through accretion over centuries. To refer in general to a site where a building is or was located, whether or not the building is under construction, use \"building sites.\""@en ;
  rdfs:comment """Sites waarop een gebouw is gebouwd, dat door grootschalige bijbouw een ander gebouw wordt, of dat is herbouwd tot een ander gebouw, maar wel dezelfde functie heeft behouden en vaak nog dezelfde naam draagt. De term wordt vaak, maar niet uitsluitend, gebruikt voor archeologische sites met dit kenmerk, en verwijst zowel naar de site als naar alle constructies die in de loop van de tijd op de site hebben gestaan. Voorbeelden zijn de Azteekse Templo Mayor, die zesmaal op dezelfde site herbouwd is, de joodse tempel in Jeruzalem, eveneens meerdere malen op dezelfde site herbouwd, en Stonehenge, dat in de loop der eeuwen is gegroeid. Gebruik 'bouwterreinen' om in het algemeen te verwijzen naar een site waar zich een gebouw bevindt of bevonden heeft, of waar de bouw nog aan de gang is.
"""@nl ;
  rdfs:isDefinedBy <https://w3id.org/con-tax/zones/aat-buildingSites> ;
  rdfs:label "herbouwsite"@nl ;
  rdfs:label "herbouwsites"@nl ;
  rdfs:label "rebuilding sites"@en ;
  rdfs:seeAlso <http://vocab.getty.edu/aat/300404840> ;
  rdfs:subClassOf <https://w3id.org/con-tax/zones/aat-buildingSites#300000809> ;
.
<https://w3id.org/con-tax/zones/aat-buildingSites#300404907>
  rdf:type owl:Class ;
  rdfs:comment """Sedimentaire afzettingen die grote hoeveelheden bewaard gebleven fossielen bevatten. Paleontologen verdelen ze in twee subtypen: Konservat-Lagerstätten en Konzentrat-Lagerstätten. De laatste verwijst naar afzettingen van fossielen die zich in een geconcentreerde toestand bevinden door sedimentologische processen waarbij geen details (zoals organen) bewaard blijven, en de eerste verwijst naar afzettingen met een grote concentratie fossielen die uitzonderlijk goed bewaard zijn gebleven.
"""@nl ;
  rdfs:comment "Sedimentary deposits which contain large amounts of preserved fossils. Paleontologists divide them into two subtypes: Konservat-Lagerstätten and Konzentrat-Lagerstätten. The latter relates to desposits of fossils that are concentrated by sedimentological processes which do not preserve details (such as organs), and the former refers to deposits containing a large concentration of fossils that are exceptionally well-preserved."@en ;
  rdfs:isDefinedBy <https://w3id.org/con-tax/zones/aat-buildingSites> ;
  rdfs:label "Lagerstätte"@nl ;
  rdfs:label "Lagerstätten"@en ;
  rdfs:label "Lagerstätten"@nl ;
  rdfs:seeAlso <http://vocab.getty.edu/aat/300404907> ;
  rdfs:subClassOf <https://w3id.org/con-tax/zones/aat-buildingSites#300266152> ;
.
<https://w3id.org/con-tax/zones/aat-buildingSites#300410262>
  rdf:type owl:Class ;
  rdfs:comment "Complexes of buildings comprising the permanent establishment of a Christian missionary post or station. Buildings may include the central church, structures for the housing of the friars or other personnell, kitchen, storage, barns, surrounding grounds, and possibly other buildings."@en ;
  rdfs:comment """Gebouwencomplexen waar permanent een christelijke missie gevestigd is. Een missie kan onder meer bestaan uit de centrale kerk, gebouwen voor broeders of ander personeel, keuken, opslagplaats, schuren en omringend land.
"""@nl ;
  rdfs:isDefinedBy <https://w3id.org/con-tax/zones/aat-buildingSites> ;
  rdfs:label "missiepost (gebouwen)"@nl ;
  rdfs:label "missiepost"@nl ;
  rdfs:label "missieposten (gebouwen)"@nl ;
  rdfs:label "missieposten"@nl ;
  rdfs:label "missions (complexes)"@en ;
  rdfs:seeAlso <http://vocab.getty.edu/aat/300410262> ;
  rdfs:subClassOf <https://w3id.org/con-tax/zones/aat-buildingSites#300000202> ;
.
<https://w3id.org/con-tax/zones/aat-buildingSites#300410458>
  rdf:type owl:Class ;
  rdfs:comment """Militaire terreinen die in de eerste plaats of geheel gereserveerd zijn voor het schieten met artillerie: vuurwapens met een kaliber van meer dan een inch (2,5 cm).
"""@nl ;
  rdfs:comment "Military ranges reserved primarily or entirely to the firing of artillery, which include firearms generally having a bore of over one inch in diameter."@en ;
  rdfs:isDefinedBy <https://w3id.org/con-tax/zones/aat-buildingSites> ;
  rdfs:label "artillerieterrein"@nl ;
  rdfs:label "artillerieterreinen"@nl ;
  rdfs:label "artillery ranges"@en ;
  rdfs:seeAlso <http://vocab.getty.edu/aat/300410458> ;
  rdfs:subClassOf <https://w3id.org/con-tax/zones/aat-buildingSites#300000451> ;
.
<https://w3id.org/con-tax/zones/aat-buildingSites#300411363>
  rdf:type owl:Class ;
  rdfs:comment "Plaats waar een straf voltrokken wordt."@nl ;
  rdfs:comment "Places, either sites or structures, set aside by a community, ruler, etc. for delivering corporal punishment or executions."@en ;
  rdfs:isDefinedBy <https://w3id.org/con-tax/zones/aat-buildingSites> ;
  rdfs:label "executieplaats"@nl ;
  rdfs:label "executieplaatsen"@nl ;
  rdfs:label "gerechtsplaats"@nl ;
  rdfs:label "gerechtsplaatsen"@nl ;
  rdfs:label "places of punishment"@en ;
  rdfs:label "strafplaats"@nl ;
  rdfs:label "strafplaatsen"@nl ;
  rdfs:label "strafvoltrekkingsplaats"@nl ;
  rdfs:label "strafvoltrekkingsplaatsen"@nl ;
  rdfs:seeAlso <http://vocab.getty.edu/aat/300411363> ;
  rdfs:subClassOf <https://w3id.org/con-tax/zones/aat-buildingSites#300000809> ;
.
<https://w3id.org/con-tax/zones/aat-buildingSites#300411503>
  rdf:type owl:Class ;
  rdfs:comment "Bedrijven van bijenhouders waar de bijen meestal in bijenkorven gehouden worden."@nl ;
  rdfs:comment "Complexes or plots of land where bees are raised in apiaries and where their products collected for livelihood or commerce."@en ;
  rdfs:isDefinedBy <https://w3id.org/con-tax/zones/aat-buildingSites> ;
  rdfs:label "bee farms"@en ;
  rdfs:label "imkerij"@nl ;
  rdfs:label "imkerijen (bedrijven)"@nl ;
  rdfs:label "imkerijen"@nl ;
  rdfs:seeAlso <http://vocab.getty.edu/aat/300411503> ;
  rdfs:subClassOf <https://w3id.org/con-tax/zones/aat-buildingSites#300000206> ;
.
<https://w3id.org/con-tax/zones/aat-buildingSites#300411506>
  rdf:type owl:Class ;
  rdfs:comment "Een heuvel om goederentreinen te splitsen met daarover een of meerdere sporen waar de te heuvelen wagens overheen worden geduwd die vervolgens door de zwaartekracht zelfstandig verder rollen."@nl ;
  rdfs:comment "Railway yards that employ lead tracks on small rises over which an engine pushes single cars, or blocks of coupled cars, where they roll by gravity onto destination tracks where the cars are sorted."@en ;
  rdfs:isDefinedBy <https://w3id.org/con-tax/zones/aat-buildingSites> ;
  rdfs:label "hump yards"@en ;
  rdfs:label "rangeerheuvel"@nl ;
  rdfs:label "rangeerheuvels"@nl ;
  rdfs:seeAlso <http://vocab.getty.edu/aat/300411506> ;
  rdfs:subClassOf <https://w3id.org/con-tax/zones/aat-buildingSites#300000691> ;
.
<https://w3id.org/con-tax/zones/aat-buildingSites#300411558>
  rdf:type owl:Class ;
  rdfs:comment "Areas in the sea where oysters are cultivated for human consumption. "@en ;
  rdfs:comment "Plaats in zee waar men oesters kweekt."@nl ;
  rdfs:isDefinedBy <https://w3id.org/con-tax/zones/aat-buildingSites> ;
  rdfs:label "oesterkwekerij"@nl ;
  rdfs:label "oesterkwekerijen"@nl ;
  rdfs:label "oesterteelt"@nl ;
  rdfs:label "oyster farms"@en ;
  rdfs:seeAlso <http://vocab.getty.edu/aat/300411558> ;
  rdfs:subClassOf <https://w3id.org/con-tax/zones/aat-buildingSites#300000206> ;
.
<https://w3id.org/con-tax/zones/aat-buildingSites#300412066>
  rdf:type owl:Class ;
  rdfs:comment "Spiritual places in the Inca religion. Included are Pre-Columbian Inca tombs or temples, usually a truncated pyramid of stone, and often of immense size. Huacas could also be caves, springs, special rocks, and man-made shrines."@en ;
  rdfs:isDefinedBy <https://w3id.org/con-tax/zones/aat-buildingSites> ;
  rdfs:label "huacas"@en ;
  rdfs:seeAlso <http://vocab.getty.edu/aat/300412066> ;
  rdfs:subClassOf <https://w3id.org/con-tax/zones/aat-buildingSites#300386998> ;
.
<https://w3id.org/con-tax/zones/aat-buildingSites#300417317>
  rdf:type owl:Class ;
  rdfs:comment "Complexes of built works surrounding the palace or palaces of a ruler. An example is the Forbidden City in Beijing."@en ;
  rdfs:isDefinedBy <https://w3id.org/con-tax/zones/aat-buildingSites> ;
  rdfs:label "palace complexes"@en ;
  rdfs:seeAlso <http://vocab.getty.edu/aat/300417317> ;
  rdfs:subClassOf <https://w3id.org/con-tax/zones/aat-buildingSites#300000202> ;
.
<https://w3id.org/con-tax/zones/aat-buildingSites#300417706>
  rdf:type owl:Class ;
  rdfs:comment "Recreational parks that are open to the public."@en ;
  rdfs:isDefinedBy <https://w3id.org/con-tax/zones/aat-buildingSites> ;
  rdfs:label "public parks"@en ;
  rdfs:seeAlso <http://vocab.getty.edu/aat/300417706> ;
  rdfs:subClassOf <https://w3id.org/con-tax/zones/aat-buildingSites#300008187> ;
.
